@prefix : <http://peterbrau.com/yeast/> .
@prefix gr: <http://purl.org/goodrelations/v1#> .
@prefix owl: <http://www.w3.org/2002/07/owl#> .
@prefix rdf: <http://www.w3.org/1999/02/22-rdf-syntax-ns#> .
@prefix wlp: <http://peterbrau.com/whitelabs/yeast-bank/> .
@prefix xml: <http://www.w3.org/XML/1998/namespace> .
@prefix xsd: <http://www.w3.org/2001/XMLSchema#> .
@prefix rdfs: <http://www.w3.org/2000/01/rdf-schema#> .
@prefix skos: <http://www.w3.org/2004/02/skos/core#> .
@prefix vann: <http://purl.org/vocab/vann/> .
@prefix bevon: <http://rdfs.co/bevon/> .
@prefix yeast: <http://peterbrau.com/yeast/> .
@prefix dcterms: <http://purl.org/dc/terms/> .
@prefix dc: <http://purl.org/dc/elements/1.1/> .
@prefix beertype: <http://peterbrau.com/whitelabs/yeast-bank-types/> .
@base <http://peterbrau.com/yeast/> .

<http://peterbrau.com/yeast/> rdf:type owl:Ontology ;
                               dc:title "The Brewer's Yeast Ontology" ;
                               owl:versionIRI <http://peterbrau.com/yeast/1.0.0> ;
                               owl:imports <http://rdfs.co/bevon/0.8> ;
                               vann:preferredNamespacePrefix "yeast" ;
                               vann:preferredNamespaceUri "http://peterbrau.com/yeast/" .

#################################################################
#    Annotation properties
#################################################################

###  http://peterbrau.com/yeast/usedForBrewingStyle
yeast:usedForBrewingStyle rdf:type owl:AnnotationProperty ;
                          rdfs:label "used for brewing style" ;
                          skos:prefLabel "used for brewing style" ;
                          rdfs:range bevon:FermentedBeverage ;
                          rdfs:domain yeast:BrewersYeast .


###  http://purl.org/dc/terms/bibliographicCitation
dcterms:bibliographicCitation rdf:type owl:AnnotationProperty .


###  http://purl.org/goodrelations/v1#hasMPN
gr:hasMPN rdf:type owl:AnnotationProperty .


###  http://www.w3.org/2004/02/skos/core#broader
skos:broader rdf:type owl:AnnotationProperty .


###  http://www.w3.org/2004/02/skos/core#definition
skos:definition rdf:type owl:AnnotationProperty .


###  http://www.w3.org/2004/02/skos/core#exactMatch
skos:exactMatch rdf:type owl:AnnotationProperty .


###  http://www.w3.org/2004/02/skos/core#prefLabel
skos:prefLabel rdf:type owl:AnnotationProperty .


#################################################################
#    Data properties
#################################################################

###  http://peterbrau.com/yeast/hasAlcoholTolerance
yeast:hasAlcoholTolerance rdf:type owl:DatatypeProperty ;
                          rdfs:domain yeast:BrewersYeast ;
                          rdfs:range xsd:string ;
                          rdfs:label "has Alcohol Tolerance" ;
                          skos:prefLabel "has Alcohol Tolerance" .


###  http://peterbrau.com/yeast/hasFlocculation
yeast:hasFlocculation rdf:type owl:DatatypeProperty ;
                      rdfs:domain yeast:BrewersYeast ;
                      rdfs:range xsd:string ;
                      rdfs:label "has Flocculation" ;
                      skos:prefLabel "has Flocculation" .


###  http://peterbrau.com/yeast/hasHighAttenuation
yeast:hasHighAttenuation rdf:type owl:DatatypeProperty ;
                         rdfs:domain yeast:BrewersYeast ;
                         rdfs:range xsd:decimal ;
                         rdfs:label "has High Attenuation" ;
                         skos:prefLabel "has High Attenuation" .


###  http://peterbrau.com/yeast/hasHighOptimumFermentationTemperature
yeast:hasHighOptimumFermentationTemperature rdf:type owl:DatatypeProperty ;
                                            rdfs:domain yeast:BrewersYeast ;
                                            rdfs:range xsd:decimal ;
                                            rdfs:label "has High Optimum Fermentation Temperature" ;
                                            skos:prefLabel "has High Optimum Fermentation Temperature" .


###  http://peterbrau.com/yeast/hasLowAttenuation
yeast:hasLowAttenuation rdf:type owl:DatatypeProperty ;
                        rdfs:domain yeast:BrewersYeast ;
                        rdfs:range xsd:decimal ;
                        rdfs:label "has Low Attenuation" ;
                        skos:prefLabel "has Low Attenuation" .


###  http://peterbrau.com/yeast/hasLowOptimumFermentationTemperature
yeast:hasLowOptimumFermentationTemperature rdf:type owl:DatatypeProperty ;
                                           rdfs:domain yeast:BrewersYeast ;
                                           rdfs:range xsd:decimal ;
                                           rdfs:label "has Low Optimum Fermentation Temperature" ;
                                           skos:prefLabel "has Low Optimum Fermentation Temperature" .


#################################################################
#    Classes
#################################################################

###  http://peterbrau.com/whitelabs/yeast-bank-types/american-amber
beertype:american-amber rdf:type owl:Class ;
                        rdfs:subClassOf bevon:Beer ;
                        dcterms:bibliographicCitation "http://www.whitelabs.com/category/yeast-bank-types/american-amber" ;
                        rdfs:label "American Amber" ;
                        skos:prefLabel "American Amber" .


###  http://peterbrau.com/whitelabs/yeast-bank-types/american-brown-ale
beertype:american-brown-ale rdf:type owl:Class ;
                            rdfs:subClassOf bevon:Beer ;
                            dcterms:bibliographicCitation "http://www.whitelabs.com/category/yeast-bank-types/american-brown-ale" ;
                            rdfs:label "American Brown Ale" ;
                            skos:prefLabel "American Brown Ale" .


###  http://peterbrau.com/whitelabs/yeast-bank-types/american-india-pale-ale
beertype:american-india-pale-ale rdf:type owl:Class ;
                                 rdfs:subClassOf bevon:Beer ;
                                 dcterms:bibliographicCitation "http://www.whitelabs.com/category/yeast-bank-types/american-india-pale-ale" ;
                                 rdfs:label "American India Pale Ale" ;
                                 skos:prefLabel "American India Pale Ale" .


###  http://peterbrau.com/whitelabs/yeast-bank-types/american-lager
beertype:american-lager rdf:type owl:Class ;
                        rdfs:subClassOf bevon:Beer ;
                        dcterms:bibliographicCitation "http://www.whitelabs.com/category/yeast-bank-types/american-lager" ;
                        rdfs:label "American Lager" ;
                        skos:broader bevon:Lager ;
                        skos:prefLabel "American Lager" .


###  http://peterbrau.com/whitelabs/yeast-bank-types/american-light-lager
beertype:american-light-lager rdf:type owl:Class ;
                              rdfs:subClassOf bevon:Beer ;
                              dcterms:bibliographicCitation "http://www.whitelabs.com/category/yeast-bank-types/american-light-lager" ;
                              rdfs:label "American Light Lager" ;
                              skos:broader bevon:Lager ;
                              skos:prefLabel "American Light Lager" .


###  http://peterbrau.com/whitelabs/yeast-bank-types/american-pale-ale
beertype:american-pale-ale rdf:type owl:Class ;
                           rdfs:subClassOf bevon:Beer ;
                           dcterms:bibliographicCitation "http://www.whitelabs.com/category/yeast-bank-types/american-pale-ale" ;
                           rdfs:label "American Pale Ale" ;
                           skos:broader bevon:PaleAle ;
                           skos:prefLabel "American Pale Ale" .


###  http://peterbrau.com/whitelabs/yeast-bank-types/american-porter
beertype:american-porter rdf:type owl:Class ;
                         rdfs:subClassOf bevon:Beer ;
                         dcterms:bibliographicCitation "http://www.whitelabs.com/category/yeast-bank-types/american-porter" ;
                         rdfs:label "American Porter" ;
                         skos:broader bevon:Porter ;
                         skos:prefLabel "American Porter" .


###  http://peterbrau.com/whitelabs/yeast-bank-types/american-stout
beertype:american-stout rdf:type owl:Class ;
                        rdfs:subClassOf bevon:Beer ;
                        dcterms:bibliographicCitation "http://www.whitelabs.com/category/yeast-bank-types/american-stout" ;
                        rdfs:label "American Stout" ;
                        skos:broader bevon:Stout ;
                        skos:prefLabel "American Stout" .


###  http://peterbrau.com/whitelabs/yeast-bank-types/american-wheat-ale
beertype:american-wheat-ale rdf:type owl:Class ;
                            rdfs:subClassOf bevon:Beer ;
                            dcterms:bibliographicCitation "http://www.whitelabs.com/category/yeast-bank-types/american-wheat-ale" ;
                            rdfs:label "American Wheat Ale" ;
                            skos:prefLabel "American Wheat Ale" .


###  http://peterbrau.com/whitelabs/yeast-bank-types/apple-wine
beertype:apple-wine rdf:type owl:Class ;
                    rdfs:subClassOf bevon:Wine ;
                    dcterms:bibliographicCitation "http://www.whitelabs.com/category/yeast-bank-types/apple-wine" ;
                    rdfs:label "Apple Wine" ;
                    skos:prefLabel "Apple Wine" .


###  http://peterbrau.com/whitelabs/yeast-bank-types/baltic-style-porter
beertype:baltic-style-porter rdf:type owl:Class ;
                             rdfs:subClassOf bevon:Beer ;
                             dcterms:bibliographicCitation "http://www.whitelabs.com/category/yeast-bank-types/baltic-style-porter" ;
                             rdfs:label "Baltic-Style Porter" ;
                             skos:broader bevon:Porter ;
                             skos:prefLabel "Baltic-Style Porter" .


###  http://peterbrau.com/whitelabs/yeast-bank-types/barleywine-ale
beertype:barleywine-ale rdf:type owl:Class ;
                        rdfs:subClassOf bevon:Beer ;
                        dcterms:bibliographicCitation "http://www.whitelabs.com/category/yeast-bank-types/barleywine-ale" ;
                        rdfs:label "Barleywine Ale" ;
                        skos:prefLabel "Barleywine Ale" .


###  http://peterbrau.com/whitelabs/yeast-bank-types/belgian-blond
beertype:belgian-blond rdf:type owl:Class ;
                       rdfs:subClassOf bevon:Beer ;
                       dcterms:bibliographicCitation "http://www.whitelabs.com/category/yeast-bank-types/belgian-blond" ;
                       rdfs:label "Belgian Blond" ;
                       skos:prefLabel "Belgian Blond" .


###  http://peterbrau.com/whitelabs/yeast-bank-types/belgian-dark-strong-ale
beertype:belgian-dark-strong-ale rdf:type owl:Class ;
                                 rdfs:subClassOf bevon:Beer ;
                                 dcterms:bibliographicCitation "http://www.whitelabs.com/category/yeast-bank-types/belgian-dark-strong-ale" ;
                                 rdfs:label "Belgian Dark Strong Ale" ;
                                 skos:prefLabel "Belgian Dark Strong Ale" .


###  http://peterbrau.com/whitelabs/yeast-bank-types/belgian-table-bier
beertype:belgian-table-bier rdf:type owl:Class ;
                            rdfs:subClassOf bevon:Beer ;
                            dcterms:bibliographicCitation "http://www.whitelabs.com/category/yeast-bank-types/belgian-table-bier" ;
                            rdfs:label "Belgian Table Bier" ;
                            skos:prefLabel "Belgian Table Bier" .


###  http://peterbrau.com/whitelabs/yeast-bank-types/belgian-wit
beertype:belgian-wit rdf:type owl:Class ;
                     rdfs:subClassOf bevon:Beer ;
                     dcterms:bibliographicCitation "http://www.whitelabs.com/category/yeast-bank-types/belgian-wit" ;
                     rdfs:label "Belgian Wit" ;
                     skos:prefLabel "Belgian Wit" .


###  http://peterbrau.com/whitelabs/yeast-bank-types/berliner-weisse
beertype:berliner-weisse rdf:type owl:Class ;
                         rdfs:subClassOf bevon:Beer ;
                         dcterms:bibliographicCitation "http://www.whitelabs.com/category/yeast-bank-types/berliner-weisse" ;
                         rdfs:label "Berliner Weisse" ;
                         skos:prefLabel "Berliner Weisse" .


###  http://peterbrau.com/whitelabs/yeast-bank-types/biere-de-garde
beertype:biere-de-garde rdf:type owl:Class ;
                        rdfs:subClassOf bevon:Beer ;
                        dcterms:bibliographicCitation "http://www.whitelabs.com/category/yeast-bank-types/biere-de-garde" ;
                        rdfs:label "Biere de Garde" ;
                        skos:prefLabel "Biere de Garde" .


###  http://peterbrau.com/whitelabs/yeast-bank-types/blonde-ale
beertype:blonde-ale rdf:type owl:Class ;
                    rdfs:subClassOf bevon:Beer ;
                    dcterms:bibliographicCitation "http://www.whitelabs.com/category/yeast-bank-types/blonde-ale" ;
                    rdfs:label "Blonde Ale" ;
                    skos:prefLabel "Blonde Ale" .


###  http://peterbrau.com/whitelabs/yeast-bank-types/bock
beertype:bock rdf:type owl:Class ;
              rdfs:subClassOf bevon:Beer ;
              dcterms:bibliographicCitation "http://www.whitelabs.com/category/yeast-bank-types/bock" ;
              rdfs:label "Bock" ;
              skos:prefLabel "Bock" .


###  http://peterbrau.com/whitelabs/yeast-bank-types/bohemian-pilsner
beertype:bohemian-pilsner rdf:type owl:Class ;
                          owl:equivalentClass bevon:Pilsner ;
                          rdfs:subClassOf bevon:Beer ;
                          dcterms:bibliographicCitation "http://www.whitelabs.com/category/yeast-bank-types/bohemian-pilsner" ;
                          rdfs:label "Bohemian Pilsner" ;
                          skos:prefLabel "Bohemian Pilsner" .


###  http://peterbrau.com/whitelabs/yeast-bank-types/bourbon-whiskey
beertype:bourbon-whiskey rdf:type owl:Class ;
                         rdfs:subClassOf bevon:BourbonWhiskey ;
                         dcterms:bibliographicCitation "http://www.whitelabs.com/category/yeast-bank-types/bourbon-whiskey" ;
                         rdfs:label "Bourbon Whiskey" ;
                         skos:prefLabel "Bourbon Whiskey" .


###  http://peterbrau.com/whitelabs/yeast-bank-types/braggot
beertype:braggot rdf:type owl:Class ;
                 rdfs:subClassOf yeast:Mead ;
                 dcterms:bibliographicCitation "http://www.whitelabs.com/category/yeast-bank-types/braggot" ;
                 rdfs:label "Braggot" ;
                 skos:prefLabel "Braggot" .


###  http://peterbrau.com/whitelabs/yeast-bank-types/brandy
beertype:brandy rdf:type owl:Class ;
                rdfs:subClassOf bevon:Brandy ;
                dcterms:bibliographicCitation "http://www.whitelabs.com/category/yeast-bank-types/brandy" ;
                rdfs:label "Brandy" ;
                skos:prefLabel "Brandy" .


###  http://peterbrau.com/whitelabs/yeast-bank-types/cabernet-franc
beertype:cabernet-franc rdf:type owl:Class ;
                        rdfs:subClassOf bevon:Wine ;
                        dcterms:bibliographicCitation "http://www.whitelabs.com/category/yeast-bank-types/cabernet-franc" ;
                        rdfs:label "Cabernet Franc" ;
                        skos:prefLabel "Cabernet Franc" .


###  http://peterbrau.com/whitelabs/yeast-bank-types/cabernet-sauvignon
beertype:cabernet-sauvignon rdf:type owl:Class ;
                            rdfs:subClassOf bevon:Wine ;
                            dcterms:bibliographicCitation "http://www.whitelabs.com/category/yeast-bank-types/cabernet-sauvignon" ;
                            rdfs:label "Cabernet Sauvignon" ;
                            skos:prefLabel "Cabernet Sauvignon" .


###  http://peterbrau.com/whitelabs/yeast-bank-types/champagne-sparkling-wine
beertype:champagne-sparkling-wine rdf:type owl:Class ;
                                  rdfs:subClassOf bevon:Wine ;
                                  dcterms:bibliographicCitation "http://www.whitelabs.com/category/yeast-bank-types/champagne-sparkling-wine" ;
                                  rdfs:label "Champagne/Sparkling Wine" ;
                                  skos:prefLabel "Champagne/Sparkling Wine" .


###  http://peterbrau.com/whitelabs/yeast-bank-types/chardonnay
beertype:chardonnay rdf:type owl:Class ;
                    rdfs:subClassOf bevon:Wine ;
                    dcterms:bibliographicCitation "http://www.whitelabs.com/category/yeast-bank-types/chardonnay" ;
                    rdfs:label "Chardonnay" ;
                    skos:prefLabel "Chardonnay" .


###  http://peterbrau.com/whitelabs/yeast-bank-types/cider
beertype:cider rdf:type owl:Class ;
               rdfs:subClassOf yeast:Cider ;
               dcterms:bibliographicCitation "http://www.whitelabs.com/category/yeast-bank-types/cider" ;
               rdfs:label "Cider" ;
               skos:prefLabel "Cider" .


###  http://peterbrau.com/whitelabs/yeast-bank-types/common-perry
beertype:common-perry rdf:type owl:Class ;
                      rdfs:subClassOf yeast:Perry ;
                      dcterms:bibliographicCitation "http://www.whitelabs.com/category/yeast-bank-types/common-perry" ;
                      rdfs:label "Common Perry" ;
                      skos:prefLabel "Common Perry" .


###  http://peterbrau.com/whitelabs/yeast-bank-types/cream-ale
beertype:cream-ale rdf:type owl:Class ;
                   rdfs:subClassOf bevon:Beer ;
                   dcterms:bibliographicCitation "http://www.whitelabs.com/category/yeast-bank-types/cream-ale" ;
                   rdfs:label "Cream Ale" ;
                   skos:prefLabel "Cream Ale" .


###  http://peterbrau.com/whitelabs/yeast-bank-types/cyser
beertype:cyser rdf:type owl:Class ;
               rdfs:subClassOf yeast:Mead ;
               dcterms:bibliographicCitation "http://www.whitelabs.com/category/yeast-bank-types/cyser" ;
               rdfs:label "Cyser" ;
               skos:prefLabel "Cyser" .


###  http://peterbrau.com/whitelabs/yeast-bank-types/doppelbock
beertype:doppelbock rdf:type owl:Class ;
                    rdfs:subClassOf bevon:Beer ;
                    dcterms:bibliographicCitation "http://www.whitelabs.com/category/yeast-bank-types/doppelbock" ;
                    rdfs:label "Doppelbock" ;
                    skos:prefLabel "Doppelbock" .


###  http://peterbrau.com/whitelabs/yeast-bank-types/dubbel
beertype:dubbel rdf:type owl:Class ;
                rdfs:subClassOf bevon:Beer ;
                dcterms:bibliographicCitation "http://www.whitelabs.com/category/yeast-bank-types/dubbel" ;
                rdfs:label "Dubbel" ;
                skos:prefLabel "Dubbel" .


###  http://peterbrau.com/whitelabs/yeast-bank-types/dusseldorf-altbier
beertype:dusseldorf-altbier rdf:type owl:Class ;
                            rdfs:subClassOf bevon:Beer ;
                            dcterms:bibliographicCitation "http://www.whitelabs.com/category/yeast-bank-types/dusseldorf-altbier" ;
                            rdfs:label "Dusseldorf Altbier" ;
                            skos:prefLabel "Dusseldorf Altbier" .


###  http://peterbrau.com/whitelabs/yeast-bank-types/english-brown-ale
beertype:english-brown-ale rdf:type owl:Class ;
                           rdfs:subClassOf bevon:Beer ;
                           dcterms:bibliographicCitation "http://www.whitelabs.com/category/yeast-bank-types/english-brown-ale" ;
                           rdfs:label "English Brown Ale" ;
                           skos:prefLabel "English Brown Ale" .


###  http://peterbrau.com/whitelabs/yeast-bank-types/english-cider
beertype:english-cider rdf:type owl:Class ;
                       rdfs:subClassOf yeast:Cider ;
                       dcterms:bibliographicCitation "http://www.whitelabs.com/category/yeast-bank-types/english-cider" ;
                       rdfs:label "English Cider" ;
                       skos:prefLabel "English Cider" .


###  http://peterbrau.com/whitelabs/yeast-bank-types/english-india-pale-ale
beertype:english-india-pale-ale rdf:type owl:Class ;
                                rdfs:subClassOf bevon:Beer ;
                                dcterms:bibliographicCitation "http://www.whitelabs.com/category/yeast-bank-types/english-india-pale-ale" ;
                                rdfs:label "English India Pale Ale" ;
                                skos:prefLabel "English India Pale Ale" .


###  http://peterbrau.com/whitelabs/yeast-bank-types/english-old-ale
beertype:english-old-ale rdf:type owl:Class ;
                         rdfs:subClassOf bevon:Beer ;
                         dcterms:bibliographicCitation "http://www.whitelabs.com/category/yeast-bank-types/english-old-ale" ;
                         rdfs:label "English Old Ale" ;
                         skos:prefLabel "English Old Ale" .


###  http://peterbrau.com/whitelabs/yeast-bank-types/english-pale-ale
beertype:english-pale-ale rdf:type owl:Class ;
                          rdfs:subClassOf bevon:Beer ;
                          dcterms:bibliographicCitation "http://www.whitelabs.com/category/yeast-bank-types/english-pale-ale" ;
                          rdfs:label "English Pale Ale" ;
                          skos:broader bevon:PaleAle ;
                          skos:prefLabel "English Pale Ale" .


###  http://peterbrau.com/whitelabs/yeast-bank-types/extra-special-bitter
beertype:extra-special-bitter rdf:type owl:Class ;
                              rdfs:subClassOf bevon:Beer ;
                              dcterms:bibliographicCitation "http://www.whitelabs.com/category/yeast-bank-types/extra-special-bitter" ;
                              rdfs:label "Extra Special Bitter" ;
                              skos:prefLabel "Extra Special Bitter" .


###  http://peterbrau.com/whitelabs/yeast-bank-types/flanders-brown
beertype:flanders-brown rdf:type owl:Class ;
                        rdfs:subClassOf bevon:Beer ;
                        dcterms:bibliographicCitation "http://www.whitelabs.com/category/yeast-bank-types/flanders-brown" ;
                        rdfs:label "Flanders Brown" ;
                        skos:prefLabel "Flanders Brown" .


###  http://peterbrau.com/whitelabs/yeast-bank-types/flanders-red
beertype:flanders-red rdf:type owl:Class ;
                      rdfs:subClassOf bevon:Beer ;
                      dcterms:bibliographicCitation "http://www.whitelabs.com/category/yeast-bank-types/flanders-red" ;
                      rdfs:label "Flanders Red" ;
                      skos:prefLabel "Flanders Red" .


###  http://peterbrau.com/whitelabs/yeast-bank-types/foreign-export-stout
beertype:foreign-export-stout rdf:type owl:Class ;
                              rdfs:subClassOf bevon:Beer ;
                              dcterms:bibliographicCitation "http://www.whitelabs.com/category/yeast-bank-types/foreign-export-stout" ;
                              rdfs:label "Foreign Export Stout" ;
                              skos:broader bevon:Stout ;
                              skos:prefLabel "Foreign Export Stout" .


###  http://peterbrau.com/whitelabs/yeast-bank-types/french-cider
beertype:french-cider rdf:type owl:Class ;
                      rdfs:subClassOf yeast:Cider ;
                      dcterms:bibliographicCitation "http://www.whitelabs.com/category/yeast-bank-types/french-cider" ;
                      rdfs:label "French Cider" ;
                      skos:prefLabel "French Cider" .


###  http://peterbrau.com/whitelabs/yeast-bank-types/geuze
beertype:geuze rdf:type owl:Class ;
               rdfs:subClassOf bevon:Beer ;
               dcterms:bibliographicCitation "http://www.whitelabs.com/category/yeast-bank-types/geuze" ;
               rdfs:label "Geuze" ;
               skos:prefLabel "Geuze" .


###  http://peterbrau.com/whitelabs/yeast-bank-types/gew-rztraminer
beertype:gew-rztraminer rdf:type owl:Class ;
                        rdfs:subClassOf bevon:Wine ;
                        dcterms:bibliographicCitation "http://www.whitelabs.com/category/yeast-bank-types/gew-rztraminer" ;
                        rdfs:label "Gewürztraminer" ;
                        skos:prefLabel "Gewürztraminer" .


###  http://peterbrau.com/whitelabs/yeast-bank-types/gin
beertype:gin rdf:type owl:Class ;
             rdfs:subClassOf bevon:Gin ;
             dcterms:bibliographicCitation "http://www.whitelabs.com/category/yeast-bank-types/gin" ;
             rdfs:label "Gin" ;
             skos:prefLabel "Gin" .


###  http://peterbrau.com/whitelabs/yeast-bank-types/gose
beertype:gose rdf:type owl:Class ;
              rdfs:subClassOf bevon:Beer ;
              dcterms:bibliographicCitation "http://www.whitelabs.com/category/yeast-bank-types/gose" ;
              rdfs:label "Gose" ;
              skos:prefLabel "Gose" .


###  http://peterbrau.com/whitelabs/yeast-bank-types/grappa
beertype:grappa rdf:type owl:Class ;
                rdfs:subClassOf bevon:Brandy ;
                dcterms:bibliographicCitation "http://www.whitelabs.com/category/yeast-bank-types/grappa" ;
                rdfs:label "Grappa" ;
                skos:prefLabel "Grappa" .


###  http://peterbrau.com/whitelabs/yeast-bank-types/grenache
beertype:grenache rdf:type owl:Class ;
                  rdfs:subClassOf bevon:Wine ;
                  dcterms:bibliographicCitation "http://www.whitelabs.com/category/yeast-bank-types/grenache" ;
                  rdfs:label "Grenache" ;
                  skos:prefLabel "Grenache" .


###  http://peterbrau.com/whitelabs/yeast-bank-types/hazy-ipa-pale-ale
beertype:hazy-ipa-pale-ale rdf:type owl:Class ;
                           rdfs:subClassOf bevon:Beer ;
                           dcterms:bibliographicCitation "http://www.whitelabs.com/category/yeast-bank-types/hazy-ipa-pale-ale" ;
                           rdfs:label "Hazy IPA/Pale Ale" ;
                           skos:prefLabel "Hazy IPA/Pale Ale" .


###  http://peterbrau.com/whitelabs/yeast-bank-types/hefeweizen
beertype:hefeweizen rdf:type owl:Class ;
                    rdfs:subClassOf bevon:Beer ;
                    dcterms:bibliographicCitation "http://www.whitelabs.com/category/yeast-bank-types/hefeweizen" ;
                    rdfs:label "Hefeweizen" ;
                    skos:prefLabel "Hefeweizen" .


###  http://peterbrau.com/whitelabs/yeast-bank-types/imperial-india-pale-ale
beertype:imperial-india-pale-ale rdf:type owl:Class ;
                                 rdfs:subClassOf bevon:Beer ;
                                 dcterms:bibliographicCitation "http://www.whitelabs.com/category/yeast-bank-types/imperial-india-pale-ale" ;
                                 rdfs:label "Imperial India Pale Ale" ;
                                 skos:prefLabel "Imperial India Pale Ale" .


###  http://peterbrau.com/whitelabs/yeast-bank-types/imperial-stout
beertype:imperial-stout rdf:type owl:Class ;
                        rdfs:subClassOf bevon:Beer ;
                        dcterms:bibliographicCitation "http://www.whitelabs.com/category/yeast-bank-types/imperial-stout" ;
                        rdfs:label "Imperial Stout" ;
                        skos:broader bevon:Stout ;
                        skos:prefLabel "Imperial Stout" .


###  http://peterbrau.com/whitelabs/yeast-bank-types/irish-dry-stout
beertype:irish-dry-stout rdf:type owl:Class ;
                         rdfs:subClassOf bevon:Beer ;
                         dcterms:bibliographicCitation "http://www.whitelabs.com/category/yeast-bank-types/irish-dry-stout" ;
                         rdfs:label "Irish Dry Stout" ;
                         skos:exactMatch bevon:DryStout ;
                         skos:prefLabel "Irish Dry Stout" .


###  http://peterbrau.com/whitelabs/yeast-bank-types/irish-red-ale
beertype:irish-red-ale rdf:type owl:Class ;
                       owl:equivalentClass bevon:IrishRedAle ;
                       rdfs:subClassOf bevon:Beer ;
                       dcterms:bibliographicCitation "http://www.whitelabs.com/category/yeast-bank-types/irish-red-ale" ;
                       rdfs:label "Irish Red Ale" ;
                       skos:prefLabel "Irish Red Ale" .


###  http://peterbrau.com/whitelabs/yeast-bank-types/kolsch
beertype:kolsch rdf:type owl:Class ;
                rdfs:subClassOf bevon:Beer ;
                dcterms:bibliographicCitation "http://www.whitelabs.com/category/yeast-bank-types/kolsch" ;
                rdfs:label "Kolsch" ;
                skos:prefLabel "Kolsch" .


###  http://peterbrau.com/whitelabs/yeast-bank-types/kombucha
beertype:kombucha rdf:type owl:Class ;
                  rdfs:subClassOf yeast:Kombucha ;
                  dcterms:bibliographicCitation "http://www.whitelabs.com/category/yeast-bank-types/kombucha" ;
                  rdfs:label "Kombucha" ;
                  skos:prefLabel "Kombucha" .


###  http://peterbrau.com/whitelabs/yeast-bank-types/kombucha-0
beertype:kombucha-0 rdf:type owl:Class ;
                    rdfs:subClassOf yeast:Kombucha ;
                    dcterms:bibliographicCitation "http://www.whitelabs.com/category/yeast-bank-types/kombucha-0" ;
                    rdfs:label "Kombucha" ;
                    skos:prefLabel "Kombucha" .


###  http://peterbrau.com/whitelabs/yeast-bank-types/lager
beertype:lager rdf:type owl:Class ;
               owl:equivalentClass bevon:Lager ;
               rdfs:subClassOf bevon:Beer ;
               dcterms:bibliographicCitation "http://www.whitelabs.com/category/yeast-bank-types/lager" ;
               rdfs:label "Lager" ;
               skos:prefLabel "Lager" .


###  http://peterbrau.com/whitelabs/yeast-bank-types/lambic
beertype:lambic rdf:type owl:Class ;
                rdfs:subClassOf bevon:Beer ;
                dcterms:bibliographicCitation "http://www.whitelabs.com/category/yeast-bank-types/lambic" ;
                rdfs:label "Lambic" ;
                skos:prefLabel "Lambic" .


###  http://peterbrau.com/whitelabs/yeast-bank-types/m-nchen-helles
beertype:m-nchen-helles rdf:type owl:Class ;
                        rdfs:subClassOf bevon:Beer ;
                        dcterms:bibliographicCitation "http://www.whitelabs.com/category/yeast-bank-types/m-nchen-helles" ;
                        rdfs:label "München Helles" ;
                        skos:prefLabel "München Helles" .


###  http://peterbrau.com/whitelabs/yeast-bank-types/m-nchner-dunkel
beertype:m-nchner-dunkel rdf:type owl:Class ;
                         owl:equivalentClass bevon:Dunkel ;
                         rdfs:subClassOf bevon:Beer ;
                         dcterms:bibliographicCitation "http://www.whitelabs.com/category/yeast-bank-types/m-nchner-dunkel" ;
                         rdfs:label "Münchner Dunkel" ;
                         skos:prefLabel "Münchner Dunkel" .


###  http://peterbrau.com/whitelabs/yeast-bank-types/m-rzen
beertype:m-rzen rdf:type owl:Class ;
                rdfs:subClassOf bevon:Beer ;
                dcterms:bibliographicCitation "http://www.whitelabs.com/category/yeast-bank-types/m-rzen" ;
                rdfs:label "Märzen" ;
                skos:prefLabel "Märzen" .


###  http://peterbrau.com/whitelabs/yeast-bank-types/madeira
beertype:madeira rdf:type owl:Class ;
                 rdfs:subClassOf bevon:Wine ;
                 dcterms:bibliographicCitation "http://www.whitelabs.com/category/yeast-bank-types/madeira" ;
                 rdfs:label "Madeira" ;
                 skos:prefLabel "Madeira" .


###  http://peterbrau.com/whitelabs/yeast-bank-types/malbec
beertype:malbec rdf:type owl:Class ;
                rdfs:subClassOf bevon:Wine ;
                dcterms:bibliographicCitation "http://www.whitelabs.com/category/yeast-bank-types/malbec" ;
                rdfs:label "Malbec" ;
                skos:prefLabel "Malbec" .


###  http://peterbrau.com/whitelabs/yeast-bank-types/merlot
beertype:merlot rdf:type owl:Class ;
                rdfs:subClassOf bevon:Wine ;
                dcterms:bibliographicCitation "http://www.whitelabs.com/category/yeast-bank-types/merlot" ;
                rdfs:label "Merlot" ;
                skos:prefLabel "Merlot" .


###  http://peterbrau.com/whitelabs/yeast-bank-types/nebbiolo
beertype:nebbiolo rdf:type owl:Class ;
                  rdfs:subClassOf bevon:Wine ;
                  dcterms:bibliographicCitation "http://www.whitelabs.com/category/yeast-bank-types/nebbiolo" ;
                  rdfs:label "Nebbiolo" ;
                  skos:prefLabel "Nebbiolo" .


###  http://peterbrau.com/whitelabs/yeast-bank-types/new-england-cider
beertype:new-england-cider rdf:type owl:Class ;
                           rdfs:subClassOf yeast:Cider ;
                           dcterms:bibliographicCitation "http://www.whitelabs.com/category/yeast-bank-types/new-england-cider" ;
                           rdfs:label "New England Cider" ;
                           skos:prefLabel "New England Cider" .


###  http://peterbrau.com/whitelabs/yeast-bank-types/oatmeal-stout
beertype:oatmeal-stout rdf:type owl:Class ;
                       rdfs:subClassOf bevon:Beer ;
                       dcterms:bibliographicCitation "http://www.whitelabs.com/category/yeast-bank-types/oatmeal-stout" ;
                       rdfs:label "Oatmeal Stout" ;
                       skos:broader bevon:Stout ;
                       skos:prefLabel "Oatmeal Stout" .


###  http://peterbrau.com/whitelabs/yeast-bank-types/ordinary-bitter
beertype:ordinary-bitter rdf:type owl:Class ;
                         rdfs:subClassOf bevon:Beer ;
                         dcterms:bibliographicCitation "http://www.whitelabs.com/category/yeast-bank-types/ordinary-bitter" ;
                         rdfs:label "Ordinary Bitter" ;
                         skos:prefLabel "Ordinary Bitter" .


###  http://peterbrau.com/whitelabs/yeast-bank-types/pinot-noir
beertype:pinot-noir rdf:type owl:Class ;
                    rdfs:subClassOf bevon:Wine ;
                    dcterms:bibliographicCitation "http://www.whitelabs.com/category/yeast-bank-types/pinot-noir" ;
                    rdfs:label "Pinot Noir" ;
                    skos:prefLabel "Pinot Noir" .


###  http://peterbrau.com/whitelabs/yeast-bank-types/port
beertype:port rdf:type owl:Class ;
              rdfs:subClassOf bevon:Wine ;
              dcterms:bibliographicCitation "http://www.whitelabs.com/category/yeast-bank-types/port" ;
              rdfs:label "Port" ;
              skos:prefLabel "Port" .


###  http://peterbrau.com/whitelabs/yeast-bank-types/riesling
beertype:riesling rdf:type owl:Class ;
                  rdfs:subClassOf bevon:Wine ;
                  dcterms:bibliographicCitation "http://www.whitelabs.com/category/yeast-bank-types/riesling" ;
                  rdfs:label "Riesling" ;
                  skos:prefLabel "Riesling" .


###  http://peterbrau.com/whitelabs/yeast-bank-types/rum
beertype:rum rdf:type owl:Class ;
             rdfs:subClassOf bevon:Rum ;
             dcterms:bibliographicCitation "http://www.whitelabs.com/category/yeast-bank-types/rum" ;
             rdfs:label "Rum" ;
             skos:prefLabel "Rum" .


###  http://peterbrau.com/whitelabs/yeast-bank-types/rye-whiskey
beertype:rye-whiskey rdf:type owl:Class ;
                     rdfs:subClassOf bevon:Whisky ;
                     dcterms:bibliographicCitation "http://www.whitelabs.com/category/yeast-bank-types/rye-whiskey" ;
                     rdfs:label "Rye Whiskey" ;
                     skos:prefLabel "Rye Whiskey" .


###  http://peterbrau.com/whitelabs/yeast-bank-types/saison
beertype:saison rdf:type owl:Class ;
                rdfs:subClassOf bevon:Beer ;
                dcterms:bibliographicCitation "http://www.whitelabs.com/category/yeast-bank-types/saison" ;
                rdfs:label "Saison" ;
                skos:prefLabel "Saison" .


###  http://peterbrau.com/whitelabs/yeast-bank-types/sake
beertype:sake rdf:type owl:Class ;
              rdfs:subClassOf bevon:Sake ;
              dcterms:bibliographicCitation "http://www.whitelabs.com/category/yeast-bank-types/sake" ;
              rdfs:label "Sake" ;
              skos:prefLabel "Sake" .


###  http://peterbrau.com/whitelabs/yeast-bank-types/sangiovese
beertype:sangiovese rdf:type owl:Class ;
                    rdfs:subClassOf bevon:Wine ;
                    dcterms:bibliographicCitation "http://www.whitelabs.com/category/yeast-bank-types/sangiovese" ;
                    rdfs:label "Sangiovese" ;
                    skos:prefLabel "Sangiovese" .


###  http://peterbrau.com/whitelabs/yeast-bank-types/sauvignon-blanc
beertype:sauvignon-blanc rdf:type owl:Class ;
                         rdfs:subClassOf bevon:Wine ;
                         dcterms:bibliographicCitation "http://www.whitelabs.com/category/yeast-bank-types/sauvignon-blanc" ;
                         rdfs:label "Sauvignon Blanc" ;
                         skos:prefLabel "Sauvignon Blanc" .


###  http://peterbrau.com/whitelabs/yeast-bank-types/schwarzbier
beertype:schwarzbier rdf:type owl:Class ;
                     rdfs:subClassOf bevon:Beer ;
                     dcterms:bibliographicCitation "http://www.whitelabs.com/category/yeast-bank-types/schwarzbier" ;
                     rdfs:label "Schwarzbier" ;
                     skos:prefLabel "Schwarzbier" .


###  http://peterbrau.com/whitelabs/yeast-bank-types/scotch-ale-wee-heavy
beertype:scotch-ale-wee-heavy rdf:type owl:Class ;
                              rdfs:subClassOf bevon:Beer ;
                              dcterms:bibliographicCitation "http://www.whitelabs.com/category/yeast-bank-types/scotch-ale-wee-heavy" ;
                              rdfs:label "Scotch Ale (Wee Heavy)" ;
                              skos:prefLabel "Scotch Ale (Wee Heavy)" .


###  http://peterbrau.com/whitelabs/yeast-bank-types/scotch-whisky
beertype:scotch-whisky rdf:type owl:Class ;
                       rdfs:subClassOf bevon:ScotchWhisky ;
                       dcterms:bibliographicCitation "http://www.whitelabs.com/category/yeast-bank-types/scotch-whisky" ;
                       rdfs:label "Scotch Whisky" ;
                       skos:prefLabel "Scotch Whisky" .


###  http://peterbrau.com/whitelabs/yeast-bank-types/semi-sweet-mead
beertype:semi-sweet-mead rdf:type owl:Class ;
                         rdfs:subClassOf yeast:Mead ;
                         dcterms:bibliographicCitation "http://www.whitelabs.com/category/yeast-bank-types/semi-sweet-mead" ;
                         rdfs:label "Semi-Sweet Mead" ;
                         skos:prefLabel "Semi-Sweet Mead" .


###  http://peterbrau.com/whitelabs/yeast-bank-types/semillon
beertype:semillon rdf:type owl:Class ;
                  rdfs:subClassOf bevon:Wine ;
                  dcterms:bibliographicCitation "http://www.whitelabs.com/category/yeast-bank-types/semillon" ;
                  rdfs:label "Semillon" ;
                  skos:prefLabel "Semillon" .


###  http://peterbrau.com/whitelabs/yeast-bank-types/sherry
beertype:sherry rdf:type owl:Class ;
                rdfs:subClassOf bevon:Wine ;
                dcterms:bibliographicCitation "http://www.whitelabs.com/category/yeast-bank-types/sherry" ;
                rdfs:label "Sherry" ;
                skos:prefLabel "Sherry" .


###  http://peterbrau.com/whitelabs/yeast-bank-types/shiraz
beertype:shiraz rdf:type owl:Class ;
                rdfs:subClassOf bevon:Wine ;
                dcterms:bibliographicCitation "http://www.whitelabs.com/category/yeast-bank-types/shiraz" ;
                rdfs:label "Shiraz" ;
                skos:prefLabel "Shiraz" .


###  http://peterbrau.com/whitelabs/yeast-bank-types/specialty-belgian
beertype:specialty-belgian rdf:type owl:Class ;
                           rdfs:subClassOf bevon:Beer ;
                           dcterms:bibliographicCitation "http://www.whitelabs.com/category/yeast-bank-types/specialty-belgian" ;
                           rdfs:label "Specialty / Belgian" ;
                           skos:prefLabel "Specialty / Belgian" .


###  http://peterbrau.com/whitelabs/yeast-bank-types/sweet-cider
beertype:sweet-cider rdf:type owl:Class ;
                     rdfs:subClassOf yeast:Cider ;
                     dcterms:bibliographicCitation "http://www.whitelabs.com/category/yeast-bank-types/sweet-cider" ;
                     rdfs:label "Sweet Cider" ;
                     skos:prefLabel "Sweet Cider" .


###  http://peterbrau.com/whitelabs/yeast-bank-types/sweet-mead
beertype:sweet-mead rdf:type owl:Class ;
                    rdfs:subClassOf yeast:Mead ;
                    dcterms:bibliographicCitation "http://www.whitelabs.com/category/yeast-bank-types/sweet-mead" ;
                    rdfs:label "Sweet Mead" ;
                    skos:prefLabel "Sweet Mead" .


###  http://peterbrau.com/whitelabs/yeast-bank-types/sweet-stout
beertype:sweet-stout rdf:type owl:Class ;
                     rdfs:subClassOf bevon:Beer ;
                     dcterms:bibliographicCitation "http://www.whitelabs.com/category/yeast-bank-types/sweet-stout" ;
                     rdfs:label "Sweet Stout" ;
                     skos:broader bevon:Stout ;
                     skos:prefLabel "Sweet Stout" .


###  http://peterbrau.com/whitelabs/yeast-bank-types/tequila
beertype:tequila rdf:type owl:Class ;
                 rdfs:subClassOf bevon:Tequila ;
                 dcterms:bibliographicCitation "http://www.whitelabs.com/category/yeast-bank-types/tequila" ;
                 rdfs:label "Tequila" ;
                 skos:prefLabel "Tequila" .


###  http://peterbrau.com/whitelabs/yeast-bank-types/traditional-perry
beertype:traditional-perry rdf:type owl:Class ;
                           rdfs:subClassOf yeast:Perry ;
                           dcterms:bibliographicCitation "http://www.whitelabs.com/category/yeast-bank-types/traditional-perry" ;
                           rdfs:label "Traditional Perry" ;
                           skos:prefLabel "Traditional Perry" .


###  http://peterbrau.com/whitelabs/yeast-bank-types/tripel
beertype:tripel rdf:type owl:Class ;
                rdfs:subClassOf bevon:Beer ;
                dcterms:bibliographicCitation "http://www.whitelabs.com/category/yeast-bank-types/tripel" ;
                rdfs:label "Tripel" ;
                skos:prefLabel "Tripel" .


###  http://peterbrau.com/whitelabs/yeast-bank-types/vienna-lager
beertype:vienna-lager rdf:type owl:Class ;
                      rdfs:subClassOf bevon:Beer ;
                      dcterms:bibliographicCitation "http://www.whitelabs.com/category/yeast-bank-types/vienna-lager" ;
                      rdfs:label "Vienna Lager" ;
                      skos:broader bevon:Lager ;
                      skos:prefLabel "Vienna Lager" .


###  http://peterbrau.com/whitelabs/yeast-bank-types/vodka
beertype:vodka rdf:type owl:Class ;
               rdfs:subClassOf bevon:Vodka ;
               dcterms:bibliographicCitation "http://www.whitelabs.com/category/yeast-bank-types/vodka" ;
               rdfs:label "Vodka" ;
               skos:prefLabel "Vodka" .


###  http://peterbrau.com/whitelabs/yeast-bank-types/wheat-ale
beertype:wheat-ale rdf:type owl:Class ;
                   rdfs:subClassOf bevon:Beer ;
                   dcterms:bibliographicCitation "http://www.whitelabs.com/category/yeast-bank-types/wheat-ale" ;
                   rdfs:label "Wheat Ale" ;
                   skos:prefLabel "Wheat Ale" .


###  http://peterbrau.com/whitelabs/yeast-bank-types/zinfandel
beertype:zinfandel rdf:type owl:Class ;
                   rdfs:subClassOf bevon:Wine ;
                   dcterms:bibliographicCitation "http://www.whitelabs.com/category/yeast-bank-types/zinfandel" ;
                   rdfs:label "Zinfandel" ;
                   skos:prefLabel "Zinfandel" .


###  http://peterbrau.com/yeast/BrewersYeast
yeast:BrewersYeast rdf:type owl:Class ;
                   rdfs:subClassOf owl:Thing ;
                   dcterms:bibliographicCitation "https://en.wikipedia.org/wiki/Yeast#Beer" ;
                   rdfs:label "Brewer's Yeast" ;
                   skos:altLabel "Ale Yeast" ,
                                 "Lager Yeast" ,
                                 "S. cerevisiae" ,
                                 "S. pastorianus" ,
                                 "Saccharomyces" ,
                                 "Saccharomyces cerevisiae" ,
                                 "Saccharomyces pastorianus" ,
                                 "Yeast" ,
                                 "Ale Yeast" ,
                                 "Lager Yeast" ,
                                 "cerevisiae" ,
                                 "pastorianus" ;
                   skos:definition "Brewing yeasts may be classed as \"top-cropping\" (or \"top-fermenting\") and \"bottom-cropping\" (or \"bottom-fermenting\"). Top-cropping yeasts are so called because they form a foam at the top of the wort during fermentation. An example of a top-cropping yeast is Saccharomyces cerevisiae, sometimes called an \"ale yeast\". Bottom-cropping yeasts are typically used to produce lager-type beers, though they can also produce ale-type beers. These yeasts ferment well at low temperatures. An example of bottom-cropping yeast is Saccharomyces pastorianus, formerly known as S. carlsbergensis." ;
                   skos:prefLabel "Brewer's Yeast" .


###  http://peterbrau.com/yeast/Cider
yeast:Cider rdf:type owl:Class ;
            rdfs:subClassOf bevon:FermentedBeverage ;
            rdfs:label "Cider" ;
            skos:prefLabel "Cider" .


###  http://peterbrau.com/yeast/Kombucha
yeast:Kombucha rdf:type owl:Class ;
               rdfs:subClassOf bevon:FermentedBeverage ;
               rdfs:label "Kombucha" ;
               skos:prefLabel "Kombucha" .


###  http://peterbrau.com/yeast/Mead
yeast:Mead rdf:type owl:Class ;
           rdfs:subClassOf bevon:FermentedBeverage ;
           rdfs:label "Mead" ;
           skos:prefLabel "Mead" .


###  http://peterbrau.com/yeast/Perry
yeast:Perry rdf:type owl:Class ;
            rdfs:subClassOf bevon:FermentedBeverage ;
            rdfs:label "Perry" ;
            skos:prefLabel "Perry" .


###  http://peterbrau.com/yeast/WildYeastAndBacteria
yeast:WildYeastAndBacteria rdf:type owl:Class ;
                           rdfs:subClassOf yeast:BrewersYeast ;
                           dcterms:bibliographicCitation "http://www.whitelabs.com/category/yeast-bank-types/wild-yeast-bacteria" ,
                                                         "https://en.wikipedia.org/wiki/Brettanomyces" ,
                                                         "https://en.wikipedia.org/wiki/Lactobacillus" ,
                                                         "https://en.wikipedia.org/wiki/Pediococcus" ,
                                                         "https://www.merriam-webster.com/dictionary/wild%20yeast" ;
                           rdfs:label "Wild Yeast & Bacteria" ;
                           skos:altLabel "B. anomalus" ,
                                         "B. bruxellensis" ,
                                         "B. claussenii" ,
                                         "B. custersianus" ,
                                         "B. naardenensis" ,
                                         "B. nanus" ,
                                         "Brettanomyces" ,
                                         "Brettanomyces anomalus" ,
                                         "Brettanomyces bruxellensis" ,
                                         "Brettanomyces claussenii" ,
                                         "Brettanomyces custersianus" ,
                                         "Brettanomyces naardenensis" ,
                                         "Brettanomyces nanus" ,
                                         "Debaryomyces" ,
                                         "Dekkera" ,
                                         "L. brevis" ,
                                         "L. casei" ,
                                         "Lactobacillus" ,
                                         "Lactobacillus brevis" ,
                                         "Lactobacillus casei" ,
                                         "P. damnosus" ,
                                         "Pediococcus" ,
                                         "Pediococcus damnosus" ,
                                         "anomalus" ,
                                         "brevis" ,
                                         "bruxellensis" ,
                                         "casei" ,
                                         "claussenii" ,
                                         "custersianus" ,
                                         "damnosus" ,
                                         "naardenensis" ,
                                         "nanus" ;
                           skos:prefLabel "Wild Yeast & Bacteria" ;
                           skos:definition "Any of various yeasts occurring naturally in the air or on surfaces especially of fruits as distinguished from those selected and artificially cultured (as for use in brewing or baking)" .


###  http://rdfs.co/bevon/Beer
bevon:Beer rdf:type owl:Class .


###  http://rdfs.co/bevon/BourbonWhiskey
bevon:BourbonWhiskey rdf:type owl:Class .


###  http://rdfs.co/bevon/Brandy
bevon:Brandy rdf:type owl:Class .


###  http://rdfs.co/bevon/Container
bevon:Container rdf:type owl:Class .


###  http://rdfs.co/bevon/Dunkel

###  http://rdfs.co/bevon/FermentedBeverage
bevon:FermentedBeverage rdf:type owl:Class .


###  http://rdfs.co/bevon/Gin
bevon:Gin rdf:type owl:Class .


###  http://rdfs.co/bevon/IrishRedAle

###  http://rdfs.co/bevon/Lager

###  http://rdfs.co/bevon/Pilsner

###  http://rdfs.co/bevon/Rum
bevon:Rum rdf:type owl:Class .


###  http://rdfs.co/bevon/Sake
bevon:Sake rdf:type owl:Class .


###  http://rdfs.co/bevon/ScotchWhisky
bevon:ScotchWhisky rdf:type owl:Class .


###  http://rdfs.co/bevon/Tequila
bevon:Tequila rdf:type owl:Class .


###  http://rdfs.co/bevon/Vodka
bevon:Vodka rdf:type owl:Class .


###  http://rdfs.co/bevon/Whisky
bevon:Whisky rdf:type owl:Class .


###  http://rdfs.co/bevon/Wine
bevon:Wine rdf:type owl:Class .


#################################################################
#    Individuals
#################################################################

###  http://peterbrau.com/whitelabs/yeast-bank/pinnacle-distillers-yeast-g-wldpinnacle-g-500g
wlp:pinnacle-distillers-yeast-g-wldpinnacle-g-500g rdf:type owl:NamedIndividual ,
                                                            yeast:BrewersYeast ;
                                                   yeast:hasAlcoholTolerance "High (10 - 15%)" ;
                                                   yeast:hasHighOptimumFermentationTemperature 98.00 ;
                                                   yeast:hasLowOptimumFermentationTemperature 92.00 ;
                                                   yeast:usedForBrewingStyle beertype:bourbon-whiskey ,
                                                                             beertype:gin ,
                                                                             beertype:rum ,
                                                                             beertype:rye-whiskey ,
                                                                             beertype:scotch-whisky ,
                                                                             beertype:tequila ,
                                                                             beertype:vodka ;
                                                   dcterms:bibliographicCitation "http://www.whitelabs.com/yeast-bank/pinnacle-distillers-yeast-g-wldpinnacle-g-500g" ;
                                                   rdfs:label "Pinnacle Distillers Yeast (G) - WLDPINNACLE G 500G" ;
                                                   skos:definition "An active dried yeast well-suited for use in simultaneous saccharification fermentation of starch substrates from grain. It has a high tolerance to liberated glucose." ;
                                                   skos:prefLabel "Pinnacle Distillers Yeast (G) - WLDPINNACLE G 500G" .


###  http://peterbrau.com/whitelabs/yeast-bank/pinnacle-distillers-yeast-m-wldpinnacle-m-500g
wlp:pinnacle-distillers-yeast-m-wldpinnacle-m-500g rdf:type owl:NamedIndividual ,
                                                            yeast:BrewersYeast ;
                                                   yeast:hasHighOptimumFermentationTemperature 90.00 ;
                                                   yeast:hasLowOptimumFermentationTemperature 82.00 ;
                                                   yeast:usedForBrewingStyle beertype:bourbon-whiskey ,
                                                                             beertype:rye-whiskey ,
                                                                             beertype:scotch-whisky ;
                                                   dcterms:bibliographicCitation "http://www.whitelabs.com/yeast-bank/pinnacle-distillers-yeast-m-wldpinnacle-m-500g" ;
                                                   rdfs:label "Pinnacle Distillers Yeast (M) - WLDPINNACLE M 500G" ;
                                                   skos:definition "An active dried yeast well-suited for use in malt-based fermentations. It rapidly consumes maltose and produces a flavorful spirit." ;
                                                   skos:prefLabel "Pinnacle Distillers Yeast (M) - WLDPINNACLE M 500G" .


###  http://peterbrau.com/whitelabs/yeast-bank/pinnacle-distillers-yeast-mg-wldpinnacle-mg-500g
wlp:pinnacle-distillers-yeast-mg-wldpinnacle-mg-500g rdf:type owl:NamedIndividual ,
                                                              yeast:BrewersYeast ;
                                                     yeast:hasAlcoholTolerance "High (10 - 15%)" ;
                                                     yeast:hasHighOptimumFermentationTemperature 100.00 ;
                                                     yeast:hasLowOptimumFermentationTemperature 82.00 ;
                                                     yeast:usedForBrewingStyle beertype:bourbon-whiskey ,
                                                                               beertype:brandy ,
                                                                               beertype:gin ,
                                                                               beertype:grappa ,
                                                                               beertype:rum ,
                                                                               beertype:rye-whiskey ,
                                                                               beertype:scotch-whisky ,
                                                                               beertype:tequila ,
                                                                               beertype:vodka ;
                                                     dcterms:bibliographicCitation "http://www.whitelabs.com/yeast-bank/pinnacle-distillers-yeast-mg-wldpinnacle-mg-500g" ;
                                                     rdfs:label "Pinnacle Distillers Yeast (MG+) - WLDPINNACLE MG+ 500G" ;
                                                     skos:definition "An active dried yeast well-suited for use in both malt and grain fermentations. It has the collective capability to tolerate high gravity and temperature." ;
                                                     skos:prefLabel "Pinnacle Distillers Yeast (MG+) - WLDPINNACLE MG+ 500G" .


###  http://peterbrau.com/whitelabs/yeast-bank/pinnacle-distillers-yeast-s-wldpinnacle-s
wlp:pinnacle-distillers-yeast-s-wldpinnacle-s rdf:type owl:NamedIndividual ,
                                                       yeast:BrewersYeast ;
                                              yeast:hasAlcoholTolerance "Very High (Over 15%)" ;
                                              yeast:hasHighOptimumFermentationTemperature 98.00 ;
                                              yeast:hasLowOptimumFermentationTemperature 92.00 ;
                                              yeast:usedForBrewingStyle beertype:rum ;
                                              dcterms:bibliographicCitation "http://www.whitelabs.com/yeast-bank/pinnacle-distillers-yeast-s-wldpinnacle-s" ;
                                              rdfs:label "Pinnacle Distillers Yeast (S) - WLDPINNACLE S" ;
                                              skos:definition "An active dry yeast well-suited for use in batch and continuous fermentations of molasses and pure sugars. It has a high tolerance to early residual sugars." ;
                                              skos:prefLabel "Pinnacle Distillers Yeast (S) - WLDPINNACLE S" .


###  http://peterbrau.com/whitelabs/yeast-bank/rum-turbo-wldrumag-1kg
wlp:rum-turbo-wldrumag-1kg rdf:type owl:NamedIndividual ,
                                    yeast:BrewersYeast ;
                           yeast:usedForBrewingStyle beertype:rum ;
                           dcterms:bibliographicCitation "http://www.whitelabs.com/yeast-bank/rum-turbo-wldrumag-1kg" ;
                           rdfs:label "Rum Turbo - WLDRUMAG-1KG" ;
                           skos:definition "An osmophilic Saccharomyces cerevisiae strain that is especially suited to 50:50 blend of molasses and sucrose fermentations up to 15% ABV, and produces full, rich, and fruity aromatics. It contains complete nutrition for rapid fermentation, including amyloglucosidase for breaking longer sugar chains and optimum yield. Size: 1kg." ;
                           skos:prefLabel "Rum Turbo - WLDRUMAG-1KG" .


###  http://peterbrau.com/whitelabs/yeast-bank/ty-48-high-performance-yeast-wldty48-1kg
wlp:ty-48-high-performance-yeast-wldty48-1kg rdf:type owl:NamedIndividual ,
                                                      yeast:BrewersYeast ;
                                             yeast:hasAlcoholTolerance "N/A" ;
                                             yeast:usedForBrewingStyle beertype:gin ,
                                                                       beertype:rum ,
                                                                       beertype:tequila ,
                                                                       beertype:vodka ;
                                             dcterms:bibliographicCitation "http://www.whitelabs.com/yeast-bank/ty-48-high-performance-yeast-wldty48-1kg" ;
                                             rdfs:label "TY 48 High Performance Yeast - WLDTY48-1KG" ;
                                             skos:definition "High-performance temperature and ethanol tolerant yeast capable of reaching 20% ABV from pure sugar wash in 8 days. With AG enzyme to allow starch-based feedstock after normal gelatination and alpha-amylase treatment. " ;
                                             skos:prefLabel "TY 48 High Performance Yeast - WLDTY48-1KG" .


###  http://peterbrau.com/whitelabs/yeast-bank/vodka-turbo-wldvodkaag-1kg
wlp:vodka-turbo-wldvodkaag-1kg rdf:type owl:NamedIndividual ,
                                        yeast:BrewersYeast ;
                               yeast:hasAlcoholTolerance "N/A" ;
                               yeast:usedForBrewingStyle beertype:gin ,
                                                         beertype:vodka ;
                               dcterms:bibliographicCitation "http://www.whitelabs.com/yeast-bank/vodka-turbo-wldvodkaag-1kg" ;
                               rdfs:label "Vodka Turbo - WLDVODKAAG-1KG" ;
                               skos:definition "High yield vodka strain with extraordinarily low metabolite production ideal for use with sugar, grain or potato feedstock in vodka production. Provides complete nutrition for easy fermentation of low-nutrition washes together with amyloglucosidase enzyme for dextrins conversion." ;
                               skos:prefLabel "Vodka Turbo - WLDVODKAAG-1KG" .


###  http://peterbrau.com/whitelabs/yeast-bank/whiskey-turbo-wldwhiskeyag-1kg
wlp:whiskey-turbo-wldwhiskeyag-1kg rdf:type owl:NamedIndividual ,
                                            yeast:BrewersYeast ;
                                   yeast:hasAlcoholTolerance "N/A" ;
                                   yeast:usedForBrewingStyle beertype:bourbon-whiskey ,
                                                             beertype:rye-whiskey ;
                                   dcterms:bibliographicCitation "http://www.whitelabs.com/yeast-bank/whiskey-turbo-wldwhiskeyag-1kg" ;
                                   rdfs:label "Whiskey Turbo - WLDWHISKEYAG-1KG " ;
                                   skos:definition "None" ;
                                   skos:prefLabel "Whiskey Turbo - WLDWHISKEYAG-1KG " .


###  http://peterbrau.com/whitelabs/yeast-bank/wldrumag-1kg-rum-turbo-ag-1kg-distillers-yeast
wlp:wldrumag-1kg-rum-turbo-ag-1kg-distillers-yeast rdf:type owl:NamedIndividual ,
                                                            yeast:BrewersYeast ;
                                                   dcterms:bibliographicCitation "http://www.whitelabs.com/yeast-bank/wldrumag-1kg-rum-turbo-ag-1kg-distillers-yeast" ;
                                                   rdfs:label "WLDRUMAG-1KG Rum Turbo AG-1kg (Distillers Yeast)" ;
                                                   skos:prefLabel "WLDRUMAG-1KG Rum Turbo AG-1kg (Distillers Yeast)" .


###  http://peterbrau.com/whitelabs/yeast-bank/wlp001-california-ale-yeast
wlp:wlp001-california-ale-yeast rdf:type owl:NamedIndividual ,
                                         yeast:BrewersYeast ;
                                yeast:hasAlcoholTolerance "High (10 - 15%)" ;
                                yeast:hasFlocculation "Medium" ;
                                yeast:hasHighAttenuation 80.00 ;
                                yeast:hasHighOptimumFermentationTemperature 73.00 ;
                                yeast:hasLowAttenuation 73.00 ;
                                yeast:hasLowOptimumFermentationTemperature 68.00 ;
                                yeast:usedForBrewingStyle beertype:american-amber ,
                                                          beertype:american-brown-ale ,
                                                          beertype:american-india-pale-ale ,
                                                          beertype:american-pale-ale ,
                                                          beertype:american-porter ,
                                                          beertype:apple-wine ,
                                                          beertype:barleywine-ale ,
                                                          beertype:bourbon-whiskey ,
                                                          beertype:common-perry ,
                                                          beertype:cream-ale ,
                                                          beertype:dusseldorf-altbier ,
                                                          beertype:english-brown-ale ,
                                                          beertype:english-cider ,
                                                          beertype:english-old-ale ,
                                                          beertype:english-pale-ale ,
                                                          beertype:extra-special-bitter ,
                                                          beertype:foreign-export-stout ,
                                                          beertype:french-cider ,
                                                          beertype:gin ,
                                                          beertype:imperial-india-pale-ale ,
                                                          beertype:imperial-stout ,
                                                          beertype:irish-dry-stout ,
                                                          beertype:irish-red-ale ,
                                                          beertype:kolsch ,
                                                          beertype:oatmeal-stout ,
                                                          beertype:ordinary-bitter ,
                                                          beertype:rye-whiskey ,
                                                          beertype:scotch-ale-wee-heavy ,
                                                          beertype:sweet-cider ,
                                                          beertype:tequila ,
                                                          beertype:traditional-perry ,
                                                          beertype:vodka ,
                                                          beertype:wheat-ale ;
                                dcterms:bibliographicCitation "http://www.whitelabs.com/yeast-bank/wlp001-california-ale-yeast" ;
                                gr:hasMPN "wlp001" ;
                                rdfs:label "WLP001 California Ale Yeast" ;
                                skos:definition "This strain was the first yeast strain produced by White Labs in 1995. It’s our best-selling yeast, famous for its clean flavors and hardy fermentations. Known for its use in hoppy beers, it accentuates hop flavors and aromas and attenuates well, even for high gravity beers. This strain has the ability to be used in almost any style of ale ranging from IPA to porter and even kölsch, which makes it a great all-around house strain. " ;
                                skos:prefLabel "WLP001 California Ale Yeast" .


###  http://peterbrau.com/whitelabs/yeast-bank/wlp002-english-ale-yeast
wlp:wlp002-english-ale-yeast rdf:type owl:NamedIndividual ,
                                      yeast:BrewersYeast ;
                             yeast:hasAlcoholTolerance "Medium (5 - 10%)" ;
                             yeast:hasFlocculation "Very High" ;
                             yeast:hasHighAttenuation 70.00 ;
                             yeast:hasHighOptimumFermentationTemperature 68.00 ;
                             yeast:hasLowAttenuation 63.00 ;
                             yeast:hasLowOptimumFermentationTemperature 65.00 ;
                             yeast:usedForBrewingStyle beertype:american-amber ,
                                                       beertype:american-brown-ale ,
                                                       beertype:american-india-pale-ale ,
                                                       beertype:american-pale-ale ,
                                                       beertype:american-porter ,
                                                       beertype:apple-wine ,
                                                       beertype:barleywine-ale ,
                                                       beertype:common-perry ,
                                                       beertype:cream-ale ,
                                                       beertype:dusseldorf-altbier ,
                                                       beertype:english-brown-ale ,
                                                       beertype:english-cider ,
                                                       beertype:english-india-pale-ale ,
                                                       beertype:english-old-ale ,
                                                       beertype:english-pale-ale ,
                                                       beertype:extra-special-bitter ,
                                                       beertype:foreign-export-stout ,
                                                       beertype:french-cider ,
                                                       beertype:imperial-india-pale-ale ,
                                                       beertype:imperial-stout ,
                                                       beertype:irish-dry-stout ,
                                                       beertype:irish-red-ale ,
                                                       beertype:kolsch ,
                                                       beertype:oatmeal-stout ,
                                                       beertype:ordinary-bitter ,
                                                       beertype:scotch-ale-wee-heavy ,
                                                       beertype:sweet-stout ,
                                                       beertype:wheat-ale ;
                             dcterms:bibliographicCitation "http://www.whitelabs.com/yeast-bank/wlp002-english-ale-yeast" ;
                             gr:hasMPN "wlp002" ;
                             rdfs:label "WLP002 English Ale Yeast" ;
                             skos:definition "This is a classic ESB strain from one of England’s largest independent breweries. While it is traditionally used for English-style ales including milds, bitters, porters, and stouts, it is also ideal for American-style pale ales and IPAs. Residual sweetness accentuates malt character along with mild fruity esters, adding complexity to the flavor and aroma of finished beers. Slight diacetyl production is common. Due to this strain’s high flocculation, the beer will finish clear and the yeast can easily be harvested from the fermenter for future use. It is common for this yeast to look coagulated." ;
                             skos:prefLabel "WLP002 English Ale Yeast" .


###  http://peterbrau.com/whitelabs/yeast-bank/wlp003-german-ale-ii-yeast
wlp:wlp003-german-ale-ii-yeast rdf:type owl:NamedIndividual ,
                                        yeast:BrewersYeast ;
                               yeast:hasAlcoholTolerance "Medium (5 - 10%)" ;
                               yeast:hasFlocculation "Medium" ;
                               yeast:hasHighAttenuation 80.00 ;
                               yeast:hasHighOptimumFermentationTemperature 70.00 ;
                               yeast:hasLowAttenuation 73.00 ;
                               yeast:hasLowOptimumFermentationTemperature 65.00 ;
                               yeast:usedForBrewingStyle beertype:blonde-ale ,
                                                         beertype:dusseldorf-altbier ,
                                                         beertype:kolsch ;
                               dcterms:bibliographicCitation "http://www.whitelabs.com/yeast-bank/wlp003-german-ale-ii-yeast" ;
                               gr:hasMPN "wlp003" ;
                               rdfs:label "WLP003 German Ale II Yeast " ;
                               skos:definition "A great strain for clean ales such as kölsch, altbier, and German-style pale ales. It has a strong sulfur component that will reduce with conditioning. Lager-like in flavor, this strain ferments clean and produces subdued fruity esters which are more present than WLP029 German/Kölsch Ale Yeast." ;
                               skos:prefLabel "WLP003 German Ale II Yeast " .


###  http://peterbrau.com/whitelabs/yeast-bank/wlp004-irish-ale-yeast
wlp:wlp004-irish-ale-yeast rdf:type owl:NamedIndividual ,
                                    yeast:BrewersYeast ;
                           yeast:hasAlcoholTolerance "Medium - High (8 - 12%)" ;
                           yeast:hasFlocculation "Medium to High" ;
                           yeast:hasHighAttenuation 74.00 ;
                           yeast:hasHighOptimumFermentationTemperature 68.00 ;
                           yeast:hasLowAttenuation 69.00 ;
                           yeast:hasLowOptimumFermentationTemperature 65.00 ;
                           yeast:usedForBrewingStyle beertype:american-amber ,
                                                     beertype:american-brown-ale ,
                                                     beertype:american-india-pale-ale ,
                                                     beertype:american-pale-ale ,
                                                     beertype:american-porter ,
                                                     beertype:barleywine-ale ,
                                                     beertype:cream-ale ,
                                                     beertype:english-brown-ale ,
                                                     beertype:english-india-pale-ale ,
                                                     beertype:english-old-ale ,
                                                     beertype:english-pale-ale ,
                                                     beertype:extra-special-bitter ,
                                                     beertype:foreign-export-stout ,
                                                     beertype:imperial-india-pale-ale ,
                                                     beertype:imperial-stout ,
                                                     beertype:irish-dry-stout ,
                                                     beertype:irish-red-ale ,
                                                     beertype:kolsch ,
                                                     beertype:oatmeal-stout ,
                                                     beertype:ordinary-bitter ,
                                                     beertype:scotch-ale-wee-heavy ,
                                                     beertype:sweet-stout ,
                                                     beertype:wheat-ale ;
                           dcterms:bibliographicCitation "http://www.whitelabs.com/yeast-bank/wlp004-irish-ale-yeast" ;
                           gr:hasMPN "wlp004" ;
                           rdfs:label "WLP004 Irish Ale Yeast" ;
                           skos:definition "This yeast is from one of the oldest stout-producing breweries in the world. It’s great for many beer styles but really shines in malty British styles such as stouts, porters and brown ales. Medium attenuation helps with a dry finish that promotes roasty notes. Esters help round out the overall flavor making a soft drinkable stout." ;
                           skos:prefLabel "WLP004 Irish Ale Yeast" .


###  http://peterbrau.com/whitelabs/yeast-bank/wlp005-british-ale-yeast
wlp:wlp005-british-ale-yeast rdf:type owl:NamedIndividual ,
                                      yeast:BrewersYeast ;
                             yeast:hasAlcoholTolerance "Medium (5 - 10%)" ;
                             yeast:hasFlocculation "High" ;
                             yeast:hasHighAttenuation 74.00 ;
                             yeast:hasHighOptimumFermentationTemperature 70.00 ;
                             yeast:hasLowAttenuation 67.00 ;
                             yeast:hasLowOptimumFermentationTemperature 65.00 ;
                             yeast:usedForBrewingStyle beertype:american-amber ,
                                                       beertype:american-brown-ale ,
                                                       beertype:american-india-pale-ale ,
                                                       beertype:american-pale-ale ,
                                                       beertype:american-porter ,
                                                       beertype:barleywine-ale ,
                                                       beertype:cream-ale ,
                                                       beertype:english-brown-ale ,
                                                       beertype:english-india-pale-ale ,
                                                       beertype:english-old-ale ,
                                                       beertype:english-pale-ale ,
                                                       beertype:extra-special-bitter ,
                                                       beertype:foreign-export-stout ,
                                                       beertype:imperial-stout ,
                                                       beertype:irish-dry-stout ,
                                                       beertype:irish-red-ale ,
                                                       beertype:kolsch ,
                                                       beertype:oatmeal-stout ,
                                                       beertype:ordinary-bitter ,
                                                       beertype:scotch-ale-wee-heavy ,
                                                       beertype:sweet-stout ,
                                                       beertype:wheat-ale ;
                             dcterms:bibliographicCitation "http://www.whitelabs.com/yeast-bank/wlp005-british-ale-yeast" ;
                             gr:hasMPN "wlp005" ;
                             rdfs:label "WLP005 British Ale Yeast" ;
                             skos:definition "Known for its use in malty English beers, this strain is a great choice for any beers using traditional English malts like Marris Otter, Golden Promise or floor malted barley. This strain will push bready, grainy malt flavors while being a mild ester producer." ;
                             skos:prefLabel "WLP005 British Ale Yeast" .


###  http://peterbrau.com/whitelabs/yeast-bank/wlp006-bedford-british-ale-yeast
wlp:wlp006-bedford-british-ale-yeast rdf:type owl:NamedIndividual ,
                                              yeast:BrewersYeast ;
                                     yeast:hasAlcoholTolerance "Medium (5 - 10%)" ;
                                     yeast:hasFlocculation "High" ;
                                     yeast:hasHighAttenuation 80.00 ;
                                     yeast:hasHighOptimumFermentationTemperature 70.00 ;
                                     yeast:hasLowAttenuation 72.00 ;
                                     yeast:hasLowOptimumFermentationTemperature 65.00 ;
                                     yeast:usedForBrewingStyle beertype:american-brown-ale ,
                                                               beertype:american-porter ,
                                                               beertype:english-brown-ale ,
                                                               beertype:english-india-pale-ale ,
                                                               beertype:english-old-ale ,
                                                               beertype:english-pale-ale ,
                                                               beertype:extra-special-bitter ,
                                                               beertype:imperial-india-pale-ale ,
                                                               beertype:irish-red-ale ,
                                                               beertype:scotch-ale-wee-heavy ;
                                     dcterms:bibliographicCitation "http://www.whitelabs.com/yeast-bank/wlp006-bedford-british-ale-yeast" ;
                                     gr:hasMPN "wlp006" ;
                                     rdfs:label "WLP006 Bedford British Ale Yeast" ;
                                     skos:definition "Ferments dry and flocculates very well; produces a distinct ester profile. This yeast yields a full mouthfeel, perfect for creating English-style ales, including bitters, pale ales, porters, stouts and browns." ;
                                     skos:prefLabel "WLP006 Bedford British Ale Yeast" .


###  http://peterbrau.com/whitelabs/yeast-bank/wlp007-dry-english-ale-yeast
wlp:wlp007-dry-english-ale-yeast rdf:type owl:NamedIndividual ,
                                          yeast:BrewersYeast ;
                                 yeast:hasAlcoholTolerance "Medium - High (8 - 12%)" ;
                                 yeast:hasFlocculation "Medium to High" ;
                                 yeast:hasHighAttenuation 80.00 ;
                                 yeast:hasHighOptimumFermentationTemperature 70.00 ;
                                 yeast:hasLowAttenuation 70.00 ;
                                 yeast:hasLowOptimumFermentationTemperature 65.00 ;
                                 yeast:usedForBrewingStyle beertype:american-amber ,
                                                           beertype:american-brown-ale ,
                                                           beertype:american-india-pale-ale ,
                                                           beertype:american-pale-ale ,
                                                           beertype:american-porter ,
                                                           beertype:barleywine-ale ,
                                                           beertype:cream-ale ,
                                                           beertype:english-brown-ale ,
                                                           beertype:english-india-pale-ale ,
                                                           beertype:english-old-ale ,
                                                           beertype:english-pale-ale ,
                                                           beertype:extra-special-bitter ,
                                                           beertype:foreign-export-stout ,
                                                           beertype:imperial-india-pale-ale ,
                                                           beertype:imperial-stout ,
                                                           beertype:irish-dry-stout ,
                                                           beertype:irish-red-ale ,
                                                           beertype:kolsch ,
                                                           beertype:oatmeal-stout ,
                                                           beertype:ordinary-bitter ,
                                                           beertype:scotch-ale-wee-heavy ,
                                                           beertype:sweet-stout ,
                                                           beertype:wheat-ale ;
                                 dcterms:bibliographicCitation "http://www.whitelabs.com/yeast-bank/wlp007-dry-english-ale-yeast" ;
                                 gr:hasMPN "wlp007" ;
                                 rdfs:label "WLP007 Dry English Ale Yeast" ;
                                 skos:definition "This yeast is known for its high attenuation, achieving 80% even with 10% ABV beers. The high attenuation eliminates residual sweetness, making the yeast well-suited for high gravity ales and clean, well-attenuated beer styles. This strain has become a go-to house strain for American breweries due to its clean profile and high attenuation. It’s an ideal strain for American and English hoppy beers as well as malty ambers, porters and brown ales. This strain can be a substitute for WLP001 California Ale Yeast®." ;
                                 skos:prefLabel "WLP007 Dry English Ale Yeast" .


###  http://peterbrau.com/whitelabs/yeast-bank/wlp008-east-coast-ale-yeast
wlp:wlp008-east-coast-ale-yeast rdf:type owl:NamedIndividual ,
                                         yeast:BrewersYeast ;
                                yeast:hasAlcoholTolerance "Medium (5 - 10%)" ;
                                yeast:hasFlocculation "Medium to Low" ;
                                yeast:hasHighAttenuation 75.00 ;
                                yeast:hasHighOptimumFermentationTemperature 73.00 ;
                                yeast:hasLowAttenuation 70.00 ;
                                yeast:hasLowOptimumFermentationTemperature 68.00 ;
                                yeast:usedForBrewingStyle beertype:american-amber ,
                                                          beertype:american-brown-ale ,
                                                          beertype:american-india-pale-ale ,
                                                          beertype:american-pale-ale ,
                                                          beertype:american-porter ,
                                                          beertype:barleywine-ale ,
                                                          beertype:cream-ale ,
                                                          beertype:dusseldorf-altbier ,
                                                          beertype:english-brown-ale ,
                                                          beertype:english-india-pale-ale ,
                                                          beertype:english-old-ale ,
                                                          beertype:english-pale-ale ,
                                                          beertype:extra-special-bitter ,
                                                          beertype:foreign-export-stout ,
                                                          beertype:hazy-ipa-pale-ale ,
                                                          beertype:imperial-india-pale-ale ,
                                                          beertype:imperial-stout ,
                                                          beertype:irish-dry-stout ,
                                                          beertype:irish-red-ale ,
                                                          beertype:kolsch ,
                                                          beertype:oatmeal-stout ,
                                                          beertype:ordinary-bitter ,
                                                          beertype:scotch-ale-wee-heavy ,
                                                          beertype:sweet-stout ,
                                                          beertype:wheat-ale ;
                                dcterms:bibliographicCitation "http://www.whitelabs.com/yeast-bank/wlp008-east-coast-ale-yeast" ;
                                gr:hasMPN "wlp008" ;
                                rdfs:label "WLP008 East Coast Ale Yeast" ;
                                skos:definition "This strain can be used to reproduce many American versions of classic beer styles but has been gaining popularity for its use in East Coast IPAs. It is cleaner and crisper than other haze producing strains. It possesses the similar neutral character of WLP001 California Ale Yeast® with slightly higher ester production. This strain’s attenuation leaves some mouthfeel and residual sweetness which balances hop bitterness. It’s a great all-around strain for balanced, accessible beer styles such as blondes, pale ales and amber ales." ;
                                skos:prefLabel "WLP008 East Coast Ale Yeast" .


###  http://peterbrau.com/whitelabs/yeast-bank/wlp009-australian-ale-yeast
wlp:wlp009-australian-ale-yeast rdf:type owl:NamedIndividual ,
                                         yeast:BrewersYeast ;
                                yeast:hasAlcoholTolerance "Medium (5 - 10%)" ;
                                yeast:hasFlocculation "High" ;
                                yeast:hasHighAttenuation 75.00 ;
                                yeast:hasHighOptimumFermentationTemperature 70.00 ;
                                yeast:hasLowAttenuation 70.00 ;
                                yeast:hasLowOptimumFermentationTemperature 65.00 ;
                                yeast:usedForBrewingStyle beertype:american-amber ,
                                                          beertype:american-india-pale-ale ,
                                                          beertype:american-pale-ale ,
                                                          beertype:cream-ale ,
                                                          beertype:english-india-pale-ale ,
                                                          beertype:imperial-india-pale-ale ,
                                                          beertype:kolsch ,
                                                          beertype:ordinary-bitter ;
                                dcterms:bibliographicCitation "http://www.whitelabs.com/yeast-bank/wlp009-australian-ale-yeast" ;
                                gr:hasMPN "wlp009" ;
                                rdfs:label "WLP009 Australian Ale Yeast" ;
                                skos:definition "This yeast produces a clean, malty beer with pleasant ester characters that can be described as “bready.” It ferments successfully and cleanly at higher temperatures, combined with good flocculation and good attenuation." ;
                                skos:prefLabel "WLP009 Australian Ale Yeast" .


###  http://peterbrau.com/whitelabs/yeast-bank/wlp011-european-ale-yeast
wlp:wlp011-european-ale-yeast rdf:type owl:NamedIndividual ,
                                       yeast:BrewersYeast ;
                              yeast:hasAlcoholTolerance "Medium (5 - 10%)" ;
                              yeast:hasFlocculation "Medium" ;
                              yeast:hasHighAttenuation 70.00 ;
                              yeast:hasHighOptimumFermentationTemperature 70.00 ;
                              yeast:hasLowAttenuation 65.00 ;
                              yeast:hasLowOptimumFermentationTemperature 65.00 ;
                              yeast:usedForBrewingStyle beertype:american-amber ,
                                                        beertype:american-brown-ale ,
                                                        beertype:american-india-pale-ale ,
                                                        beertype:american-pale-ale ,
                                                        beertype:american-porter ,
                                                        beertype:barleywine-ale ,
                                                        beertype:cream-ale ,
                                                        beertype:dusseldorf-altbier ,
                                                        beertype:english-brown-ale ,
                                                        beertype:english-india-pale-ale ,
                                                        beertype:english-old-ale ,
                                                        beertype:english-pale-ale ,
                                                        beertype:extra-special-bitter ,
                                                        beertype:foreign-export-stout ,
                                                        beertype:imperial-india-pale-ale ,
                                                        beertype:imperial-stout ,
                                                        beertype:irish-dry-stout ,
                                                        beertype:irish-red-ale ,
                                                        beertype:kolsch ,
                                                        beertype:oatmeal-stout ,
                                                        beertype:ordinary-bitter ,
                                                        beertype:scotch-ale-wee-heavy ,
                                                        beertype:sweet-stout ,
                                                        beertype:wheat-ale ;
                              dcterms:bibliographicCitation "http://www.whitelabs.com/yeast-bank/wlp011-european-ale-yeast" ;
                              gr:hasMPN "wlp011" ;
                              rdfs:label "WLP011 European Ale Yeast " ;
                              skos:definition "A malty northern European-origin ale yeast. Its low ester production gives it a clean profile, with little to no sulfur production. Low attenuation helps to contribute to the malty character. Good for altbiers, kölsch-style ales, malty English-style ales, and fruit beers." ;
                              skos:prefLabel "WLP011 European Ale Yeast " .


###  http://peterbrau.com/whitelabs/yeast-bank/wlp013-london-ale-yeast
wlp:wlp013-london-ale-yeast rdf:type owl:NamedIndividual ,
                                     yeast:BrewersYeast ;
                            yeast:hasAlcoholTolerance "Medium (5 - 10%)" ;
                            yeast:hasFlocculation "Medium" ;
                            yeast:hasHighAttenuation 75.00 ;
                            yeast:hasHighOptimumFermentationTemperature 71.00 ;
                            yeast:hasLowAttenuation 67.00 ;
                            yeast:hasLowOptimumFermentationTemperature 66.00 ;
                            yeast:usedForBrewingStyle beertype:american-amber ,
                                                      beertype:american-brown-ale ,
                                                      beertype:american-india-pale-ale ,
                                                      beertype:american-pale-ale ,
                                                      beertype:american-porter ,
                                                      beertype:barleywine-ale ,
                                                      beertype:cream-ale ,
                                                      beertype:dusseldorf-altbier ,
                                                      beertype:english-brown-ale ,
                                                      beertype:english-india-pale-ale ,
                                                      beertype:english-old-ale ,
                                                      beertype:english-pale-ale ,
                                                      beertype:extra-special-bitter ,
                                                      beertype:foreign-export-stout ,
                                                      beertype:hazy-ipa-pale-ale ,
                                                      beertype:imperial-india-pale-ale ,
                                                      beertype:imperial-stout ,
                                                      beertype:irish-dry-stout ,
                                                      beertype:irish-red-ale ,
                                                      beertype:oatmeal-stout ,
                                                      beertype:ordinary-bitter ,
                                                      beertype:scotch-ale-wee-heavy ,
                                                      beertype:sweet-stout ,
                                                      beertype:wheat-ale ;
                            dcterms:bibliographicCitation "http://www.whitelabs.com/yeast-bank/wlp013-london-ale-yeast" ;
                            gr:hasMPN "wlp013" ;
                            rdfs:label "WLP013 London Ale Yeast" ;
                            skos:definition "Oak ester character makes this yeast well-suited for classic British beer styles such as pales and bitters, or dark malty beers like brown ales and porters. Medium flocculation characteristics allow attenuation up to 75% leaving beer dry while adding malt complexity and pushing hop bitterness. If you love WLP001 California Ale Yeast®, give this strain a try as it has more character." ;
                            skos:prefLabel "WLP013 London Ale Yeast" .


###  http://peterbrau.com/whitelabs/yeast-bank/wlp017-whitbread-ii-ale-yeast
wlp:wlp017-whitbread-ii-ale-yeast rdf:type owl:NamedIndividual ,
                                           yeast:BrewersYeast ;
                                  yeast:hasAlcoholTolerance "Medium (5 - 10%)" ;
                                  yeast:hasFlocculation "High" ;
                                  yeast:hasHighAttenuation 73.00 ;
                                  yeast:hasHighOptimumFermentationTemperature 70.00 ;
                                  yeast:hasLowAttenuation 67.00 ;
                                  yeast:hasLowOptimumFermentationTemperature 66.00 ;
                                  yeast:usedForBrewingStyle beertype:american-porter ,
                                                            beertype:english-brown-ale ,
                                                            beertype:english-pale-ale ,
                                                            beertype:imperial-stout ;
                                  dcterms:bibliographicCitation "http://www.whitelabs.com/yeast-bank/wlp017-whitbread-ii-ale-yeast" ;
                                  gr:hasMPN "wlp017" ;
                                  rdfs:label "WLP017 Whitbread II Ale Yeast" ;
                                  skos:definition "Traditional mixed yeast culture with British character. Slightly fruity with a hint of sulfur production. This yeast can be used for many different beer styles. The most traditional choices would be English-style ales, including milds, bitters, porters, and English-style stouts. North American-style ales will also benefit from fermentation with this strain." ;
                                  skos:prefLabel "WLP017 Whitbread II Ale Yeast" .


###  http://peterbrau.com/whitelabs/yeast-bank/wlp019-california-iv-ale-yeast
wlp:wlp019-california-iv-ale-yeast rdf:type owl:NamedIndividual ,
                                            yeast:BrewersYeast ;
                                   yeast:usedForBrewingStyle beertype:english-brown-ale ;
                                   dcterms:bibliographicCitation "http://www.whitelabs.com/yeast-bank/wlp019-california-iv-ale-yeast" ;
                                   gr:hasMPN "wlp019" ;
                                   rdfs:label "WLP019 California IV Ale Yeast" ;
                                   skos:definition "Moderately clean strain with a low ester profile and less sulfur production than WLP051." ;
                                   skos:prefLabel "WLP019 California IV Ale Yeast" .


###  http://peterbrau.com/whitelabs/yeast-bank/wlp022-essex-ale-yeast
wlp:wlp022-essex-ale-yeast rdf:type owl:NamedIndividual ,
                                    yeast:BrewersYeast ;
                           yeast:hasAlcoholTolerance "Medium (5 - 10%)" ;
                           yeast:hasFlocculation "Medium to High" ;
                           yeast:hasHighAttenuation 76.00 ;
                           yeast:hasHighOptimumFermentationTemperature 70.00 ;
                           yeast:hasLowAttenuation 71.00 ;
                           yeast:hasLowOptimumFermentationTemperature 66.00 ;
                           yeast:usedForBrewingStyle beertype:american-porter ,
                                                     beertype:english-brown-ale ,
                                                     beertype:english-pale-ale ,
                                                     beertype:extra-special-bitter ;
                           dcterms:bibliographicCitation "http://www.whitelabs.com/yeast-bank/wlp022-essex-ale-yeast" ;
                           gr:hasMPN "wlp022" ;
                           rdfs:label "WLP022 Essex Ale Yeast" ;
                           skos:definition "A flavorful British-style yeast that produces slightly fruity and bready characters. A good top-fermenting yeast strain that is well suited for top cropping. It is ideal for classic British-style milds, pale ales, bitters and stouts. Does not flocculate as much as other English strains." ;
                           skos:prefLabel "WLP022 Essex Ale Yeast" .


###  http://peterbrau.com/whitelabs/yeast-bank/wlp023-burton-ale-yeast
wlp:wlp023-burton-ale-yeast rdf:type owl:NamedIndividual ,
                                     yeast:BrewersYeast ;
                            yeast:hasAlcoholTolerance "Medium (5 - 10%)" ;
                            yeast:hasFlocculation "Medium" ;
                            yeast:hasHighAttenuation 75.00 ;
                            yeast:hasHighOptimumFermentationTemperature 73.00 ;
                            yeast:hasLowAttenuation 69.00 ;
                            yeast:hasLowOptimumFermentationTemperature 68.00 ;
                            yeast:usedForBrewingStyle beertype:american-amber ,
                                                      beertype:american-brown-ale ,
                                                      beertype:american-india-pale-ale ,
                                                      beertype:american-pale-ale ,
                                                      beertype:american-porter ,
                                                      beertype:barleywine-ale ,
                                                      beertype:cream-ale ,
                                                      beertype:dusseldorf-altbier ,
                                                      beertype:english-brown-ale ,
                                                      beertype:english-india-pale-ale ,
                                                      beertype:english-old-ale ,
                                                      beertype:english-pale-ale ,
                                                      beertype:extra-special-bitter ,
                                                      beertype:foreign-export-stout ,
                                                      beertype:imperial-india-pale-ale ,
                                                      beertype:imperial-stout ,
                                                      beertype:irish-dry-stout ,
                                                      beertype:irish-red-ale ,
                                                      beertype:oatmeal-stout ,
                                                      beertype:scotch-ale-wee-heavy ,
                                                      beertype:sweet-stout ,
                                                      beertype:wheat-ale ;
                            dcterms:bibliographicCitation "http://www.whitelabs.com/yeast-bank/wlp023-burton-ale-yeast" ;
                            gr:hasMPN "wlp023" ;
                            rdfs:label "WLP023 Burton Ale Yeast" ;
                            skos:definition "This strain is sourced from Burton upon Trent, England which is known for pushing IPAs into the spotlight. It produces a subtle fruity ester profile which can be described as notes of apple, clover honey and pear. A background sulfur note is common with this strain. Great for use in hoppy American and English styles such as pale ales, bitters and ambers. Can also be an alternative to WLP001 California Ale Yeast®." ;
                            skos:prefLabel "WLP023 Burton Ale Yeast" .


###  http://peterbrau.com/whitelabs/yeast-bank/wlp025-southwold-ale-yeast
wlp:wlp025-southwold-ale-yeast rdf:type owl:NamedIndividual ,
                                        yeast:BrewersYeast ;
                               yeast:hasAlcoholTolerance "Medium (5 - 10%)" ;
                               yeast:hasFlocculation "Medium" ;
                               yeast:hasHighAttenuation 75.00 ;
                               yeast:hasHighOptimumFermentationTemperature 69.00 ;
                               yeast:hasLowAttenuation 68.00 ;
                               yeast:hasLowOptimumFermentationTemperature 66.00 ;
                               yeast:usedForBrewingStyle beertype:english-pale-ale ,
                                                         beertype:extra-special-bitter ,
                                                         beertype:ordinary-bitter ;
                               dcterms:bibliographicCitation "http://www.whitelabs.com/yeast-bank/wlp025-southwold-ale-yeast" ;
                               gr:hasMPN "wlp025" ;
                               rdfs:label "WLP025 Southwold Ale Yeast" ;
                               skos:definition "From Suffolk County, England. This yeast produces complex fruit, citrus, and spice flavors. Great for British-style bitters and pale ales. A slight sulfur note is produced during fermentation, but disappears with aging." ;
                               skos:prefLabel "WLP025 Southwold Ale Yeast" .


###  http://peterbrau.com/whitelabs/yeast-bank/wlp026-premium-bitter-ale-yeast
wlp:wlp026-premium-bitter-ale-yeast rdf:type owl:NamedIndividual ,
                                             yeast:BrewersYeast ;
                                    yeast:hasAlcoholTolerance "Medium (5 - 10%)" ;
                                    yeast:hasFlocculation "Medium" ;
                                    yeast:hasHighAttenuation 75.00 ;
                                    yeast:hasHighOptimumFermentationTemperature 70.00 ;
                                    yeast:hasLowAttenuation 70.00 ;
                                    yeast:hasLowOptimumFermentationTemperature 67.00 ;
                                    yeast:usedForBrewingStyle beertype:american-porter ,
                                                              beertype:barleywine-ale ,
                                                              beertype:english-brown-ale ,
                                                              beertype:english-old-ale ,
                                                              beertype:english-pale-ale ,
                                                              beertype:extra-special-bitter ,
                                                              beertype:imperial-stout ,
                                                              beertype:ordinary-bitter ;
                                    dcterms:bibliographicCitation "http://www.whitelabs.com/yeast-bank/wlp026-premium-bitter-ale-yeast" ;
                                    gr:hasMPN "wlp026" ;
                                    rdfs:label "WLP026 Premium Bitter Ale Yeast" ;
                                    skos:definition "From Staffordshire, England. Fermentation gives a mild but complex estery character. Ferments strong and dry and is good for high-gravity beers. Best for all English-style ales, including bitters, milds, ESBs, porters, stouts and barleywines." ;
                                    skos:prefLabel "WLP026 Premium Bitter Ale Yeast" .


###  http://peterbrau.com/whitelabs/yeast-bank/wlp028-edinburgh-scottish-ale-yeast
wlp:wlp028-edinburgh-scottish-ale-yeast rdf:type owl:NamedIndividual ,
                                                 yeast:BrewersYeast ;
                                        yeast:hasAlcoholTolerance "Medium - High (8 - 12%)" ;
                                        yeast:hasFlocculation "Medium" ;
                                        yeast:hasHighAttenuation 75.00 ;
                                        yeast:hasHighOptimumFermentationTemperature 70.00 ;
                                        yeast:hasLowAttenuation 70.00 ;
                                        yeast:hasLowOptimumFermentationTemperature 65.00 ;
                                        yeast:usedForBrewingStyle beertype:american-amber ,
                                                                  beertype:american-brown-ale ,
                                                                  beertype:american-india-pale-ale ,
                                                                  beertype:american-pale-ale ,
                                                                  beertype:american-porter ,
                                                                  beertype:barleywine-ale ,
                                                                  beertype:bourbon-whiskey ,
                                                                  beertype:braggot ,
                                                                  beertype:cream-ale ,
                                                                  beertype:dusseldorf-altbier ,
                                                                  beertype:english-brown-ale ,
                                                                  beertype:english-india-pale-ale ,
                                                                  beertype:english-old-ale ,
                                                                  beertype:english-pale-ale ,
                                                                  beertype:extra-special-bitter ,
                                                                  beertype:foreign-export-stout ,
                                                                  beertype:hazy-ipa-pale-ale ,
                                                                  beertype:imperial-stout ,
                                                                  beertype:irish-dry-stout ,
                                                                  beertype:irish-red-ale ,
                                                                  beertype:kolsch ,
                                                                  beertype:oatmeal-stout ,
                                                                  beertype:ordinary-bitter ,
                                                                  beertype:scotch-ale-wee-heavy ,
                                                                  beertype:scotch-whisky ,
                                                                  beertype:sweet-stout ,
                                                                  beertype:wheat-ale ;
                                        dcterms:bibliographicCitation "http://www.whitelabs.com/yeast-bank/wlp028-edinburgh-scottish-ale-yeast" ;
                                        gr:hasMPN "wlp028" ;
                                        rdfs:label "WLP028 Edinburgh Scottish Ale Yeast" ;
                                        skos:definition "This strain produces underlying esters of pear and melon which work well with hop and malt derived notes. It’s medium to high alcohol tolerance is well-suited for strong Scotch-style ales or barleywine beers. This is a versatile strain that can be neutral at the low end of the recommended fermentation temperature range or provide more esters at the higher range." ;
                                        skos:prefLabel "WLP028 Edinburgh Scottish Ale Yeast" .


###  http://peterbrau.com/whitelabs/yeast-bank/wlp029-german-ale-k-lsch-yeast
wlp:wlp029-german-ale-k-lsch-yeast rdf:type owl:NamedIndividual ,
                                            yeast:BrewersYeast ;
                                   yeast:hasAlcoholTolerance "Medium (5 - 10%)" ;
                                   yeast:hasFlocculation "Medium" ;
                                   yeast:hasHighAttenuation 78.00 ;
                                   yeast:hasHighOptimumFermentationTemperature 69.00 ;
                                   yeast:hasLowAttenuation 72.00 ;
                                   yeast:hasLowOptimumFermentationTemperature 65.00 ;
                                   yeast:usedForBrewingStyle beertype:american-amber ,
                                                             beertype:american-brown-ale ,
                                                             beertype:american-india-pale-ale ,
                                                             beertype:american-pale-ale ,
                                                             beertype:american-porter ,
                                                             beertype:barleywine-ale ,
                                                             beertype:cream-ale ,
                                                             beertype:dusseldorf-altbier ,
                                                             beertype:english-brown-ale ,
                                                             beertype:english-india-pale-ale ,
                                                             beertype:english-old-ale ,
                                                             beertype:english-pale-ale ,
                                                             beertype:extra-special-bitter ,
                                                             beertype:foreign-export-stout ,
                                                             beertype:imperial-india-pale-ale ,
                                                             beertype:imperial-stout ,
                                                             beertype:irish-dry-stout ,
                                                             beertype:irish-red-ale ,
                                                             beertype:kolsch ,
                                                             beertype:oatmeal-stout ,
                                                             beertype:ordinary-bitter ,
                                                             beertype:scotch-ale-wee-heavy ,
                                                             beertype:sweet-stout ,
                                                             beertype:wheat-ale ;
                                   dcterms:bibliographicCitation "http://www.whitelabs.com/yeast-bank/wlp029-german-ale-k-lsch-yeast" ;
                                   gr:hasMPN "wlp029" ;
                                   rdfs:label "WLP029 German Ale/ Kölsch Yeast" ;
                                   skos:definition " " ;
                                   skos:prefLabel "WLP029 German Ale/ Kölsch Yeast" .


###  http://peterbrau.com/whitelabs/yeast-bank/wlp030-thames-valley-ale-yeast
wlp:wlp030-thames-valley-ale-yeast rdf:type owl:NamedIndividual ,
                                            yeast:BrewersYeast ;
                                   yeast:hasFlocculation "High" ;
                                   yeast:hasHighAttenuation 78.00 ;
                                   yeast:hasLowAttenuation 72.00 ;
                                   yeast:usedForBrewingStyle beertype:blonde-ale ,
                                                             beertype:english-brown-ale ,
                                                             beertype:english-india-pale-ale ,
                                                             beertype:english-old-ale ,
                                                             beertype:english-pale-ale ,
                                                             beertype:extra-special-bitter ,
                                                             beertype:foreign-export-stout ,
                                                             beertype:irish-dry-stout ,
                                                             beertype:irish-red-ale ,
                                                             beertype:oatmeal-stout ,
                                                             beertype:ordinary-bitter ;
                                   dcterms:bibliographicCitation "http://www.whitelabs.com/yeast-bank/wlp030-thames-valley-ale-yeast" ;
                                   gr:hasMPN "wlp030" ;
                                   rdfs:label "WLP030 Thames Valley Ale Yeast" ;
                                   skos:definition "Very flocculant strain for all things English. Great for porters, stouts and ESBs. Lower ester production than most English strains but creates a bigger mouthfeel than most cleaner strains." ;
                                   skos:prefLabel "WLP030 Thames Valley Ale Yeast" .


###  http://peterbrau.com/whitelabs/yeast-bank/wlp033-klassic-ale-yeast
wlp:wlp033-klassic-ale-yeast rdf:type owl:NamedIndividual ,
                                      yeast:BrewersYeast ;
                             yeast:hasAlcoholTolerance "Medium (5 - 10%)" ;
                             yeast:hasFlocculation "Medium" ;
                             yeast:hasHighAttenuation 74.00 ;
                             yeast:hasHighOptimumFermentationTemperature 70.00 ;
                             yeast:hasLowAttenuation 66.00 ;
                             yeast:hasLowOptimumFermentationTemperature 66.00 ;
                             yeast:usedForBrewingStyle beertype:american-porter ,
                                                       beertype:american-stout ,
                                                       beertype:extra-special-bitter ,
                                                       beertype:foreign-export-stout ,
                                                       beertype:imperial-stout ,
                                                       beertype:irish-dry-stout ,
                                                       beertype:irish-red-ale ,
                                                       beertype:oatmeal-stout ,
                                                       beertype:ordinary-bitter ,
                                                       beertype:sweet-stout ;
                             dcterms:bibliographicCitation "http://www.whitelabs.com/yeast-bank/wlp033-klassic-ale-yeast" ;
                             gr:hasMPN "wlp033" ;
                             rdfs:label "WLP033 Klassic Ale Yeast" ;
                             skos:definition "Traditional English single-strain yeast. Produces signature ester characters and does not mask hop flavors. Leaves ales with a slightly sweet malt character. Best for bitters, milds, porters and stouts. Also good for Scottish-style ales." ;
                             skos:prefLabel "WLP033 Klassic Ale Yeast" .


###  http://peterbrau.com/whitelabs/yeast-bank/wlp036-d-sseldorf-alt-ale-yeast
wlp:wlp036-d-sseldorf-alt-ale-yeast rdf:type owl:NamedIndividual ,
                                             yeast:BrewersYeast ;
                                    yeast:hasAlcoholTolerance "Medium (5 - 10%)" ;
                                    yeast:hasFlocculation "Medium" ;
                                    yeast:hasHighAttenuation 72.00 ;
                                    yeast:hasHighOptimumFermentationTemperature 69.00 ;
                                    yeast:hasLowAttenuation 65.00 ;
                                    yeast:hasLowOptimumFermentationTemperature 65.00 ;
                                    yeast:usedForBrewingStyle beertype:american-amber ,
                                                              beertype:american-brown-ale ,
                                                              beertype:american-india-pale-ale ,
                                                              beertype:american-pale-ale ,
                                                              beertype:american-porter ,
                                                              beertype:barleywine-ale ,
                                                              beertype:cream-ale ,
                                                              beertype:dusseldorf-altbier ,
                                                              beertype:english-brown-ale ,
                                                              beertype:english-india-pale-ale ,
                                                              beertype:english-old-ale ,
                                                              beertype:english-pale-ale ,
                                                              beertype:extra-special-bitter ,
                                                              beertype:foreign-export-stout ,
                                                              beertype:imperial-stout ,
                                                              beertype:irish-dry-stout ,
                                                              beertype:irish-red-ale ,
                                                              beertype:kolsch ,
                                                              beertype:oatmeal-stout ,
                                                              beertype:ordinary-bitter ,
                                                              beertype:scotch-ale-wee-heavy ,
                                                              beertype:sweet-stout ;
                                    dcterms:bibliographicCitation "http://www.whitelabs.com/yeast-bank/wlp036-d-sseldorf-alt-ale-yeast" ;
                                    gr:hasMPN "wlp036" ;
                                    rdfs:label "WLP036 Düsseldorf Alt Ale Yeast" ;
                                    skos:definition "A traditional altbier-style yeast from Düsseldorf, Germany. It produces clean, malty German brown and amber ales. This strain keeps the contribution of hop bitterness in the background while promoting sweet malt notes." ;
                                    skos:prefLabel "WLP036 Düsseldorf Alt Ale Yeast" .


###  http://peterbrau.com/whitelabs/yeast-bank/wlp037-yorkshire-square-ale-yeast
wlp:wlp037-yorkshire-square-ale-yeast rdf:type owl:NamedIndividual ,
                                               yeast:BrewersYeast ;
                                      yeast:hasAlcoholTolerance "Medium - High (8 - 12%)" ;
                                      yeast:hasFlocculation "High" ;
                                      yeast:hasHighAttenuation 72.00 ;
                                      yeast:hasHighOptimumFermentationTemperature 70.00 ;
                                      yeast:hasLowAttenuation 68.00 ;
                                      yeast:hasLowOptimumFermentationTemperature 65.00 ;
                                      yeast:usedForBrewingStyle beertype:american-brown-ale ,
                                                                beertype:american-pale-ale ,
                                                                beertype:english-brown-ale ,
                                                                beertype:english-pale-ale ,
                                                                beertype:extra-special-bitter ,
                                                                beertype:ordinary-bitter ;
                                      dcterms:bibliographicCitation "http://www.whitelabs.com/yeast-bank/wlp037-yorkshire-square-ale-yeast" ;
                                      gr:hasMPN "wlp037" ;
                                      rdfs:label "WLP037 Yorkshire Square Ale Yeast" ;
                                      skos:definition "This yeast produces a beer that is malty and well balanced. Expect toasty flavors with malt-driven esters. Highly flocculent and a good choice for English-style pale ales, brown ales, and milds." ;
                                      skos:prefLabel "WLP037 Yorkshire Square Ale Yeast" .


###  http://peterbrau.com/whitelabs/yeast-bank/wlp038-manchester-ale-yeast
wlp:wlp038-manchester-ale-yeast rdf:type owl:NamedIndividual ,
                                         yeast:BrewersYeast ;
                                yeast:hasAlcoholTolerance "Medium - High (8 - 12%)" ;
                                yeast:hasFlocculation "Medium to High" ;
                                yeast:hasHighAttenuation 74.00 ;
                                yeast:hasHighOptimumFermentationTemperature 70.00 ;
                                yeast:hasLowAttenuation 70.00 ;
                                yeast:hasLowOptimumFermentationTemperature 65.00 ;
                                yeast:usedForBrewingStyle beertype:english-brown-ale ,
                                                          beertype:english-india-pale-ale ,
                                                          beertype:english-old-ale ,
                                                          beertype:english-pale-ale ,
                                                          beertype:extra-special-bitter ,
                                                          beertype:ordinary-bitter ;
                                dcterms:bibliographicCitation "http://www.whitelabs.com/yeast-bank/wlp038-manchester-ale-yeast" ;
                                gr:hasMPN "wlp038" ;
                                rdfs:label "WLP038 Manchester Ale Yeast" ;
                                skos:definition "A top-fermenting ale yeast that is traditionally good for top-cropping. Moderately flocculent with a clean, dry finish. Has a low ester profile and produces a highly balanced English-style beer." ;
                                skos:prefLabel "WLP038 Manchester Ale Yeast" .


###  http://peterbrau.com/whitelabs/yeast-bank/wlp039-east-midlands-ale-yeast
wlp:wlp039-east-midlands-ale-yeast rdf:type owl:NamedIndividual ,
                                            yeast:BrewersYeast ;
                                   yeast:hasAlcoholTolerance "Medium (5 - 10%)" ;
                                   yeast:hasFlocculation "Medium to High" ;
                                   yeast:hasHighAttenuation 82.00 ;
                                   yeast:hasHighOptimumFermentationTemperature 70.00 ;
                                   yeast:hasLowAttenuation 73.00 ;
                                   yeast:hasLowOptimumFermentationTemperature 66.00 ;
                                   yeast:usedForBrewingStyle beertype:american-pale-ale ,
                                                             beertype:american-porter ,
                                                             beertype:american-stout ,
                                                             beertype:english-pale-ale ,
                                                             beertype:foreign-export-stout ,
                                                             beertype:imperial-stout ,
                                                             beertype:oatmeal-stout ;
                                   dcterms:bibliographicCitation "http://www.whitelabs.com/yeast-bank/wlp039-east-midlands-ale-yeast" ;
                                   gr:hasMPN "wlp039" ;
                                   rdfs:label "WLP039 East Midlands Ale Yeast" ;
                                   skos:definition "British-style ale yeast with a very dry finish. Medium to low fruit and fusel alcohol production. A good top-fermenting yeast strain well suited for top-cropping. A great choice for pale ales, ambers, porters and stouts." ;
                                   skos:prefLabel "WLP039 East Midlands Ale Yeast" .


###  http://peterbrau.com/whitelabs/yeast-bank/wlp041-pacific-ale-yeast
wlp:wlp041-pacific-ale-yeast rdf:type owl:NamedIndividual ,
                                      yeast:BrewersYeast ;
                             yeast:hasAlcoholTolerance "Medium (5 - 10%)" ;
                             yeast:hasFlocculation "High" ;
                             yeast:hasHighAttenuation 70.00 ;
                             yeast:hasHighOptimumFermentationTemperature 68.00 ;
                             yeast:hasLowAttenuation 65.00 ;
                             yeast:hasLowOptimumFermentationTemperature 65.00 ;
                             yeast:usedForBrewingStyle beertype:american-amber ,
                                                       beertype:american-brown-ale ,
                                                       beertype:american-india-pale-ale ,
                                                       beertype:american-pale-ale ,
                                                       beertype:american-porter ,
                                                       beertype:barleywine-ale ,
                                                       beertype:cream-ale ,
                                                       beertype:english-brown-ale ,
                                                       beertype:english-india-pale-ale ,
                                                       beertype:english-old-ale ,
                                                       beertype:english-pale-ale ,
                                                       beertype:extra-special-bitter ,
                                                       beertype:foreign-export-stout ,
                                                       beertype:imperial-stout ,
                                                       beertype:irish-dry-stout ,
                                                       beertype:irish-red-ale ,
                                                       beertype:oatmeal-stout ,
                                                       beertype:scotch-ale-wee-heavy ,
                                                       beertype:sweet-stout ;
                             dcterms:bibliographicCitation "http://www.whitelabs.com/yeast-bank/wlp041-pacific-ale-yeast" ;
                             gr:hasMPN "wlp041" ;
                             rdfs:label "WLP041 Pacific Ale Yeast" ;
                             skos:definition "Hailing from the Pacific Northwest, this strain is a mild ester producer while promoting malt character. It can be used for a range of styles from an English mild to an American IPA or Irish stout. A great flocculator, it leaves a clear beer and saves on conditioning time." ;
                             skos:prefLabel "WLP041 Pacific Ale Yeast" .


###  http://peterbrau.com/whitelabs/yeast-bank/wlp045-scotch-whisky-yeast
wlp:wlp045-scotch-whisky-yeast rdf:type owl:NamedIndividual ,
                                        yeast:BrewersYeast ;
                               yeast:hasAlcoholTolerance "High (10 - 15%)" ;
                               yeast:hasFlocculation "Medium" ;
                               yeast:hasHighAttenuation 80.00 ;
                               yeast:hasHighOptimumFermentationTemperature 77.00 ;
                               yeast:hasLowAttenuation 75.00 ;
                               yeast:hasLowOptimumFermentationTemperature 72.00 ;
                               yeast:usedForBrewingStyle beertype:scotch-whisky ;
                               dcterms:bibliographicCitation "http://www.whitelabs.com/yeast-bank/wlp045-scotch-whisky-yeast" ;
                               gr:hasMPN "wlp045" ;
                               rdfs:label "WLP045 Scotch Whisky Yeast" ;
                               skos:definition "A strain that has been widely used for Scotch whisky production since the early 1950s. This yeast produces a complex array of ester compounds and fusel oils, as well as some spicy clover character. Suitable for Scotch or American-style whiskeys." ;
                               skos:prefLabel "WLP045 Scotch Whisky Yeast" .


###  http://peterbrau.com/whitelabs/yeast-bank/wlp050-tennessee-whiskey-yeast
wlp:wlp050-tennessee-whiskey-yeast rdf:type owl:NamedIndividual ,
                                            yeast:BrewersYeast ;
                                   yeast:hasAlcoholTolerance "High (10 - 15%)" ;
                                   yeast:hasFlocculation "Medium" ;
                                   yeast:hasHighAttenuation 80.00 ;
                                   yeast:hasHighOptimumFermentationTemperature 79.00 ;
                                   yeast:hasLowAttenuation 75.00 ;
                                   yeast:hasLowOptimumFermentationTemperature 75.00 ;
                                   yeast:usedForBrewingStyle beertype:bourbon-whiskey ,
                                                             beertype:rye-whiskey ;
                                   dcterms:bibliographicCitation "http://www.whitelabs.com/yeast-bank/wlp050-tennessee-whiskey-yeast" ;
                                   gr:hasMPN "wlp050" ;
                                   rdfs:label "WLP050 Tennessee Whiskey Yeast" ;
                                   skos:definition "Suitable or American-style whiskeys and bourbons, this strain is famous for creating rich, smooth flavors. A clean and dry-fermenting yeast that will tolerate high alcohol concentrations (up to 15% ABV). Ester production is low." ;
                                   skos:prefLabel "WLP050 Tennessee Whiskey Yeast" .


###  http://peterbrau.com/whitelabs/yeast-bank/wlp051-california-v-ale-yeast
wlp:wlp051-california-v-ale-yeast rdf:type owl:NamedIndividual ,
                                           yeast:BrewersYeast ;
                                  yeast:hasAlcoholTolerance "Medium - High (8 - 12%)" ;
                                  yeast:hasFlocculation "Medium to High" ;
                                  yeast:hasHighAttenuation 75.00 ;
                                  yeast:hasHighOptimumFermentationTemperature 70.00 ;
                                  yeast:hasLowAttenuation 70.00 ;
                                  yeast:hasLowOptimumFermentationTemperature 66.00 ;
                                  yeast:usedForBrewingStyle beertype:american-amber ,
                                                            beertype:american-brown-ale ,
                                                            beertype:american-india-pale-ale ,
                                                            beertype:american-pale-ale ,
                                                            beertype:american-porter ,
                                                            beertype:barleywine-ale ,
                                                            beertype:cream-ale ,
                                                            beertype:dusseldorf-altbier ,
                                                            beertype:english-brown-ale ,
                                                            beertype:english-india-pale-ale ,
                                                            beertype:english-old-ale ,
                                                            beertype:english-pale-ale ,
                                                            beertype:extra-special-bitter ,
                                                            beertype:foreign-export-stout ,
                                                            beertype:imperial-india-pale-ale ,
                                                            beertype:imperial-stout ,
                                                            beertype:irish-dry-stout ,
                                                            beertype:irish-red-ale ,
                                                            beertype:kolsch ,
                                                            beertype:oatmeal-stout ,
                                                            beertype:ordinary-bitter ,
                                                            beertype:scotch-ale-wee-heavy ,
                                                            beertype:sweet-stout ,
                                                            beertype:wheat-ale ;
                                  dcterms:bibliographicCitation "http://www.whitelabs.com/yeast-bank/wlp051-california-v-ale-yeast" ;
                                  gr:hasMPN "wlp051" ;
                                  rdfs:label "WLP051 California V Ale Yeast" ;
                                  skos:definition "This strain has more similarities to an English strain than WLP001 California Ale Yeast®. It is a big ester producer, showcasing notes of cherry and apple which compliment pale ales, blonde and brown ales. Typically leaves some residual, lager-like sulfur compounds in finished beer. Recent sequencing studies show that WLP051 belongs to Saccharomyces pastorianus species, the same hybrid species as most lager strains. However, this strain has been used to make ales for decades and was previously categorized as belonging to Saccharomyces cerevisiae." ;
                                  skos:prefLabel "WLP051 California V Ale Yeast" .


###  http://peterbrau.com/whitelabs/yeast-bank/wlp059-melbourne-ale-yeast
wlp:wlp059-melbourne-ale-yeast rdf:type owl:NamedIndividual ,
                                        yeast:BrewersYeast ;
                               yeast:hasFlocculation "Medium" ;
                               yeast:hasHighAttenuation 78.00 ;
                               yeast:hasLowAttenuation 74.00 ;
                               yeast:usedForBrewingStyle beertype:american-india-pale-ale ,
                                                         beertype:american-pale-ale ,
                                                         beertype:blonde-ale ,
                                                         beertype:english-india-pale-ale ,
                                                         beertype:english-pale-ale ,
                                                         beertype:ordinary-bitter ,
                                                         beertype:wheat-ale ;
                               dcterms:bibliographicCitation "http://www.whitelabs.com/yeast-bank/wlp059-melbourne-ale-yeast" ;
                               gr:hasMPN "wlp059" ;
                               rdfs:label "WLP059 Melbourne Ale Yeast" ;
                               skos:definition "A yeast isolated from Australia in the early 1900s, it is a clean fermenting strain well suited for many American and English beer styles. Renowned Australian homebrewer, Peter Symon, researched this strain for his book Bronzed Brews and asked White Labs to acquire it from a yeast bank in London, England. This historic strain was used in Australia because of its ability to ferment well in the Australian climate and Australian cane sugar." ;
                               skos:prefLabel "WLP059 Melbourne Ale Yeast" .


###  http://peterbrau.com/whitelabs/yeast-bank/wlp060-american-ale-yeast-blend
wlp:wlp060-american-ale-yeast-blend rdf:type owl:NamedIndividual ,
                                             yeast:BrewersYeast ;
                                    yeast:hasAlcoholTolerance "Medium - High (8 - 12%)" ;
                                    yeast:hasFlocculation "Medium" ;
                                    yeast:hasHighAttenuation 80.00 ;
                                    yeast:hasHighOptimumFermentationTemperature 72.00 ;
                                    yeast:hasLowAttenuation 72.00 ;
                                    yeast:hasLowOptimumFermentationTemperature 68.00 ;
                                    yeast:usedForBrewingStyle beertype:american-amber ,
                                                              beertype:american-brown-ale ,
                                                              beertype:american-india-pale-ale ,
                                                              beertype:american-pale-ale ,
                                                              beertype:american-porter ,
                                                              beertype:barleywine-ale ,
                                                              beertype:braggot ,
                                                              beertype:cream-ale ,
                                                              beertype:dusseldorf-altbier ,
                                                              beertype:english-brown-ale ,
                                                              beertype:english-old-ale ,
                                                              beertype:english-pale-ale ,
                                                              beertype:extra-special-bitter ,
                                                              beertype:foreign-export-stout ,
                                                              beertype:imperial-india-pale-ale ,
                                                              beertype:imperial-stout ,
                                                              beertype:irish-dry-stout ,
                                                              beertype:irish-red-ale ,
                                                              beertype:kolsch ,
                                                              beertype:oatmeal-stout ,
                                                              beertype:ordinary-bitter ,
                                                              beertype:scotch-ale-wee-heavy ,
                                                              beertype:wheat-ale ;
                                    dcterms:bibliographicCitation "http://www.whitelabs.com/yeast-bank/wlp060-american-ale-yeast-blend" ;
                                    gr:hasMPN "wlp060" ;
                                    rdfs:label "WLP060 American Ale Yeast Blend" ;
                                    skos:definition "This blend of three strains creates a clean and neutral fermentation character, making it ideal for use in many different American beer styles. The blend lends complexity to finished beer by exhibiting a crisp, clean lager-like character with accentuated hop flavors and bitterness. A slight amount of sulfur can be produced during peak fermentation." ;
                                    skos:prefLabel "WLP060 American Ale Yeast Blend" .


###  http://peterbrau.com/whitelabs/yeast-bank/wlp064-buchner-ale-yeast-blend
wlp:wlp064-buchner-ale-yeast-blend rdf:type owl:NamedIndividual ,
                                            yeast:BrewersYeast ;
                                   yeast:hasAlcoholTolerance "Medium - High (8 - 12%)" ;
                                   yeast:hasFlocculation "Medium" ;
                                   yeast:hasHighAttenuation 78.00 ;
                                   yeast:hasHighOptimumFermentationTemperature 72.00 ;
                                   yeast:hasLowAttenuation 72.00 ;
                                   yeast:hasLowOptimumFermentationTemperature 67.00 ;
                                   yeast:usedForBrewingStyle beertype:american-amber ,
                                                             beertype:american-brown-ale ,
                                                             beertype:american-pale-ale ,
                                                             beertype:american-porter ,
                                                             beertype:blonde-ale ,
                                                             beertype:cream-ale ,
                                                             beertype:english-brown-ale ,
                                                             beertype:wheat-ale ;
                                   dcterms:bibliographicCitation "http://www.whitelabs.com/yeast-bank/wlp064-buchner-ale-yeast-blend" ;
                                   gr:hasMPN "wlp064" ;
                                   rdfs:label "WLP064 Buchner Ale Yeast Blend" ;
                                   skos:definition "A blend of two strains that adds creaminess with a hint of crispness. Great for pale ales, cream ales and American wheats. Flocculation is good due to one of the strains being a heavy flocculator." ;
                                   skos:prefLabel "WLP064 Buchner Ale Yeast Blend" .


###  http://peterbrau.com/whitelabs/yeast-bank/wlp065-american-whiskey-yeast
wlp:wlp065-american-whiskey-yeast rdf:type owl:NamedIndividual ,
                                           yeast:BrewersYeast ;
                                  yeast:hasAlcoholTolerance "High (10 - 15%)" ;
                                  yeast:hasFlocculation "Medium" ;
                                  yeast:hasHighAttenuation 82.00 ;
                                  yeast:hasHighOptimumFermentationTemperature 82.00 ;
                                  yeast:hasLowAttenuation 76.00 ;
                                  yeast:hasLowOptimumFermentationTemperature 75.00 ;
                                  yeast:usedForBrewingStyle beertype:bourbon-whiskey ,
                                                            beertype:rye-whiskey ;
                                  dcterms:bibliographicCitation "http://www.whitelabs.com/yeast-bank/wlp065-american-whiskey-yeast" ;
                                  gr:hasMPN "wlp065" ;
                                  rdfs:label "WLP065 American Whiskey Yeast" ;
                                  skos:definition "A yeast strain that produces a low ester profile and moderate fusel oils. It is temperature and alcohol tolerant and suitable for American-style whiskeys using barley or corn bases." ;
                                  skos:prefLabel "WLP065 American Whiskey Yeast" .


###  http://peterbrau.com/whitelabs/yeast-bank/wlp066-london-fog-ale-yeast
wlp:wlp066-london-fog-ale-yeast rdf:type owl:NamedIndividual ,
                                         yeast:BrewersYeast ;
                                yeast:hasAlcoholTolerance "Medium - High (8 - 12%)" ;
                                yeast:hasFlocculation "Medium to Low" ;
                                yeast:hasHighAttenuation 82.00 ;
                                yeast:hasHighOptimumFermentationTemperature 72.00 ;
                                yeast:hasLowAttenuation 75.00 ;
                                yeast:hasLowOptimumFermentationTemperature 64.00 ;
                                yeast:usedForBrewingStyle beertype:american-amber ,
                                                          beertype:american-india-pale-ale ,
                                                          beertype:american-pale-ale ,
                                                          beertype:blonde-ale ,
                                                          beertype:english-india-pale-ale ,
                                                          beertype:english-pale-ale ,
                                                          beertype:extra-special-bitter ,
                                                          beertype:hazy-ipa-pale-ale ,
                                                          beertype:imperial-india-pale-ale ,
                                                          beertype:irish-red-ale ,
                                                          beertype:ordinary-bitter ;
                                dcterms:bibliographicCitation "http://www.whitelabs.com/yeast-bank/wlp066-london-fog-ale-yeast" ;
                                gr:hasMPN "wlp066" ;
                                rdfs:label "WLP066 London Fog Ale Yeast" ;
                                skos:definition "This is the go-to strain for New England-style IPAs. It produces a medium ester profile similar to WLP008 East Coast Ale Yeast. It leaves some residual sweetness, helping accentuate both malt and hop flavors and aromas, while retaining a velvety mouthfeel." ;
                                skos:prefLabel "WLP066 London Fog Ale Yeast" .


###  http://peterbrau.com/whitelabs/yeast-bank/wlp067-coastal-haze-ale-yeast-blend
wlp:wlp067-coastal-haze-ale-yeast-blend rdf:type owl:NamedIndividual ,
                                                 yeast:BrewersYeast ;
                                        yeast:hasAlcoholTolerance "Medium - High (8 - 12%)" ;
                                        yeast:hasFlocculation "Medium to Low" ;
                                        yeast:hasHighAttenuation 75.00 ;
                                        yeast:hasHighOptimumFermentationTemperature 72.00 ;
                                        yeast:hasLowAttenuation 70.00 ;
                                        yeast:hasLowOptimumFermentationTemperature 68.00 ;
                                        yeast:usedForBrewingStyle beertype:american-india-pale-ale ,
                                                                  beertype:american-pale-ale ,
                                                                  beertype:blonde-ale ,
                                                                  beertype:hazy-ipa-pale-ale ,
                                                                  beertype:imperial-india-pale-ale ;
                                        dcterms:bibliographicCitation "http://www.whitelabs.com/yeast-bank/wlp067-coastal-haze-ale-yeast-blend" ;
                                        gr:hasMPN "wlp067" ;
                                        rdfs:label "WLP067 Coastal Haze Ale Yeast Blend" ;
                                        skos:definition "This blend of our favorite New England-style IPA strains is great for producing beers with a hazy appearance and tropical, fruit-forward esters. Producing dry, yet juicy beers, the mango and pineapple characteristics will lend to added drinkability." ;
                                        skos:prefLabel "WLP067 Coastal Haze Ale Yeast Blend" .


###  http://peterbrau.com/whitelabs/yeast-bank/wlp070-kentucky-bourbon-yeast
wlp:wlp070-kentucky-bourbon-yeast rdf:type owl:NamedIndividual ,
                                           yeast:BrewersYeast ;
                                  yeast:hasAlcoholTolerance "High (10 - 15%)" ;
                                  yeast:hasFlocculation "Medium" ;
                                  yeast:hasHighAttenuation 80.00 ;
                                  yeast:hasHighOptimumFermentationTemperature 77.00 ;
                                  yeast:hasLowAttenuation 75.00 ;
                                  yeast:hasLowOptimumFermentationTemperature 72.00 ;
                                  yeast:usedForBrewingStyle beertype:bourbon-whiskey ;
                                  dcterms:bibliographicCitation "http://www.whitelabs.com/yeast-bank/wlp070-kentucky-bourbon-yeast" ;
                                  gr:hasMPN "wlp070" ;
                                  rdfs:label "WLP070 Kentucky Bourbon Yeast" ;
                                  skos:definition "From a traditional distillery in the heart of Bourbon Country, this strain produces a malty caramel character with a balanced ester profile. Suitable for bourbons or other American whiskeys with barley, rye, or corn base grains." ;
                                  skos:prefLabel "WLP070 Kentucky Bourbon Yeast" .


###  http://peterbrau.com/whitelabs/yeast-bank/wlp072-french-ale-yeast
wlp:wlp072-french-ale-yeast rdf:type owl:NamedIndividual ,
                                     yeast:BrewersYeast ;
                            yeast:hasAlcoholTolerance "Medium (5 - 10%)" ;
                            yeast:hasFlocculation "Medium to High" ;
                            yeast:hasHighAttenuation 75.00 ;
                            yeast:hasHighOptimumFermentationTemperature 73.00 ;
                            yeast:hasLowAttenuation 68.00 ;
                            yeast:hasLowOptimumFermentationTemperature 63.00 ;
                            yeast:usedForBrewingStyle beertype:american-amber ,
                                                      beertype:american-brown-ale ,
                                                      beertype:blonde-ale ,
                                                      beertype:english-brown-ale ;
                            dcterms:bibliographicCitation "http://www.whitelabs.com/yeast-bank/wlp072-french-ale-yeast" ;
                            gr:hasMPN "wlp072" ;
                            rdfs:label "WLP072 French Ale Yeast" ;
                            skos:definition "A clean strain that complements malt flavor. Low to moderate esters are produced when fermentation temperature is below 70°F (21°C). Moderate to high ester character achieved above 70°F (21°C). Low diacetyl production. A good yeast strain for Bière de Garde, blondes, ambers, brown ales and specialty beers." ;
                            skos:prefLabel "WLP072 French Ale Yeast" .


###  http://peterbrau.com/whitelabs/yeast-bank/wlp073-artisanal-country-ale-yeast
wlp:wlp073-artisanal-country-ale-yeast rdf:type owl:NamedIndividual ,
                                                yeast:BrewersYeast ;
                                       yeast:hasAlcoholTolerance "Medium - High (8 - 12%)" ;
                                       yeast:hasFlocculation "Medium to Low" ;
                                       yeast:hasHighAttenuation 80.00 ;
                                       yeast:hasHighOptimumFermentationTemperature 82.00 ;
                                       yeast:hasLowAttenuation 75.00 ;
                                       yeast:hasLowOptimumFermentationTemperature 70.00 ;
                                       yeast:usedForBrewingStyle beertype:belgian-dark-strong-ale ,
                                                                 beertype:belgian-table-bier ,
                                                                 beertype:biere-de-garde ,
                                                                 beertype:blonde-ale ,
                                                                 beertype:dubbel ,
                                                                 beertype:saison ,
                                                                 beertype:specialty-belgian ,
                                                                 beertype:tripel ;
                                       dcterms:bibliographicCitation "http://www.whitelabs.com/yeast-bank/wlp073-artisanal-country-ale-yeast" ;
                                       gr:hasMPN "wlp073" ;
                                       rdfs:label "WLP073 Artisanal Country Ale Yeast" ;
                                       skos:definition "A classic Bière de Garde strain, it produces slight esters and mild phenols, while preserving the sweet aromatics from the malt bill. This strain fully attenuates, leaving the beer with a crisp, dry finish." ;
                                       skos:prefLabel "WLP073 Artisanal Country Ale Yeast" .


###  http://peterbrau.com/whitelabs/yeast-bank/wlp075-hansen-ale-yeast-blend
wlp:wlp075-hansen-ale-yeast-blend rdf:type owl:NamedIndividual ,
                                           yeast:BrewersYeast ;
                                  yeast:hasAlcoholTolerance "High (10 - 15%)" ;
                                  yeast:hasFlocculation "Medium to High" ;
                                  yeast:hasHighAttenuation 80.00 ;
                                  yeast:hasHighOptimumFermentationTemperature 70.00 ;
                                  yeast:hasLowAttenuation 75.00 ;
                                  yeast:hasLowOptimumFermentationTemperature 66.00 ;
                                  yeast:usedForBrewingStyle beertype:american-amber ,
                                                            beertype:american-india-pale-ale ,
                                                            beertype:american-pale-ale ,
                                                            beertype:american-porter ,
                                                            beertype:american-stout ,
                                                            beertype:barleywine-ale ,
                                                            beertype:blonde-ale ,
                                                            beertype:imperial-india-pale-ale ,
                                                            beertype:imperial-stout ;
                                  dcterms:bibliographicCitation "http://www.whitelabs.com/yeast-bank/wlp075-hansen-ale-yeast-blend" ;
                                  gr:hasMPN "wlp075" ;
                                  rdfs:label "WLP075 Hansen Ale Yeast Blend" ;
                                  skos:definition "This is a blend of many IPA strain favorites. It has the attenuation of WLP090 San Diego Super Ale Yeast and the character of WLP007 Dry English Ale Yeast. This strain produces dry, hop-forward beers with minor ester production and is blend is a great flocculator." ;
                                  skos:prefLabel "WLP075 Hansen Ale Yeast Blend" .


###  http://peterbrau.com/whitelabs/yeast-bank/wlp076-old-sonoma-ale-yeast
wlp:wlp076-old-sonoma-ale-yeast rdf:type owl:NamedIndividual ,
                                         yeast:BrewersYeast ;
                                yeast:hasAlcoholTolerance "Medium (5 - 10%)" ;
                                yeast:hasFlocculation "Medium" ;
                                yeast:hasHighAttenuation 74.00 ;
                                yeast:hasHighOptimumFermentationTemperature 70.00 ;
                                yeast:hasLowAttenuation 70.00 ;
                                yeast:hasLowOptimumFermentationTemperature 66.00 ;
                                yeast:usedForBrewingStyle beertype:american-pale-ale ,
                                                          beertype:american-porter ,
                                                          beertype:american-stout ,
                                                          beertype:english-brown-ale ,
                                                          beertype:english-pale-ale ,
                                                          beertype:imperial-stout ;
                                dcterms:bibliographicCitation "http://www.whitelabs.com/yeast-bank/wlp076-old-sonoma-ale-yeast" ;
                                gr:hasMPN "wlp076" ;
                                rdfs:label "WLP076 Old Sonoma Ale Yeast" ;
                                skos:definition "From a historic brewery in Northern California. This strain was embraced by the early pioneers of craft beer in America and is ideal for those seeking to use a traditional British-style yeast. A neutral and versatile strain, a great for pale ales, porters, and stouts." ;
                                skos:prefLabel "WLP076 Old Sonoma Ale Yeast" .


###  http://peterbrau.com/whitelabs/yeast-bank/wlp078-neutral-grain-yeast
wlp:wlp078-neutral-grain-yeast rdf:type owl:NamedIndividual ,
                                        yeast:BrewersYeast ;
                               yeast:hasAlcoholTolerance "High (10 - 15%)" ;
                               yeast:hasFlocculation "Medium" ;
                               yeast:hasHighAttenuation 84.00 ;
                               yeast:hasHighOptimumFermentationTemperature 85.00 ;
                               yeast:hasLowAttenuation 77.00 ;
                               yeast:hasLowOptimumFermentationTemperature 76.00 ;
                               yeast:usedForBrewingStyle beertype:bourbon-whiskey ,
                                                         beertype:gin ,
                                                         beertype:rye-whiskey ,
                                                         beertype:scotch-whisky ,
                                                         beertype:tequila ,
                                                         beertype:vodka ;
                               dcterms:bibliographicCitation "http://www.whitelabs.com/yeast-bank/wlp078-neutral-grain-yeast" ;
                               gr:hasMPN "wlp078" ;
                               rdfs:label "WLP078 Neutral Grain Yeast" ;
                               skos:definition "Marked by a clean, fast fermentation, this strain is ideal for any neutral grain spirit. Alcohol and temperature tolerant." ;
                               skos:prefLabel "WLP078 Neutral Grain Yeast" .


###  http://peterbrau.com/whitelabs/yeast-bank/wlp080-cream-ale-yeast-blend
wlp:wlp080-cream-ale-yeast-blend rdf:type owl:NamedIndividual ,
                                          yeast:BrewersYeast ;
                                 yeast:hasAlcoholTolerance "Medium - High (8 - 12%)" ;
                                 yeast:hasFlocculation "Medium" ;
                                 yeast:hasHighAttenuation 80.00 ;
                                 yeast:hasHighOptimumFermentationTemperature 70.00 ;
                                 yeast:hasLowAttenuation 75.00 ;
                                 yeast:hasLowOptimumFermentationTemperature 65.00 ;
                                 yeast:usedForBrewingStyle beertype:cream-ale ,
                                                           beertype:dusseldorf-altbier ,
                                                           beertype:kolsch ,
                                                           beertype:ordinary-bitter ;
                                 dcterms:bibliographicCitation "http://www.whitelabs.com/yeast-bank/wlp080-cream-ale-yeast-blend" ;
                                 gr:hasMPN "wlp080" ;
                                 rdfs:label "WLP080 Cream Ale Yeast Blend" ;
                                 skos:definition "A blend of ale and lager yeast, this strain produces a classic cream ale. The blend produces a pleasing light fruity note from the ale yeast, while the lager strain produces clean pilsner-like flavors and a slightly subdued hop bitterness. This blend is known for producing subtle sulfur during primary fermentation." ;
                                 skos:prefLabel "WLP080 Cream Ale Yeast Blend" .


###  http://peterbrau.com/whitelabs/yeast-bank/wlp085-english-ale-yeast-blend
wlp:wlp085-english-ale-yeast-blend rdf:type owl:NamedIndividual ,
                                            yeast:BrewersYeast ;
                                   yeast:hasAlcoholTolerance "Medium (5 - 10%)" ;
                                   yeast:hasFlocculation "Medium to High" ;
                                   yeast:hasHighAttenuation 76.00 ;
                                   yeast:hasHighOptimumFermentationTemperature 72.00 ;
                                   yeast:hasLowAttenuation 69.00 ;
                                   yeast:hasLowOptimumFermentationTemperature 68.00 ;
                                   yeast:usedForBrewingStyle beertype:american-amber ,
                                                             beertype:american-brown-ale ,
                                                             beertype:american-india-pale-ale ,
                                                             beertype:american-pale-ale ,
                                                             beertype:american-porter ,
                                                             beertype:barleywine-ale ,
                                                             beertype:cream-ale ,
                                                             beertype:english-brown-ale ,
                                                             beertype:english-india-pale-ale ,
                                                             beertype:english-old-ale ,
                                                             beertype:english-pale-ale ,
                                                             beertype:extra-special-bitter ,
                                                             beertype:foreign-export-stout ,
                                                             beertype:imperial-india-pale-ale ,
                                                             beertype:imperial-stout ,
                                                             beertype:irish-dry-stout ,
                                                             beertype:irish-red-ale ,
                                                             beertype:kolsch ,
                                                             beertype:oatmeal-stout ,
                                                             beertype:ordinary-bitter ,
                                                             beertype:scotch-ale-wee-heavy ,
                                                             beertype:wheat-ale ;
                                   dcterms:bibliographicCitation "http://www.whitelabs.com/yeast-bank/wlp085-english-ale-yeast-blend" ;
                                   gr:hasMPN "wlp085" ;
                                   rdfs:label "WLP085 English Ale Yeast Blend" ;
                                   skos:definition "A blend of British ale yeast strains designed to add complexity and attenuation to your ale. Moderate fruitiness and mineral-like character, with little to no sulfur. Drier than WLP002 English Ale Yeast and WLP005 British Ale Yeast, but with similar flocculation properties. Suitable for English pale ales, bitters, porters, stouts and IPAs." ;
                                   skos:prefLabel "WLP085 English Ale Yeast Blend" .


###  http://peterbrau.com/whitelabs/yeast-bank/wlp090-san-diego-super-yeast
wlp:wlp090-san-diego-super-yeast rdf:type owl:NamedIndividual ,
                                          yeast:BrewersYeast ;
                                 yeast:hasAlcoholTolerance "High (10 - 15%)" ;
                                 yeast:hasFlocculation "Medium to High" ;
                                 yeast:hasHighAttenuation 83.00 ;
                                 yeast:hasHighOptimumFermentationTemperature 68.00 ;
                                 yeast:hasLowAttenuation 76.00 ;
                                 yeast:hasLowOptimumFermentationTemperature 65.00 ;
                                 yeast:usedForBrewingStyle beertype:american-amber ,
                                                           beertype:american-brown-ale ,
                                                           beertype:american-india-pale-ale ,
                                                           beertype:american-pale-ale ,
                                                           beertype:american-porter ,
                                                           beertype:barleywine-ale ,
                                                           beertype:cream-ale ,
                                                           beertype:dusseldorf-altbier ,
                                                           beertype:english-brown-ale ,
                                                           beertype:english-old-ale ,
                                                           beertype:english-pale-ale ,
                                                           beertype:extra-special-bitter ,
                                                           beertype:foreign-export-stout ,
                                                           beertype:imperial-india-pale-ale ,
                                                           beertype:imperial-stout ,
                                                           beertype:irish-dry-stout ,
                                                           beertype:irish-red-ale ,
                                                           beertype:kolsch ,
                                                           beertype:oatmeal-stout ,
                                                           beertype:ordinary-bitter ,
                                                           beertype:scotch-ale-wee-heavy ,
                                                           beertype:wheat-ale ;
                                 dcterms:bibliographicCitation "http://www.whitelabs.com/yeast-bank/wlp090-san-diego-super-yeast" ;
                                 gr:hasMPN "wlp090" ;
                                 rdfs:label "WLP090 San Diego Super Yeast " ;
                                 skos:definition "A low ester producing strain, it’s known for quick fermentations and producing a neutral flavor and aroma profile similar to WLP001 California Ale Yeast®. Due to high attenuation, this strain produces very dry beers with increased perceived bitterness. It also has a high alcohol tolerance which is suitable for a variety of styles and beverages from double IPAs to barleywines, ciders and mead. This is a great all around house strain and ideal for breweries who produce hop-forward beers." ;
                                 skos:prefLabel "WLP090 San Diego Super Yeast " .


###  http://peterbrau.com/whitelabs/yeast-bank/wlp095-burlington-ale-yeast
wlp:wlp095-burlington-ale-yeast rdf:type owl:NamedIndividual ,
                                         yeast:BrewersYeast ;
                                yeast:hasAlcoholTolerance "Medium - High (8 - 12%)" ;
                                yeast:hasFlocculation "Medium" ;
                                yeast:hasHighAttenuation 78.00 ;
                                yeast:hasHighOptimumFermentationTemperature 70.00 ;
                                yeast:hasLowAttenuation 73.00 ;
                                yeast:hasLowOptimumFermentationTemperature 67.00 ;
                                yeast:usedForBrewingStyle beertype:american-india-pale-ale ,
                                                          beertype:american-pale-ale ,
                                                          beertype:english-india-pale-ale ,
                                                          beertype:english-pale-ale ,
                                                          beertype:hazy-ipa-pale-ale ;
                                dcterms:bibliographicCitation "http://www.whitelabs.com/yeast-bank/wlp095-burlington-ale-yeast" ;
                                gr:hasMPN "wlp095" ;
                                rdfs:label "WLP095 Burlington Ale Yeast" ;
                                skos:definition " " ;
                                skos:prefLabel "WLP095 Burlington Ale Yeast" .


###  http://peterbrau.com/whitelabs/yeast-bank/wlp099-super-high-gravity-ale-yeast
wlp:wlp099-super-high-gravity-ale-yeast rdf:type owl:NamedIndividual ,
                                                 yeast:BrewersYeast ;
                                        yeast:hasAlcoholTolerance "Very High (Over 15%)" ;
                                        yeast:hasFlocculation "Medium" ;
                                        yeast:hasHighAttenuation 100.00 ;
                                        yeast:hasHighOptimumFermentationTemperature 69.00 ;
                                        yeast:hasLowAttenuation 80.00 ;
                                        yeast:hasLowOptimumFermentationTemperature 65.00 ;
                                        yeast:usedForBrewingStyle beertype:american-amber ,
                                                                  beertype:barleywine-ale ,
                                                                  beertype:english-old-ale ,
                                                                  beertype:foreign-export-stout ,
                                                                  beertype:imperial-india-pale-ale ,
                                                                  beertype:imperial-stout ;
                                        dcterms:bibliographicCitation "http://www.whitelabs.com/yeast-bank/wlp099-super-high-gravity-ale-yeast" ;
                                        gr:hasMPN "wlp099" ;
                                        rdfs:label "WLP099 Super High Gravity Ale Yeast" ;
                                        skos:definition "From England, this yeast can ferment up to 25% alcohol when used correctly. It produces ester characters that increase with increasing gravity. Malt character dominates at lower gravities. To achieve >25% ABV, sugar needs to be fed over the course of the fermentation." ;
                                        skos:prefLabel "WLP099 Super High Gravity Ale Yeast" .


###  http://peterbrau.com/whitelabs/yeast-bank/wlp1983-charlies-fist-bump-yeast
wlp:wlp1983-charlies-fist-bump-yeast rdf:type owl:NamedIndividual ,
                                              yeast:BrewersYeast ;
                                     yeast:hasAlcoholTolerance "Medium (5 - 10%)" ;
                                     yeast:hasFlocculation "Low" ;
                                     yeast:hasHighAttenuation 70.00 ;
                                     yeast:hasHighOptimumFermentationTemperature 73.00 ;
                                     yeast:hasLowAttenuation 66.00 ;
                                     yeast:hasLowOptimumFermentationTemperature 55.00 ;
                                     yeast:usedForBrewingStyle beertype:american-lager ,
                                                               beertype:american-light-lager ,
                                                               beertype:bock ,
                                                               beertype:bohemian-pilsner ,
                                                               beertype:doppelbock ,
                                                               beertype:english-pale-ale ,
                                                               beertype:lager ,
                                                               beertype:m-nchen-helles ,
                                                               beertype:m-nchner-dunkel ,
                                                               beertype:m-rzen ,
                                                               beertype:schwarzbier ,
                                                               beertype:vienna-lager ;
                                     dcterms:bibliographicCitation "http://www.whitelabs.com/yeast-bank/wlp1983-charlies-fist-bump-yeast" ;
                                     gr:hasMPN "wlp1983" ;
                                     rdfs:label "WLP1983 Charlie's Fist Bump Yeast" ;
                                     skos:definition "Previously called WLP862 Cry Havoc Lager Yeast, this strain is licensed from Charlie Papazian and can ferment at both ale and lager temperatures, allowing brewers to produce diverse beer styles. The recipes in both Papazian’s books, \"The Complete Joy of Homebrewing,\" \"The Homebrewer’s Companion,\" and \"Microbrewed Adventures\" were originally developed and brewed with this yeast." ;
                                     skos:prefLabel "WLP1983 Charlie's Fist Bump Yeast" .


###  http://peterbrau.com/whitelabs/yeast-bank/wlp300-hefeweizen-ale-yeast
wlp:wlp300-hefeweizen-ale-yeast rdf:type owl:NamedIndividual ,
                                         yeast:BrewersYeast ;
                                yeast:hasAlcoholTolerance "Medium (5 - 10%)" ;
                                yeast:hasFlocculation "Low" ;
                                yeast:hasHighAttenuation 76.00 ;
                                yeast:hasHighOptimumFermentationTemperature 72.00 ;
                                yeast:hasLowAttenuation 72.00 ;
                                yeast:hasLowOptimumFermentationTemperature 68.00 ;
                                yeast:usedForBrewingStyle beertype:hefeweizen ,
                                                          beertype:specialty-belgian ;
                                dcterms:bibliographicCitation "http://www.whitelabs.com/yeast-bank/wlp300-hefeweizen-ale-yeast" ;
                                gr:hasMPN "wlp300" ;
                                rdfs:label "WLP300 Hefeweizen Ale Yeast " ;
                                skos:definition "This popular German strain is used in the production of traditional, authentic hefeweizen. It produces a high level of isoamyl acetate, giving the resulting beer notes of banana. With balanced phenol production, this strain produces notes of clove but remains banana forward. Low flocculation leaves the desired cloudy look, appropriate for the German wheat beer style." ;
                                skos:prefLabel "WLP300 Hefeweizen Ale Yeast " .


###  http://peterbrau.com/whitelabs/yeast-bank/wlp320-american-hefeweizen-ale-yeast
wlp:wlp320-american-hefeweizen-ale-yeast rdf:type owl:NamedIndividual ,
                                                  yeast:BrewersYeast ;
                                         yeast:hasAlcoholTolerance "Medium (5 - 10%)" ;
                                         yeast:hasFlocculation "Low" ;
                                         yeast:hasHighAttenuation 75.00 ;
                                         yeast:hasHighOptimumFermentationTemperature 69.00 ;
                                         yeast:hasLowAttenuation 70.00 ;
                                         yeast:hasLowOptimumFermentationTemperature 65.00 ;
                                         yeast:usedForBrewingStyle beertype:american-wheat-ale ,
                                                                   beertype:specialty-belgian ;
                                         dcterms:bibliographicCitation "http://www.whitelabs.com/yeast-bank/wlp320-american-hefeweizen-ale-yeast" ;
                                         gr:hasMPN "wlp320" ;
                                         rdfs:label "WLP320 American Hefeweizen Ale Yeast" ;
                                         skos:definition "This strain ferments much cleaner than it’s hefeweizen strain counterparts. It produces very slight banana and clove notes and has low flocculation, leaving resulting beers with characteristic cloudiness." ;
                                         skos:prefLabel "WLP320 American Hefeweizen Ale Yeast" .


###  http://peterbrau.com/whitelabs/yeast-bank/wlp351-bavarian-weizen-yeast
wlp:wlp351-bavarian-weizen-yeast rdf:type owl:NamedIndividual ,
                                          yeast:BrewersYeast ;
                                 yeast:hasAlcoholTolerance "Medium (5 - 10%)" ;
                                 yeast:hasFlocculation "Low" ;
                                 yeast:hasHighAttenuation 77.00 ;
                                 yeast:hasHighOptimumFermentationTemperature 70.00 ;
                                 yeast:hasLowAttenuation 73.00 ;
                                 yeast:hasLowOptimumFermentationTemperature 66.00 ;
                                 yeast:usedForBrewingStyle beertype:belgian-wit ,
                                                           beertype:hefeweizen ,
                                                           beertype:specialty-belgian ;
                                 dcterms:bibliographicCitation "http://www.whitelabs.com/yeast-bank/wlp351-bavarian-weizen-yeast" ;
                                 gr:hasMPN "wlp351" ;
                                 rdfs:label "WLP351 Bavarian Weizen Yeast" ;
                                 skos:definition "This is former Yeast Lab W51, the description originally used by Yeast Lab still fits: “This strain produces a classic German-style wheat beer, with medium to high spicy phenolic overtones reminiscent of cloves.”" ;
                                 skos:prefLabel "WLP351 Bavarian Weizen Yeast" .


###  http://peterbrau.com/whitelabs/yeast-bank/wlp380-hefeweizen-iv-ale-yeast
wlp:wlp380-hefeweizen-iv-ale-yeast rdf:type owl:NamedIndividual ,
                                            yeast:BrewersYeast ;
                                   yeast:hasAlcoholTolerance "Medium (5 - 10%)" ;
                                   yeast:hasFlocculation "Low" ;
                                   yeast:hasHighAttenuation 80.00 ;
                                   yeast:hasHighOptimumFermentationTemperature 70.00 ;
                                   yeast:hasLowAttenuation 73.00 ;
                                   yeast:hasLowOptimumFermentationTemperature 66.00 ;
                                   yeast:usedForBrewingStyle beertype:belgian-wit ,
                                                             beertype:hefeweizen ,
                                                             beertype:specialty-belgian ;
                                   dcterms:bibliographicCitation "http://www.whitelabs.com/yeast-bank/wlp380-hefeweizen-iv-ale-yeast" ;
                                   gr:hasMPN "wlp380" ;
                                   rdfs:label "WLP380 Hefeweizen IV Ale Yeast" ;
                                   skos:definition "This strain produces a balance of phenolics and esters. Nutmeg, clove, and spice are more dominant than the banana and bubble gum aroma. Pitching rate and temperature will dramatically affect the flavor and aroma of this strain. Traditional brewing techniques suggest underpitching to produce more classic characteristics of the style. This strain has low flocculation and minor sulfur production." ;
                                   skos:prefLabel "WLP380 Hefeweizen IV Ale Yeast" .


###  http://peterbrau.com/whitelabs/yeast-bank/wlp400-belgian-wit-ale-yeast
wlp:wlp400-belgian-wit-ale-yeast rdf:type owl:NamedIndividual ,
                                          yeast:BrewersYeast ;
                                 yeast:hasAlcoholTolerance "Medium (5 - 10%)" ;
                                 yeast:hasFlocculation "Medium to Low" ;
                                 yeast:hasHighAttenuation 78.00 ;
                                 yeast:hasHighOptimumFermentationTemperature 74.00 ;
                                 yeast:hasLowAttenuation 74.00 ;
                                 yeast:hasLowOptimumFermentationTemperature 67.00 ;
                                 yeast:usedForBrewingStyle beertype:belgian-blond ,
                                                           beertype:belgian-dark-strong-ale ,
                                                           beertype:belgian-table-bier ,
                                                           beertype:belgian-wit ,
                                                           beertype:biere-de-garde ,
                                                           beertype:dubbel ,
                                                           beertype:hefeweizen ,
                                                           beertype:saison ,
                                                           beertype:specialty-belgian ,
                                                           beertype:tripel ;
                                 dcterms:bibliographicCitation "http://www.whitelabs.com/yeast-bank/wlp400-belgian-wit-ale-yeast" ;
                                 gr:hasMPN "wlp400" ;
                                 rdfs:label "WLP400 Belgian Wit Ale Yeast" ;
                                 skos:definition "This strain is the pinnacle yeast for Belgian witbiers or white ales. High phenol production contributes an herbal aroma and flavor notes which blends well with herb and fruit adjuncts. Expect nearly 80% attenuation and a slightly lower resulting pH than English or American ale strains creating a dry beer." ;
                                 skos:prefLabel "WLP400 Belgian Wit Ale Yeast" .


###  http://peterbrau.com/whitelabs/yeast-bank/wlp410-belgian-wit-ii-ale-yeast
wlp:wlp410-belgian-wit-ii-ale-yeast rdf:type owl:NamedIndividual ,
                                             yeast:BrewersYeast ;
                                    yeast:hasAlcoholTolerance "Medium (5 - 10%)" ;
                                    yeast:hasFlocculation "Medium to Low" ;
                                    yeast:hasHighAttenuation 75.00 ;
                                    yeast:hasHighOptimumFermentationTemperature 74.00 ;
                                    yeast:hasLowAttenuation 70.00 ;
                                    yeast:hasLowOptimumFermentationTemperature 67.00 ;
                                    yeast:usedForBrewingStyle beertype:belgian-blond ,
                                                              beertype:belgian-dark-strong-ale ,
                                                              beertype:belgian-table-bier ,
                                                              beertype:belgian-wit ,
                                                              beertype:biere-de-garde ,
                                                              beertype:dubbel ,
                                                              beertype:hefeweizen ,
                                                              beertype:saison ,
                                                              beertype:specialty-belgian ,
                                                              beertype:tripel ;
                                    dcterms:bibliographicCitation "http://www.whitelabs.com/yeast-bank/wlp410-belgian-wit-ii-ale-yeast" ;
                                    gr:hasMPN "wlp410" ;
                                    rdfs:label "WLP410 Belgian Wit II Ale Yeast" ;
                                    skos:definition "A fairly clean strain with medium intensity and spice-like phenol production. With up to 75% attenuation, this strain produces a residual malt character. It helps balance any adjuncts resulting in increased drinkability. Slightly lower resulting pH than English or American ale strains, it creates a slightly tart refreshing beer. This strain is ideal for witbiers or Belgian table beers." ;
                                    skos:prefLabel "WLP410 Belgian Wit II Ale Yeast" .


###  http://peterbrau.com/whitelabs/yeast-bank/wlp500-monastery-ale-yeast
wlp:wlp500-monastery-ale-yeast rdf:type owl:NamedIndividual ,
                                        yeast:BrewersYeast ;
                               yeast:hasAlcoholTolerance "High (10 - 15%)" ;
                               yeast:hasFlocculation "Medium to Low" ;
                               yeast:hasHighAttenuation 80.00 ;
                               yeast:hasHighOptimumFermentationTemperature 72.00 ;
                               yeast:hasLowAttenuation 75.00 ;
                               yeast:hasLowOptimumFermentationTemperature 65.00 ;
                               yeast:usedForBrewingStyle beertype:belgian-blond ,
                                                         beertype:belgian-dark-strong-ale ,
                                                         beertype:belgian-table-bier ,
                                                         beertype:belgian-wit ,
                                                         beertype:biere-de-garde ,
                                                         beertype:dubbel ,
                                                         beertype:saison ,
                                                         beertype:specialty-belgian ,
                                                         beertype:tripel ;
                               dcterms:bibliographicCitation "http://www.whitelabs.com/yeast-bank/wlp500-monastery-ale-yeast" ;
                               gr:hasMPN "wlp500" ;
                               rdfs:label "WLP500 Monastery Ale Yeast" ;
                               skos:definition "Sourced from a Belgian monastery, this strain is ideal for Belgian quads, trippels and dubbels due to its high alcohol tolerance. It produces characteristic notes of plum and cherry with a hint of bubble gum. Lower fermentation temperatures (65-67°F/18-19°C) result in less fruity and more earthy beers." ;
                               skos:prefLabel "WLP500 Monastery Ale Yeast" .


###  http://peterbrau.com/whitelabs/yeast-bank/wlp510-bastogne-belgian-ale-yeast
wlp:wlp510-bastogne-belgian-ale-yeast rdf:type owl:NamedIndividual ,
                                               yeast:BrewersYeast ;
                                      yeast:hasAlcoholTolerance "High (10 - 15%)" ;
                                      yeast:hasFlocculation "Medium" ;
                                      yeast:hasHighAttenuation 80.00 ;
                                      yeast:hasHighOptimumFermentationTemperature 72.00 ;
                                      yeast:hasLowAttenuation 74.00 ;
                                      yeast:hasLowOptimumFermentationTemperature 66.00 ;
                                      yeast:usedForBrewingStyle beertype:belgian-table-bier ,
                                                                beertype:dubbel ,
                                                                beertype:specialty-belgian ,
                                                                beertype:tripel ;
                                      dcterms:bibliographicCitation "http://www.whitelabs.com/yeast-bank/wlp510-bastogne-belgian-ale-yeast" ;
                                      gr:hasMPN "wlp510" ;
                                      rdfs:label "WLP510 Bastogne Belgian Ale Yeast" ;
                                      skos:definition "A high-gravity ale yeast that produces a dry beer with a slightly acidic finish. While fruit forward, this strain is mild on spice-like phenols. With a high alcohol tolerance upwards of 15% ABV, this strain is great for any Belgian styles ranging from a table beer to a dark strong ale." ;
                                      skos:prefLabel "WLP510 Bastogne Belgian Ale Yeast" .


###  http://peterbrau.com/whitelabs/yeast-bank/wlp515-antwerp-ale-yeast
wlp:wlp515-antwerp-ale-yeast rdf:type owl:NamedIndividual ,
                                      yeast:BrewersYeast ;
                             yeast:hasAlcoholTolerance "Medium (5 - 10%)" ;
                             yeast:hasFlocculation "Medium" ;
                             yeast:hasHighAttenuation 80.00 ;
                             yeast:hasHighOptimumFermentationTemperature 70.00 ;
                             yeast:hasLowAttenuation 73.00 ;
                             yeast:hasLowOptimumFermentationTemperature 67.00 ;
                             yeast:usedForBrewingStyle beertype:belgian-table-bier ,
                                                       beertype:belgian-wit ,
                                                       beertype:biere-de-garde ,
                                                       beertype:specialty-belgian ;
                             dcterms:bibliographicCitation "http://www.whitelabs.com/yeast-bank/wlp515-antwerp-ale-yeast" ;
                             gr:hasMPN "wlp515" ;
                             rdfs:label "WLP515 Antwerp Ale Yeast" ;
                             skos:definition "Clean, almost lager like Belgian type ale yeast. Good for Belgian type pales ales and amber ales, or with blends to combine with other Belgian type yeast strains. Biscuity, ale like aroma present. Hop flavors and bitterness are accentuated. Slight sulfur will be produced during fermentation, which can give the yeast a lager-like flavor profile." ;
                             skos:prefLabel "WLP515 Antwerp Ale Yeast" .


###  http://peterbrau.com/whitelabs/yeast-bank/wlp518-opshaug-kveik-ale-yeast
wlp:wlp518-opshaug-kveik-ale-yeast rdf:type owl:NamedIndividual ,
                                            yeast:BrewersYeast ;
                                   yeast:hasAlcoholTolerance "Medium - High (8 - 12%)" ;
                                   yeast:hasFlocculation "Medium to High" ;
                                   yeast:hasHighAttenuation 80.00 ;
                                   yeast:hasHighOptimumFermentationTemperature 86.00 ;
                                   yeast:hasLowAttenuation 70.00 ;
                                   yeast:hasLowOptimumFermentationTemperature 77.00 ;
                                   yeast:usedForBrewingStyle beertype:american-india-pale-ale ,
                                                             beertype:american-pale-ale ,
                                                             beertype:imperial-india-pale-ale ,
                                                             beertype:saison ,
                                                             beertype:specialty-belgian ;
                                   dcterms:bibliographicCitation "http://www.whitelabs.com/yeast-bank/wlp518-opshaug-kveik-ale-yeast" ;
                                   gr:hasMPN "wlp518" ;
                                   rdfs:label "WLP518 Opshaug Kveik Ale Yeast" ;
                                   skos:definition "None" ;
                                   skos:prefLabel "WLP518 Opshaug Kveik Ale Yeast" .


###  http://peterbrau.com/whitelabs/yeast-bank/wlp530-abbey-ale-yeast
wlp:wlp530-abbey-ale-yeast rdf:type owl:NamedIndividual ,
                                    yeast:BrewersYeast ;
                           yeast:hasAlcoholTolerance "High (10 - 15%)" ;
                           yeast:hasFlocculation "Medium to High" ;
                           yeast:hasHighAttenuation 80.00 ;
                           yeast:hasHighOptimumFermentationTemperature 72.00 ;
                           yeast:hasLowAttenuation 75.00 ;
                           yeast:hasLowOptimumFermentationTemperature 66.00 ;
                           yeast:usedForBrewingStyle beertype:belgian-blond ,
                                                     beertype:belgian-dark-strong-ale ,
                                                     beertype:belgian-table-bier ,
                                                     beertype:belgian-wit ,
                                                     beertype:biere-de-garde ,
                                                     beertype:dubbel ,
                                                     beertype:saison ,
                                                     beertype:specialty-belgian ,
                                                     beertype:tripel ;
                           dcterms:bibliographicCitation "http://www.whitelabs.com/yeast-bank/wlp530-abbey-ale-yeast" ;
                           gr:hasMPN "wlp530" ;
                           rdfs:label "WLP530 Abbey Ale Yeast" ;
                           skos:definition "This is a traditional Belgian abbey strain perfect for use in dubbels, tripels and Belgian strong ales due to its very high alcohol tolerance of up to 15% ABV. Produces cherry, plum and pear esters. Medium flocculation results in clear, drinkable beer." ;
                           skos:prefLabel "WLP530 Abbey Ale Yeast" .


###  http://peterbrau.com/whitelabs/yeast-bank/wlp540-abbey-iv-ale-yeast
wlp:wlp540-abbey-iv-ale-yeast rdf:type owl:NamedIndividual ,
                                       yeast:BrewersYeast ;
                              yeast:hasAlcoholTolerance "High (10 - 15%)" ;
                              yeast:hasFlocculation "Medium" ;
                              yeast:hasHighAttenuation 82.00 ;
                              yeast:hasHighOptimumFermentationTemperature 72.00 ;
                              yeast:hasLowAttenuation 74.00 ;
                              yeast:hasLowOptimumFermentationTemperature 66.00 ;
                              yeast:usedForBrewingStyle beertype:belgian-table-bier ,
                                                        beertype:biere-de-garde ,
                                                        beertype:dubbel ,
                                                        beertype:saison ,
                                                        beertype:specialty-belgian ,
                                                        beertype:tripel ;
                              dcterms:bibliographicCitation "http://www.whitelabs.com/yeast-bank/wlp540-abbey-iv-ale-yeast" ;
                              gr:hasMPN "wlp540" ;
                              rdfs:label "WLP540 Abbey IV Ale Yeast" ;
                              skos:definition "This strain produces balanced fruit aroma and flavor characters. It is ideal for abbey-style beers including dubbels, trippels and Belgian strong ales." ;
                              skos:prefLabel "WLP540 Abbey IV Ale Yeast" .


###  http://peterbrau.com/whitelabs/yeast-bank/wlp545-belgian-strong-ale-yeast
wlp:wlp545-belgian-strong-ale-yeast rdf:type owl:NamedIndividual ,
                                             yeast:BrewersYeast ;
                                    yeast:hasAlcoholTolerance "High (10 - 15%)" ;
                                    yeast:hasFlocculation "Medium" ;
                                    yeast:hasHighAttenuation 85.00 ;
                                    yeast:hasHighOptimumFermentationTemperature 72.00 ;
                                    yeast:hasLowAttenuation 78.00 ;
                                    yeast:hasLowOptimumFermentationTemperature 66.00 ;
                                    yeast:usedForBrewingStyle beertype:belgian-blond ,
                                                              beertype:belgian-dark-strong-ale ,
                                                              beertype:belgian-table-bier ,
                                                              beertype:biere-de-garde ,
                                                              beertype:dubbel ,
                                                              beertype:saison ,
                                                              beertype:specialty-belgian ,
                                                              beertype:tripel ;
                                    dcterms:bibliographicCitation "http://www.whitelabs.com/yeast-bank/wlp545-belgian-strong-ale-yeast" ;
                                    gr:hasMPN "wlp545" ;
                                    rdfs:label "WLP545 Belgian Strong Ale Yeast" ;
                                    skos:definition "From the Ardennes region of Belgium, this classic yeast strain produces moderate levels of ester and phenolic characters, often described as dried sage and black cracked pepper. High attenuation results in a dry finish ideal for high gravity beers. This strain is recommended for dark strong ales, abbey ales and seasonal specialties like Belgian holiday ales." ;
                                    skos:prefLabel "WLP545 Belgian Strong Ale Yeast" .


###  http://peterbrau.com/whitelabs/yeast-bank/wlp546-mara-n-canyon-wild-cacao
wlp:wlp546-mara-n-canyon-wild-cacao rdf:type owl:NamedIndividual ,
                                             yeast:BrewersYeast ;
                                    yeast:hasAlcoholTolerance "Medium (5 - 10%)" ;
                                    yeast:hasFlocculation "Low" ;
                                    yeast:hasHighAttenuation 70.00 ;
                                    yeast:hasHighOptimumFermentationTemperature 75.00 ;
                                    yeast:hasLowAttenuation 65.00 ;
                                    yeast:hasLowOptimumFermentationTemperature 65.00 ;
                                    yeast:usedForBrewingStyle beertype:saison ,
                                                              beertype:specialty-belgian ;
                                    dcterms:bibliographicCitation "http://www.whitelabs.com/yeast-bank/wlp546-mara-n-canyon-wild-cacao" ;
                                    gr:hasMPN "wlp546" ;
                                    rdfs:label "WLP546 Marañón Canyon Wild Cacao" ;
                                    skos:definition "This yeast was isolated from the thought to be extinct Pure Nacional variety of cacao. In 2007, this rare variety with white beans was rediscovered in the remote Marañón River Canyon in Peru. The fruity, phenolic, and wild-like characteristics of this strain make it an ideal choice for farmhouse and saison-style beers." ;
                                    skos:prefLabel "WLP546 Marañón Canyon Wild Cacao" .


###  http://peterbrau.com/whitelabs/yeast-bank/wlp550-belgian-ale-yeast
wlp:wlp550-belgian-ale-yeast rdf:type owl:NamedIndividual ,
                                      yeast:BrewersYeast ;
                             yeast:hasAlcoholTolerance "Medium - High (8 - 12%)" ;
                             yeast:hasFlocculation "Medium" ;
                             yeast:hasHighAttenuation 85.00 ;
                             yeast:hasHighOptimumFermentationTemperature 78.00 ;
                             yeast:hasLowAttenuation 78.00 ;
                             yeast:hasLowOptimumFermentationTemperature 68.00 ;
                             yeast:usedForBrewingStyle beertype:belgian-blond ,
                                                       beertype:belgian-dark-strong-ale ,
                                                       beertype:belgian-table-bier ,
                                                       beertype:belgian-wit ,
                                                       beertype:biere-de-garde ,
                                                       beertype:dubbel ,
                                                       beertype:saison ,
                                                       beertype:specialty-belgian ,
                                                       beertype:tripel ;
                             dcterms:bibliographicCitation "http://www.whitelabs.com/yeast-bank/wlp550-belgian-ale-yeast" ;
                             gr:hasMPN "wlp550" ;
                             rdfs:label "WLP550 Belgian Ale Yeast" ;
                             skos:definition "This very expressive strain produces phenol forward flavors and aromas reminiscent of clove, allspice and peppercorns. It has medium to high alcohol tolerance and is ideal for many classic Belgian styles including saisons, witbiers, blondes and browns." ;
                             skos:prefLabel "WLP550 Belgian Ale Yeast" .


###  http://peterbrau.com/whitelabs/yeast-bank/wlp564-leeuwenhoek-saison-yeast-blend
wlp:wlp564-leeuwenhoek-saison-yeast-blend rdf:type owl:NamedIndividual ,
                                                   yeast:BrewersYeast ;
                                          yeast:hasAlcoholTolerance "High (10 - 15%)" ;
                                          yeast:hasFlocculation "Low" ;
                                          yeast:hasHighAttenuation 82.00 ;
                                          yeast:hasHighOptimumFermentationTemperature 75.00 ;
                                          yeast:hasLowAttenuation 76.00 ;
                                          yeast:hasLowOptimumFermentationTemperature 66.00 ;
                                          yeast:usedForBrewingStyle beertype:belgian-table-bier ,
                                                                    beertype:belgian-wit ,
                                                                    beertype:saison ,
                                                                    beertype:specialty-belgian ,
                                                                    beertype:tripel ;
                                          dcterms:bibliographicCitation "http://www.whitelabs.com/yeast-bank/wlp564-leeuwenhoek-saison-yeast-blend" ;
                                          gr:hasMPN "wlp564" ;
                                          rdfs:label "WLP564 Leeuwenhoek Saison Yeast Blend" ;
                                          skos:definition "A blend of two saison strains and a low phenolic Belgian strain, developed for the White Labs in-house saisons. Approximately 85% attenuation which makes for a dryer saison. The strain proved very versatile, creating spicy, dry and clean beers." ;
                                          skos:prefLabel "WLP564 Leeuwenhoek Saison Yeast Blend" .


###  http://peterbrau.com/whitelabs/yeast-bank/wlp565-belgian-saison-i-yeast
wlp:wlp565-belgian-saison-i-yeast rdf:type owl:NamedIndividual ,
                                           yeast:BrewersYeast ;
                                  yeast:hasAlcoholTolerance "Medium (5 - 10%)" ;
                                  yeast:hasFlocculation "Medium" ;
                                  yeast:hasHighAttenuation 75.00 ;
                                  yeast:hasHighOptimumFermentationTemperature 75.00 ;
                                  yeast:hasLowAttenuation 65.00 ;
                                  yeast:hasLowOptimumFermentationTemperature 68.00 ;
                                  yeast:usedForBrewingStyle beertype:belgian-blond ,
                                                            beertype:belgian-dark-strong-ale ,
                                                            beertype:belgian-table-bier ,
                                                            beertype:belgian-wit ,
                                                            beertype:biere-de-garde ,
                                                            beertype:dubbel ,
                                                            beertype:saison ,
                                                            beertype:specialty-belgian ,
                                                            beertype:tripel ;
                                  dcterms:bibliographicCitation "http://www.whitelabs.com/yeast-bank/wlp565-belgian-saison-i-yeast" ;
                                  gr:hasMPN "wlp565" ;
                                  rdfs:label "WLP565 Belgian Saison I Yeast " ;
                                  skos:definition "A classic saison strain sourced from the Wallonia region of Belgium. This strain makes a classic saison by producing flavors and aromas noted as earthy, peppery and spicy. With attenuation averaging around 70 to 75%, some malt flavor will remain present. For best fermentation results, let this strain free-rise to allow for complete attenuation and production of the subtle, traditional aroma characteristics. With high gravity saisons, it’s suggested to dry the beer with an alternate yeast (such as WLP001 California Ale Yeast®) added after 50 to 60% fermentation." ;
                                  skos:prefLabel "WLP565 Belgian Saison I Yeast " .


###  http://peterbrau.com/whitelabs/yeast-bank/wlp566-belgian-saison-ii-ale-yeast
wlp:wlp566-belgian-saison-ii-ale-yeast rdf:type owl:NamedIndividual ,
                                                yeast:BrewersYeast ;
                                       yeast:hasAlcoholTolerance "Medium (5 - 10%)" ;
                                       yeast:hasFlocculation "Medium" ;
                                       yeast:hasHighAttenuation 85.00 ;
                                       yeast:hasHighOptimumFermentationTemperature 78.00 ;
                                       yeast:hasLowAttenuation 78.00 ;
                                       yeast:hasLowOptimumFermentationTemperature 68.00 ;
                                       yeast:usedForBrewingStyle beertype:belgian-blond ,
                                                                 beertype:belgian-dark-strong-ale ,
                                                                 beertype:belgian-table-bier ,
                                                                 beertype:belgian-wit ,
                                                                 beertype:biere-de-garde ,
                                                                 beertype:dubbel ,
                                                                 beertype:saison ,
                                                                 beertype:specialty-belgian ,
                                                                 beertype:tripel ;
                                       dcterms:bibliographicCitation "http://www.whitelabs.com/yeast-bank/wlp566-belgian-saison-ii-ale-yeast" ;
                                       gr:hasMPN "wlp566" ;
                                       rdfs:label "WLP566 Belgian Saison II Ale Yeast " ;
                                       skos:definition "This strain is a moderate phenol producer with clove-like flavor and aromatic notes present in finished beer. Some fruit-forward ester production provides a balance between fruit and spice aroma and flavors. This strain ferments and flocculates well, making it an easy-to-use option for saison and farmhouse ales." ;
                                       skos:prefLabel "WLP566 Belgian Saison II Ale Yeast " .


###  http://peterbrau.com/whitelabs/yeast-bank/wlp568-belgian-style-saison-ale-yeast-blend
wlp:wlp568-belgian-style-saison-ale-yeast-blend rdf:type owl:NamedIndividual ,
                                                         yeast:BrewersYeast ;
                                                yeast:hasAlcoholTolerance "Medium (5 - 10%)" ;
                                                yeast:hasFlocculation "Medium" ;
                                                yeast:hasHighAttenuation 80.00 ;
                                                yeast:hasHighOptimumFermentationTemperature 80.00 ;
                                                yeast:hasLowAttenuation 70.00 ;
                                                yeast:hasLowOptimumFermentationTemperature 70.00 ;
                                                yeast:usedForBrewingStyle beertype:belgian-blond ,
                                                                          beertype:belgian-dark-strong-ale ,
                                                                          beertype:belgian-table-bier ,
                                                                          beertype:belgian-wit ,
                                                                          beertype:biere-de-garde ,
                                                                          beertype:dubbel ,
                                                                          beertype:saison ,
                                                                          beertype:specialty-belgian ,
                                                                          beertype:tripel ;
                                                dcterms:bibliographicCitation "http://www.whitelabs.com/yeast-bank/wlp568-belgian-style-saison-ale-yeast-blend" ;
                                                gr:hasMPN "wlp568" ;
                                                rdfs:label "WLP568 Belgian Style Saison Ale Yeast Blend" ;
                                                skos:definition "This blend incorporates multiple Belgian and saison strains to produce pear-like esters backed by spicy, earthy and clove-like flavors and aromas. The cultures encourage complete fermentation in a timely manner and create harmony and complexity throughout its ester and phenol production." ;
                                                skos:prefLabel "WLP568 Belgian Style Saison Ale Yeast Blend" .


###  http://peterbrau.com/whitelabs/yeast-bank/wlp570-belgian-golden-ale-yeast
wlp:wlp570-belgian-golden-ale-yeast rdf:type owl:NamedIndividual ,
                                             yeast:BrewersYeast ;
                                    yeast:hasAlcoholTolerance "High (10 - 15%)" ;
                                    yeast:hasFlocculation "Low" ;
                                    yeast:hasHighAttenuation 78.00 ;
                                    yeast:hasHighOptimumFermentationTemperature 75.00 ;
                                    yeast:hasLowAttenuation 73.00 ;
                                    yeast:hasLowOptimumFermentationTemperature 68.00 ;
                                    yeast:usedForBrewingStyle beertype:belgian-blond ,
                                                              beertype:belgian-dark-strong-ale ,
                                                              beertype:belgian-table-bier ,
                                                              beertype:belgian-wit ,
                                                              beertype:biere-de-garde ,
                                                              beertype:dubbel ,
                                                              beertype:saison ,
                                                              beertype:specialty-belgian ,
                                                              beertype:tripel ;
                                    dcterms:bibliographicCitation "http://www.whitelabs.com/yeast-bank/wlp570-belgian-golden-ale-yeast" ;
                                    gr:hasMPN "wlp570" ;
                                    rdfs:label "WLP570 Belgian Golden Ale Yeast" ;
                                    skos:definition "From East Flanders, this yeast is versatile in that it can produce low to high gravity Belgian beers up to 12% ABV. A combination of fruitiness and phenolic characteristics dominate the flavor profile. Some sulfur is produced during fermentation, which will dissipate following the end of fermentation." ;
                                    skos:prefLabel "WLP570 Belgian Golden Ale Yeast" .


###  http://peterbrau.com/whitelabs/yeast-bank/wlp575-belgian-style-ale-yeast-blend
wlp:wlp575-belgian-style-ale-yeast-blend rdf:type owl:NamedIndividual ,
                                                  yeast:BrewersYeast ;
                                         yeast:hasAlcoholTolerance "Medium - High (8 - 12%)" ;
                                         yeast:hasFlocculation "Medium" ;
                                         yeast:hasHighAttenuation 80.00 ;
                                         yeast:hasHighOptimumFermentationTemperature 75.00 ;
                                         yeast:hasLowAttenuation 74.00 ;
                                         yeast:hasLowOptimumFermentationTemperature 68.00 ;
                                         yeast:usedForBrewingStyle beertype:belgian-blond ,
                                                                   beertype:belgian-dark-strong-ale ,
                                                                   beertype:belgian-table-bier ,
                                                                   beertype:belgian-wit ,
                                                                   beertype:biere-de-garde ,
                                                                   beertype:dubbel ,
                                                                   beertype:saison ,
                                                                   beertype:specialty-belgian ,
                                                                   beertype:tripel ;
                                         dcterms:bibliographicCitation "http://www.whitelabs.com/yeast-bank/wlp575-belgian-style-ale-yeast-blend" ;
                                         gr:hasMPN "wlp575" ;
                                         rdfs:label "WLP575 Belgian Style Ale Yeast Blend " ;
                                         skos:definition "A blend of two monastery-type yeast strains and one Belgian ale-type yeast. This blend creates a versatile culture which can be used for monastery-style beers or a myriad of American-Belgian style beers." ;
                                         skos:prefLabel "WLP575 Belgian Style Ale Yeast Blend " .


###  http://peterbrau.com/whitelabs/yeast-bank/wlp590-french-saison-ale-yeast
wlp:wlp590-french-saison-ale-yeast rdf:type owl:NamedIndividual ,
                                            yeast:BrewersYeast ;
                                   yeast:hasAlcoholTolerance "Medium (5 - 10%)" ;
                                   yeast:hasFlocculation "Medium" ;
                                   yeast:hasHighAttenuation 80.00 ;
                                   yeast:hasHighOptimumFermentationTemperature 75.00 ;
                                   yeast:hasLowAttenuation 73.00 ;
                                   yeast:hasLowOptimumFermentationTemperature 69.00 ;
                                   yeast:usedForBrewingStyle beertype:belgian-dark-strong-ale ,
                                                             beertype:belgian-table-bier ,
                                                             beertype:belgian-wit ,
                                                             beertype:french-cider ,
                                                             beertype:new-england-cider ,
                                                             beertype:saison ,
                                                             beertype:specialty-belgian ,
                                                             beertype:sweet-cider ,
                                                             beertype:traditional-perry ;
                                   dcterms:bibliographicCitation "http://www.whitelabs.com/yeast-bank/wlp590-french-saison-ale-yeast" ;
                                   gr:hasMPN "wlp590" ;
                                   rdfs:label "WLP590 French Saison Ale Yeast" ;
                                   skos:definition "One of our most popular saison strains, it is great for farmhouse-style beers because it produces flavors and aromas of pear, apple and cracked pepper. This strain is a high attenuator producing a very dry and drinkable finishing beer." ;
                                   skos:prefLabel "WLP590 French Saison Ale Yeast" .


###  http://peterbrau.com/whitelabs/yeast-bank/wlp600-kombucha-scoby
wlp:wlp600-kombucha-scoby rdf:type owl:NamedIndividual ,
                                   yeast:BrewersYeast ;
                          yeast:hasFlocculation "N/A" ;
                          yeast:usedForBrewingStyle beertype:kombucha ,
                                                    beertype:kombucha-0 ;
                          dcterms:bibliographicCitation "http://www.whitelabs.com/yeast-bank/wlp600-kombucha-scoby" ;
                          gr:hasMPN "wlp600" ;
                          rdfs:label "WLP600 Kombucha SCOBY " ;
                          skos:definition "White Labs now offers WLP600 Kombucha SCOBY, a symbiotic culture of bacteria and yeast that is used for fermenting sweet tea into kombucha. White Labs’ SCOBY is free of food pathogens and has been genetically identified to know specially what yeast and bacteria are involved in the fermentation of kombucha. As we continue our genetic identification we will publish the data below. This SCOBY has medium acetic acid production and low alcohol production based on our recipe. The SCOBY diameter is 2.92 inches." ;
                          skos:prefLabel "WLP600 Kombucha SCOBY " .


###  http://peterbrau.com/whitelabs/yeast-bank/wlp603-torulaspora-delbrueckii
wlp:wlp603-torulaspora-delbrueckii rdf:type owl:NamedIndividual ,
                                            yeast:BrewersYeast ,
                                            yeast:WildYeastAndBacteria ;
                                   yeast:hasAlcoholTolerance "Medium (5 - 10%)" ;
                                   yeast:hasFlocculation "Medium to Low" ;
                                   yeast:hasHighAttenuation 50.00 ;
                                   yeast:hasHighOptimumFermentationTemperature 86.00 ;
                                   yeast:hasLowAttenuation 30.00 ;
                                   yeast:hasLowOptimumFermentationTemperature 50.00 ;
                                   yeast:usedForBrewingStyle beertype:cider ,
                                                             beertype:english-cider ,
                                                             beertype:gose ,
                                                             beertype:sauvignon-blanc ;
                                   dcterms:bibliographicCitation "http://www.whitelabs.com/yeast-bank/wlp603-torulaspora-delbrueckii" ;
                                   gr:hasMPN "wlp603" ;
                                   rdfs:label "WLP603 Torulaspora delbrueckii" ;
                                   skos:definition "None" ;
                                   skos:prefLabel "WLP603 Torulaspora delbrueckii" .


###  http://peterbrau.com/whitelabs/yeast-bank/wlp611-new-nordic-ale-yeast
wlp:wlp611-new-nordic-ale-yeast rdf:type owl:NamedIndividual ,
                                         yeast:BrewersYeast ;
                                yeast:hasAlcoholTolerance "Medium (5 - 10%)" ;
                                yeast:hasFlocculation "Medium to Low" ;
                                yeast:hasHighAttenuation 75.00 ;
                                yeast:hasLowAttenuation 65.00 ;
                                yeast:usedForBrewingStyle beertype:hefeweizen ,
                                                          beertype:saison ,
                                                          beertype:specialty-belgian ;
                                dcterms:bibliographicCitation "http://www.whitelabs.com/yeast-bank/wlp611-new-nordic-ale-yeast" ;
                                gr:hasMPN "wlp611" ;
                                rdfs:label "WLP611 New Nordic Ale Yeast" ;
                                skos:definition "None" ;
                                skos:prefLabel "WLP611 New Nordic Ale Yeast" .


###  http://peterbrau.com/whitelabs/yeast-bank/wlp616-funky-cider-blend
wlp:wlp616-funky-cider-blend rdf:type owl:NamedIndividual ,
                                      yeast:BrewersYeast ,
                                      yeast:WildYeastAndBacteria ;
                             yeast:usedForBrewingStyle beertype:cider ,
                                                       beertype:english-cider ,
                                                       beertype:gose ,
                                                       beertype:new-england-cider ;
                             dcterms:bibliographicCitation "http://www.whitelabs.com/yeast-bank/wlp616-funky-cider-blend" ;
                             gr:hasMPN "wlp616" ;
                             rdfs:label "WLP616 Funky Cider Blend" ;
                             skos:definition "None" ;
                             skos:prefLabel "WLP616 Funky Cider Blend" .


###  http://peterbrau.com/whitelabs/yeast-bank/wlp630-berliner-weisse-blend
wlp:wlp630-berliner-weisse-blend rdf:type owl:NamedIndividual ,
                                          yeast:BrewersYeast ,
                                          yeast:WildYeastAndBacteria ;
                                 yeast:hasAlcoholTolerance "Medium (5 - 10%)" ;
                                 yeast:hasFlocculation "Medium" ;
                                 yeast:hasHighAttenuation 80.00 ;
                                 yeast:hasHighOptimumFermentationTemperature 72.00 ;
                                 yeast:hasLowAttenuation 73.00 ;
                                 yeast:hasLowOptimumFermentationTemperature 68.00 ;
                                 yeast:usedForBrewingStyle beertype:berliner-weisse ,
                                                           beertype:gose ,
                                                           beertype:lambic ;
                                 dcterms:bibliographicCitation "http://www.whitelabs.com/yeast-bank/wlp630-berliner-weisse-blend" ;
                                 gr:hasMPN "wlp630" ;
                                 rdfs:label "WLP630 Berliner Weisse Blend" ;
                                 skos:definition "A blend of German weizen yeast and Lactobacillus bacteria to create a subtly tart, drinkable beer. This blend can take several months to develop tart character making it perfect for brewing a traditional Berliner Weisse." ;
                                 skos:prefLabel "WLP630 Berliner Weisse Blend" .


###  http://peterbrau.com/whitelabs/yeast-bank/wlp640-brettanomyces-anomalus
wlp:wlp640-brettanomyces-anomalus rdf:type owl:NamedIndividual ,
                                           yeast:BrewersYeast ,
                                           yeast:WildYeastAndBacteria ;
                                  yeast:hasAlcoholTolerance "Medium - High (8 - 12%)" ;
                                  yeast:hasFlocculation "Low" ;
                                  yeast:hasHighAttenuation 85.00 ;
                                  yeast:hasHighOptimumFermentationTemperature 85.00 ;
                                  yeast:hasLowAttenuation 70.00 ;
                                  yeast:hasLowOptimumFermentationTemperature 70.00 ;
                                  yeast:usedForBrewingStyle beertype:berliner-weisse ,
                                                            beertype:flanders-brown ,
                                                            beertype:flanders-red ,
                                                            beertype:geuze ,
                                                            beertype:lambic ;
                                  dcterms:bibliographicCitation "http://www.whitelabs.com/yeast-bank/wlp640-brettanomyces-anomalus" ;
                                  gr:hasMPN "wlp640" ;
                                  rdfs:label "WLP640 Brettanomyces anomalus" ;
                                  skos:definition "Typical barnyard funk character with some fruitiness. Acidity is medium. Primary fermentation can be done with this strain, but a starter may be necessary." ;
                                  skos:prefLabel "WLP640 Brettanomyces anomalus" .


###  http://peterbrau.com/whitelabs/yeast-bank/wlp644-saccharomyces-bruxellensis-trois
wlp:wlp644-saccharomyces-bruxellensis-trois rdf:type owl:NamedIndividual ,
                                                     yeast:BrewersYeast ,
                                                     yeast:WildYeastAndBacteria ;
                                            yeast:hasAlcoholTolerance "Medium - High (8 - 12%)" ;
                                            yeast:hasFlocculation "Low" ;
                                            yeast:hasHighAttenuation 85.00 ;
                                            yeast:hasHighOptimumFermentationTemperature 85.00 ;
                                            yeast:hasLowAttenuation 85.00 ;
                                            yeast:hasLowOptimumFermentationTemperature 70.00 ;
                                            yeast:usedForBrewingStyle beertype:flanders-brown ,
                                                                      beertype:flanders-red ,
                                                                      beertype:geuze ,
                                                                      beertype:gose ,
                                                                      beertype:lambic ;
                                            dcterms:bibliographicCitation "http://www.whitelabs.com/yeast-bank/wlp644-saccharomyces-bruxellensis-trois" ;
                                            gr:hasMPN "wlp644" ;
                                            rdfs:label "WLP644 Saccharomyces \"bruxellensis\" Trois" ;
                                            skos:definition "This Belgian strain, traditionally used for wild yeast fermentations, produces a slightly tart beer with delicate mango and pineapple characteristics. This wild yeast has grown in popularity for styles like American IPA, American pale and blonde ales due to its tropical and stone fruit flavors and aromas. This Saccharomyces strain can be used like other house strains and can be easily clean with proper CIP procedures." ;
                                            skos:prefLabel "WLP644 Saccharomyces \"bruxellensis\" Trois" .


###  http://peterbrau.com/whitelabs/yeast-bank/wlp645-brettanomyces-claussenii
wlp:wlp645-brettanomyces-claussenii rdf:type owl:NamedIndividual ,
                                             yeast:BrewersYeast ,
                                             yeast:WildYeastAndBacteria ;
                                    yeast:hasAlcoholTolerance "Medium - High (8 - 12%)" ;
                                    yeast:hasFlocculation "Low" ;
                                    yeast:hasHighAttenuation 85.00 ;
                                    yeast:hasHighOptimumFermentationTemperature 85.00 ;
                                    yeast:hasLowAttenuation 70.00 ;
                                    yeast:hasLowOptimumFermentationTemperature 85.00 ;
                                    yeast:usedForBrewingStyle beertype:berliner-weisse ,
                                                              beertype:flanders-brown ,
                                                              beertype:flanders-red ,
                                                              beertype:geuze ,
                                                              beertype:gose ,
                                                              beertype:lambic ;
                                    dcterms:bibliographicCitation "http://www.whitelabs.com/yeast-bank/wlp645-brettanomyces-claussenii" ;
                                    gr:hasMPN "wlp645" ;
                                    rdfs:label "WLP645 Brettanomyces claussenii" ;
                                    skos:definition "Originally isolated from strong English stock beer in the early 20th century, this yeast has low-intensity Brettanomyces character and is closely related to Brettanomyces anomalus. This strain produces fruity, pineapple-like aroma with an earthy hay-like background aroma and aroma note." ;
                                    skos:prefLabel "WLP645 Brettanomyces claussenii" .


###  http://peterbrau.com/whitelabs/yeast-bank/wlp648-brettanomyces-bruxellensis-trois-vrai
wlp:wlp648-brettanomyces-bruxellensis-trois-vrai rdf:type owl:NamedIndividual ,
                                                          yeast:BrewersYeast ,
                                                          yeast:WildYeastAndBacteria ;
                                                 yeast:hasAlcoholTolerance "Medium - High (8 - 12%)" ;
                                                 yeast:hasFlocculation "Low" ;
                                                 yeast:hasHighAttenuation 85.00 ;
                                                 yeast:hasHighOptimumFermentationTemperature 85.00 ;
                                                 yeast:hasLowAttenuation 85.00 ;
                                                 yeast:hasLowOptimumFermentationTemperature 70.00 ;
                                                 yeast:usedForBrewingStyle beertype:flanders-brown ,
                                                                           beertype:geuze ,
                                                                           beertype:gose ,
                                                                           beertype:lambic ;
                                                 dcterms:bibliographicCitation "http://www.whitelabs.com/yeast-bank/wlp648-brettanomyces-bruxellensis-trois-vrai" ;
                                                 gr:hasMPN "wlp648" ;
                                                 rdfs:label "WLP648 Brettanomyces bruxellensis Trois Vrai" ;
                                                 skos:definition "The vrai (“true” in French) Brettanomyces bruxellensis Trois. This infamous strain should be used for primary fermentations due to its ability to highly attenuate. It has a robust, complex sour character with aromas of pear." ;
                                                 skos:prefLabel "WLP648 Brettanomyces bruxellensis Trois Vrai" .


###  http://peterbrau.com/whitelabs/yeast-bank/wlp650-brettanomyces-bruxellensis
wlp:wlp650-brettanomyces-bruxellensis rdf:type owl:NamedIndividual ,
                                               yeast:BrewersYeast ,
                                               yeast:WildYeastAndBacteria ;
                                      yeast:hasAlcoholTolerance "Medium - High (8 - 12%)" ;
                                      yeast:hasFlocculation "Low" ;
                                      yeast:hasHighAttenuation 85.00 ;
                                      yeast:hasHighOptimumFermentationTemperature 85.00 ;
                                      yeast:hasLowAttenuation 85.00 ;
                                      yeast:hasLowOptimumFermentationTemperature 85.00 ;
                                      yeast:usedForBrewingStyle beertype:flanders-brown ,
                                                                beertype:flanders-red ,
                                                                beertype:geuze ,
                                                                beertype:gose ,
                                                                beertype:lambic ;
                                      dcterms:bibliographicCitation "http://www.whitelabs.com/yeast-bank/wlp650-brettanomyces-bruxellensis" ;
                                      gr:hasMPN "wlp650" ;
                                      rdfs:label "WLP650 Brettanomyces bruxellensis" ;
                                      skos:definition "A classic strain used for secondary fermentation in Belgian-style beers such as lambics. It creates a medium-intensity, earth-forward character in finished beer. A historic brewery in Belgium uses this yeast in secondary fermentation and bottling to produce the signature flavor of its beer." ;
                                      skos:prefLabel "WLP650 Brettanomyces bruxellensis" .


###  http://peterbrau.com/whitelabs/yeast-bank/wlp653-brettanomyces-lambicus
wlp:wlp653-brettanomyces-lambicus rdf:type owl:NamedIndividual ,
                                           yeast:BrewersYeast ,
                                           yeast:WildYeastAndBacteria ;
                                  yeast:hasAlcoholTolerance "Medium - High (8 - 12%)" ;
                                  yeast:hasFlocculation "Low" ;
                                  yeast:hasHighAttenuation 85.00 ;
                                  yeast:hasHighOptimumFermentationTemperature 85.00 ;
                                  yeast:hasLowAttenuation 70.00 ;
                                  yeast:hasLowOptimumFermentationTemperature 85.00 ;
                                  yeast:usedForBrewingStyle beertype:flanders-brown ,
                                                            beertype:flanders-red ,
                                                            beertype:geuze ,
                                                            beertype:gose ,
                                                            beertype:lambic ;
                                  dcterms:bibliographicCitation "http://www.whitelabs.com/yeast-bank/wlp653-brettanomyces-lambicus" ;
                                  gr:hasMPN "wlp653" ;
                                  rdfs:label "WLP653 Brettanomyces lambicus" ;
                                  skos:definition "None" ;
                                  skos:prefLabel "WLP653 Brettanomyces lambicus" .


###  http://peterbrau.com/whitelabs/yeast-bank/wlp655-belgian-sour-mix-1
wlp:wlp655-belgian-sour-mix-1 rdf:type owl:NamedIndividual ,
                                       yeast:BrewersYeast ,
                                       yeast:WildYeastAndBacteria ;
                              yeast:hasAlcoholTolerance "Medium - High (8 - 12%)" ;
                              yeast:hasFlocculation "Medium to Low" ;
                              yeast:hasHighAttenuation 80.00 ;
                              yeast:hasHighOptimumFermentationTemperature 85.00 ;
                              yeast:hasLowAttenuation 70.00 ;
                              yeast:hasLowOptimumFermentationTemperature 80.00 ;
                              yeast:usedForBrewingStyle beertype:berliner-weisse ,
                                                        beertype:flanders-brown ,
                                                        beertype:flanders-red ,
                                                        beertype:geuze ,
                                                        beertype:gose ,
                                                        beertype:lambic ;
                              dcterms:bibliographicCitation "http://www.whitelabs.com/yeast-bank/wlp655-belgian-sour-mix-1" ;
                              gr:hasMPN "wlp655" ;
                              rdfs:label "WLP655 Belgian Sour Mix 1" ;
                              skos:definition "A unique blend of Brettanomyces and Saccharomyces yeasts as well as bacterial strains Lactobacillus and Pediococcus. Perfect for duplicating traditional spontaneous fermentations similar to those found in Belgian-style ales." ;
                              skos:prefLabel "WLP655 Belgian Sour Mix 1" .


###  http://peterbrau.com/whitelabs/yeast-bank/wlp661-pediococcus-damnosus
wlp:wlp661-pediococcus-damnosus rdf:type owl:NamedIndividual ,
                                         yeast:BrewersYeast ,
                                         yeast:WildYeastAndBacteria ;
                                yeast:hasAlcoholTolerance "Medium - High (8 - 12%)" ;
                                yeast:hasFlocculation "Low" ;
                                yeast:hasHighAttenuation 0.00 ;
                                yeast:hasLowAttenuation 0.00 ;
                                yeast:usedForBrewingStyle beertype:flanders-brown ,
                                                          beertype:lambic ;
                                dcterms:bibliographicCitation "http://www.whitelabs.com/yeast-bank/wlp661-pediococcus-damnosus" ;
                                gr:hasMPN "wlp661" ;
                                rdfs:label "WLP661 Pediococcus damnosus" ;
                                skos:definition "Perfect for use in any sour program, this is a cocci bacteria known for its souring capabilities through the production of lactic acid. It is a high diacetyl producer and slow growing, so it’s suggested to use in a mixed culture." ;
                                skos:prefLabel "WLP661 Pediococcus damnosus" .


###  http://peterbrau.com/whitelabs/yeast-bank/wlp665-flemish-ale-blend
wlp:wlp665-flemish-ale-blend rdf:type owl:NamedIndividual ,
                                      yeast:BrewersYeast ,
                                      yeast:WildYeastAndBacteria ;
                             yeast:hasAlcoholTolerance "Medium - High (8 - 12%)" ;
                             yeast:hasFlocculation "Medium to Low" ;
                             yeast:hasHighAttenuation 85.00 ;
                             yeast:hasHighOptimumFermentationTemperature 80.00 ;
                             yeast:hasLowAttenuation 80.00 ;
                             yeast:hasLowOptimumFermentationTemperature 68.00 ;
                             yeast:usedForBrewingStyle beertype:flanders-brown ,
                                                       beertype:flanders-red ,
                                                       beertype:geuze ,
                                                       beertype:gose ,
                                                       beertype:lambic ,
                                                       beertype:vault-seasonal-release ;
                             dcterms:bibliographicCitation "http://www.whitelabs.com/yeast-bank/wlp665-flemish-ale-blend" ;
                             gr:hasMPN "wlp665" ;
                             rdfs:label "WLP665 Flemish Ale Blend" ;
                             skos:definition "None" ;
                             skos:prefLabel "WLP665 Flemish Ale Blend" .


###  http://peterbrau.com/whitelabs/yeast-bank/wlp669-lactobacillus-paracollinoides
wlp:wlp669-lactobacillus-paracollinoides rdf:type owl:NamedIndividual ,
                                                  yeast:BrewersYeast ,
                                                  yeast:WildYeastAndBacteria ;
                                         yeast:usedForBrewingStyle beertype:berliner-weisse ,
                                                                   beertype:flanders-brown ,
                                                                   beertype:flanders-red ,
                                                                   beertype:geuze ,
                                                                   beertype:gose ,
                                                                   beertype:lambic ;
                                         dcterms:bibliographicCitation "http://www.whitelabs.com/yeast-bank/wlp669-lactobacillus-paracollinoides" ;
                                         gr:hasMPN "wlp669" ;
                                         rdfs:label "WLP669 Lactobacillus paracollinoides" ;
                                         skos:definition "None" ;
                                         skos:prefLabel "WLP669 Lactobacillus paracollinoides" .


###  http://peterbrau.com/whitelabs/yeast-bank/wlp670-american-farmhouse-blend
wlp:wlp670-american-farmhouse-blend rdf:type owl:NamedIndividual ,
                                             yeast:BrewersYeast ,
                                             yeast:WildYeastAndBacteria ;
                                    yeast:hasAlcoholTolerance "Medium (5 - 10%)" ;
                                    yeast:hasFlocculation "Medium" ;
                                    yeast:hasHighAttenuation 82.00 ;
                                    yeast:hasHighOptimumFermentationTemperature 72.00 ;
                                    yeast:hasLowAttenuation 75.00 ;
                                    yeast:hasLowOptimumFermentationTemperature 68.00 ;
                                    dcterms:bibliographicCitation "http://www.whitelabs.com/yeast-bank/wlp670-american-farmhouse-blend" ;
                                    gr:hasMPN "wlp670" ;
                                    rdfs:label "WLP670 American Farmhouse Blend" ;
                                    skos:definition "None" ;
                                    skos:prefLabel "WLP670 American Farmhouse Blend" .


###  http://peterbrau.com/whitelabs/yeast-bank/wlp672-lactobacillus-brevis
wlp:wlp672-lactobacillus-brevis rdf:type owl:NamedIndividual ,
                                         yeast:BrewersYeast ,
                                         yeast:WildYeastAndBacteria ;
                                yeast:hasAlcoholTolerance "Medium (5 - 10%)" ;
                                yeast:hasFlocculation "Low" ;
                                yeast:hasHighAttenuation 0.00 ;
                                yeast:hasLowAttenuation 0.00 ;
                                yeast:usedForBrewingStyle beertype:berliner-weisse ,
                                                          beertype:flanders-brown ,
                                                          beertype:flanders-red ,
                                                          beertype:geuze ,
                                                          beertype:gose ,
                                                          beertype:lambic ;
                                dcterms:bibliographicCitation "http://www.whitelabs.com/yeast-bank/wlp672-lactobacillus-brevis" ;
                                gr:hasMPN "wlp672" ;
                                rdfs:label "WLP672 Lactobacillus brevis" ;
                                skos:definition "None" ;
                                skos:prefLabel "WLP672 Lactobacillus brevis" .


###  http://peterbrau.com/whitelabs/yeast-bank/wlp673-lactobacillus-buchneri
wlp:wlp673-lactobacillus-buchneri rdf:type owl:NamedIndividual ,
                                           yeast:BrewersYeast ,
                                           yeast:WildYeastAndBacteria ;
                                  yeast:usedForBrewingStyle beertype:berliner-weisse ,
                                                            beertype:cider ,
                                                            beertype:gose ;
                                  dcterms:bibliographicCitation "http://www.whitelabs.com/yeast-bank/wlp673-lactobacillus-buchneri" ;
                                  gr:hasMPN "wlp673" ;
                                  rdfs:label "WLP673 Lactobacillus buchneri" ;
                                  skos:definition "This strain is recommended for souring. Can be used for sour kettle/mash or in secondary fermentation. <15 IBU tolerance. Little to no attenuation. Experiments have shown less than <5% attenuation." ;
                                  skos:prefLabel "WLP673 Lactobacillus buchneri" .


###  http://peterbrau.com/whitelabs/yeast-bank/wlp675-malolactic-cultures
wlp:wlp675-malolactic-cultures rdf:type owl:NamedIndividual ,
                                        yeast:BrewersYeast ;
                               dcterms:bibliographicCitation "http://www.whitelabs.com/yeast-bank/wlp675-malolactic-cultures" ;
                               gr:hasMPN "wlp675" ;
                               rdfs:label "WLP675 Malolactic Cultures" ;
                               skos:definition "None" ;
                               skos:prefLabel "WLP675 Malolactic Cultures" .


###  http://peterbrau.com/whitelabs/yeast-bank/wlp677-lactobacillus-delbrueckii-bacteria
wlp:wlp677-lactobacillus-delbrueckii-bacteria rdf:type owl:NamedIndividual ,
                                                       yeast:BrewersYeast ,
                                                       yeast:WildYeastAndBacteria ;
                                              yeast:hasAlcoholTolerance "Medium (5 - 10%)" ;
                                              yeast:hasFlocculation "Low" ;
                                              yeast:hasHighAttenuation 0.00 ;
                                              yeast:hasHighOptimumFermentationTemperature 75.00 ;
                                              yeast:hasLowAttenuation 0.00 ;
                                              yeast:hasLowOptimumFermentationTemperature 70.00 ;
                                              yeast:usedForBrewingStyle beertype:berliner-weisse ,
                                                                        beertype:flanders-brown ,
                                                                        beertype:flanders-red ,
                                                                        beertype:geuze ,
                                                                        beertype:gose ,
                                                                        beertype:lambic ;
                                              dcterms:bibliographicCitation "http://www.whitelabs.com/yeast-bank/wlp677-lactobacillus-delbrueckii-bacteria" ;
                                              gr:hasMPN "wlp677" ;
                                              rdfs:label "WLP677 Lactobacillus delbrueckii Bacteria" ;
                                              skos:definition "This lactic acid bacteria produces moderate levels of acidity and sour flavors found in lambics, Berliner Weisse, sour brown ales and gueuze." ;
                                              skos:prefLabel "WLP677 Lactobacillus delbrueckii Bacteria" .


###  http://peterbrau.com/whitelabs/yeast-bank/wlp678-lactobacillus-hilgardii
wlp:wlp678-lactobacillus-hilgardii rdf:type owl:NamedIndividual ,
                                            yeast:BrewersYeast ,
                                            yeast:WildYeastAndBacteria ;
                                   yeast:usedForBrewingStyle beertype:berliner-weisse ,
                                                             beertype:cider ,
                                                             beertype:flanders-brown ,
                                                             beertype:flanders-red ,
                                                             beertype:geuze ,
                                                             beertype:gose ,
                                                             beertype:lambic ;
                                   dcterms:bibliographicCitation "http://www.whitelabs.com/yeast-bank/wlp678-lactobacillus-hilgardii" ;
                                   gr:hasMPN "wlp678" ;
                                   rdfs:label "WLP678 Lactobacillus hilgardii" ;
                                   skos:definition "None" ;
                                   skos:prefLabel "WLP678 Lactobacillus hilgardii" .


###  http://peterbrau.com/whitelabs/yeast-bank/wlp692-debaryomyces-hansenii
wlp:wlp692-debaryomyces-hansenii rdf:type owl:NamedIndividual ,
                                          yeast:BrewersYeast ,
                                          yeast:WildYeastAndBacteria ;
                                 yeast:usedForBrewingStyle beertype:cider ,
                                                           beertype:geuze ,
                                                           beertype:lambic ;
                                 dcterms:bibliographicCitation "http://www.whitelabs.com/yeast-bank/wlp692-debaryomyces-hansenii" ;
                                 gr:hasMPN "wlp692" ;
                                 rdfs:label "WLP692 Debaryomyces hansenii" ;
                                 skos:definition "None" ;
                                 skos:prefLabel "WLP692 Debaryomyces hansenii" .


###  http://peterbrau.com/whitelabs/yeast-bank/wlp693-lactobacillus-plantarum
wlp:wlp693-lactobacillus-plantarum rdf:type owl:NamedIndividual ,
                                            yeast:BrewersYeast ,
                                            yeast:WildYeastAndBacteria ;
                                   yeast:usedForBrewingStyle beertype:berliner-weisse ,
                                                             beertype:cider ,
                                                             beertype:gose ;
                                   dcterms:bibliographicCitation "http://www.whitelabs.com/yeast-bank/wlp693-lactobacillus-plantarum" ;
                                   gr:hasMPN "wlp693" ;
                                   rdfs:label "WLP693 Lactobacillus plantarum" ;
                                   skos:definition "None" ;
                                   skos:prefLabel "WLP693 Lactobacillus plantarum" .


###  http://peterbrau.com/whitelabs/yeast-bank/wlp700-flor-sherry-yeast
wlp:wlp700-flor-sherry-yeast rdf:type owl:NamedIndividual ,
                                      yeast:BrewersYeast ;
                             yeast:hasAlcoholTolerance "Very High (Over 15%)" ;
                             yeast:hasHighAttenuation 100.00 ;
                             yeast:hasHighOptimumFermentationTemperature 100.00 ;
                             yeast:hasLowAttenuation 80.00 ;
                             yeast:hasLowOptimumFermentationTemperature 70.00 ;
                             yeast:usedForBrewingStyle beertype:madeira ,
                                                       beertype:port ,
                                                       beertype:sherry ;
                             dcterms:bibliographicCitation "http://www.whitelabs.com/yeast-bank/wlp700-flor-sherry-yeast" ;
                             gr:hasMPN "wlp700" ;
                             rdfs:label "WLP700 Flor Sherry Yeast" ;
                             skos:definition "Creates green almond, Granny Smith apple and nougat characteristics found in sherry. Develops a film (flor) on the surface of the wine. For use in secondary fermentation." ;
                             skos:prefLabel "WLP700 Flor Sherry Yeast" .


###  http://peterbrau.com/whitelabs/yeast-bank/wlp705-sake-7-yeast
wlp:wlp705-sake-7-yeast rdf:type owl:NamedIndividual ,
                                 yeast:BrewersYeast ;
                        yeast:hasAlcoholTolerance "Very High (Over 15%)" ;
                        yeast:hasHighAttenuation 100.00 ;
                        yeast:hasHighOptimumFermentationTemperature 100.00 ;
                        yeast:hasLowAttenuation 80.00 ;
                        yeast:hasLowOptimumFermentationTemperature 70.00 ;
                        yeast:usedForBrewingStyle beertype:sake ;
                        dcterms:bibliographicCitation "http://www.whitelabs.com/yeast-bank/wlp705-sake-7-yeast" ;
                        gr:hasMPN "wlp705" ;
                        rdfs:label "WLP705 Sake #7 Yeast" ;
                        skos:definition "Produces a full-bodied character and subtle fruity esters. For use in rice-based fermentations; typically used in conjunction with koji (to produce fermentable sugar). This strain can also be used successfully in beer fermentations." ;
                        skos:prefLabel "WLP705 Sake #7 Yeast" .


###  http://peterbrau.com/whitelabs/yeast-bank/wlp707-california-pinot-noir-yeast
wlp:wlp707-california-pinot-noir-yeast rdf:type owl:NamedIndividual ,
                                                yeast:BrewersYeast ;
                                       yeast:hasAlcoholTolerance "Very High (Over 15%)" ;
                                       yeast:hasFlocculation "N/A" ;
                                       yeast:hasHighAttenuation 100.00 ;
                                       yeast:hasHighOptimumFermentationTemperature 90.00 ;
                                       yeast:hasLowAttenuation 80.00 ;
                                       yeast:hasLowOptimumFermentationTemperature 60.00 ;
                                       yeast:usedForBrewingStyle beertype:cabernet-sauvignon ,
                                                                 beertype:chardonnay ,
                                                                 beertype:pinot-noir ;
                                       dcterms:bibliographicCitation "http://www.whitelabs.com/yeast-bank/wlp707-california-pinot-noir-yeast" ;
                                       gr:hasMPN "wlp707" ;
                                       rdfs:label "WLP707 California Pinot Noir Yeast" ;
                                       skos:definition "Produces fruity and complex aromas and is reliable for difficult fermentations. Isolated from pinot noir grapes in Davis, CA." ;
                                       skos:prefLabel "WLP707 California Pinot Noir Yeast" .


###  http://peterbrau.com/whitelabs/yeast-bank/wlp709-sake-9-yeast
wlp:wlp709-sake-9-yeast rdf:type owl:NamedIndividual ,
                                 yeast:BrewersYeast ;
                        yeast:hasAlcoholTolerance "High (10 - 15%)" ;
                        yeast:hasFlocculation "Medium to Low" ;
                        yeast:hasHighAttenuation 78.00 ;
                        yeast:hasHighOptimumFermentationTemperature 68.00 ;
                        yeast:hasLowAttenuation 72.00 ;
                        yeast:hasLowOptimumFermentationTemperature 62.00 ;
                        yeast:usedForBrewingStyle beertype:sake ;
                        dcterms:bibliographicCitation "http://www.whitelabs.com/yeast-bank/wlp709-sake-9-yeast" ;
                        gr:hasMPN "wlp709" ;
                        rdfs:label "WLP709 Sake #9 Yeast" ;
                        skos:definition "For use in rice-based fermentations. Traditional strain used in Ginjo-shu production because of the yeast’s development of high fragrance components. Also a fairly strong fermenter, but producing a foamless fermentation." ;
                        skos:prefLabel "WLP709 Sake #9 Yeast" .


###  http://peterbrau.com/whitelabs/yeast-bank/wlp715-champagne-yeast
wlp:wlp715-champagne-yeast rdf:type owl:NamedIndividual ,
                                    yeast:BrewersYeast ;
                           yeast:hasAlcoholTolerance "Very High (Over 15%)" ;
                           yeast:hasFlocculation "Low" ;
                           yeast:hasHighAttenuation 100.00 ;
                           yeast:hasHighOptimumFermentationTemperature 75.00 ;
                           yeast:hasLowAttenuation 75.00 ;
                           yeast:hasLowOptimumFermentationTemperature 70.00 ;
                           yeast:usedForBrewingStyle beertype:american-pale-ale ,
                                                     beertype:apple-wine ,
                                                     beertype:belgian-table-bier ,
                                                     beertype:champagne-sparkling-wine ,
                                                     beertype:cider ,
                                                     beertype:cyser ,
                                                     beertype:english-cider ,
                                                     beertype:french-cider ,
                                                     beertype:new-england-cider ,
                                                     beertype:specialty-belgian ,
                                                     beertype:sweet-cider ,
                                                     beertype:traditional-perry ,
                                                     beertype:tripel ;
                           dcterms:bibliographicCitation "http://www.whitelabs.com/yeast-bank/wlp715-champagne-yeast" ;
                           gr:hasMPN "wlp715" ;
                           rdfs:label "WLP715 Champagne Yeast" ;
                           skos:definition "Classic yeast that is neutral in character, and a strong fermenter. Great for use in wine, cider and mead allowing the character of the fermentables to become prominent flavors." ;
                           skos:prefLabel "WLP715 Champagne Yeast" .


###  http://peterbrau.com/whitelabs/yeast-bank/wlp718-avize-wine-yeast
wlp:wlp718-avize-wine-yeast rdf:type owl:NamedIndividual ,
                                     yeast:BrewersYeast ;
                            yeast:hasAlcoholTolerance "High (10 - 15%)" ;
                            yeast:hasFlocculation "Low" ;
                            yeast:hasHighAttenuation 100.00 ;
                            yeast:hasHighOptimumFermentationTemperature 90.00 ;
                            yeast:hasLowAttenuation 80.00 ;
                            yeast:hasLowOptimumFermentationTemperature 60.00 ;
                            yeast:usedForBrewingStyle beertype:chardonnay ;
                            dcterms:bibliographicCitation "http://www.whitelabs.com/yeast-bank/wlp718-avize-wine-yeast" ;
                            gr:hasMPN "wlp718" ;
                            rdfs:label "WLP718 Avize Wine Yeast" ;
                            skos:definition "Champagne isolate used for complexity in whites. Contributes elegance, especially in barrel fermented Chardonnays." ;
                            skos:prefLabel "WLP718 Avize Wine Yeast" .


###  http://peterbrau.com/whitelabs/yeast-bank/wlp720-sweet-mead-wine-yeast
wlp:wlp720-sweet-mead-wine-yeast rdf:type owl:NamedIndividual ,
                                          yeast:BrewersYeast ;
                                 yeast:hasAlcoholTolerance "High (10 - 15%)" ;
                                 yeast:hasFlocculation "Low" ;
                                 yeast:hasHighOptimumFermentationTemperature 75.00 ;
                                 yeast:hasLowOptimumFermentationTemperature 70.00 ;
                                 yeast:usedForBrewingStyle beertype:apple-wine ,
                                                           beertype:braggot ,
                                                           beertype:brandy ,
                                                           beertype:cider ,
                                                           beertype:cyser ,
                                                           beertype:gew-rztraminer ,
                                                           beertype:riesling ,
                                                           beertype:rum ,
                                                           beertype:semi-sweet-mead ,
                                                           beertype:sweet-mead ;
                                 dcterms:bibliographicCitation "http://www.whitelabs.com/yeast-bank/wlp720-sweet-mead-wine-yeast" ;
                                 gr:hasMPN "wlp720" ;
                                 rdfs:label "WLP720 Sweet Mead/Wine Yeast" ;
                                 skos:definition "Produces a slightly fruity flavor and aroma while leaving more residual sweetness than WLP715 Champagne Yeast. This strain will tolerate alcohol concentrations up to 15%." ;
                                 skos:prefLabel "WLP720 Sweet Mead/Wine Yeast" .


###  http://peterbrau.com/whitelabs/yeast-bank/wlp727-steinberg-geisenheim-wine-yeast
wlp:wlp727-steinberg-geisenheim-wine-yeast rdf:type owl:NamedIndividual ,
                                                    yeast:BrewersYeast ;
                                           yeast:hasAlcoholTolerance "High (10 - 15%)" ;
                                           yeast:hasFlocculation "Low" ;
                                           yeast:hasHighAttenuation 100.00 ;
                                           yeast:hasHighOptimumFermentationTemperature 90.00 ;
                                           yeast:hasLowAttenuation 80.00 ;
                                           yeast:hasLowOptimumFermentationTemperature 50.00 ;
                                           yeast:usedForBrewingStyle beertype:gew-rztraminer ,
                                                                     beertype:riesling ;
                                           dcterms:bibliographicCitation "http://www.whitelabs.com/yeast-bank/wlp727-steinberg-geisenheim-wine-yeast" ;
                                           gr:hasMPN "wlp727" ;
                                           rdfs:label "WLP727 Steinberg-Geisenheim Wine Yeast" ;
                                           skos:definition "High fruit ester production. German in origin and cold tolerant." ;
                                           skos:prefLabel "WLP727 Steinberg-Geisenheim Wine Yeast" .


###  http://peterbrau.com/whitelabs/yeast-bank/wlp730-chardonnay-white-wine-yeast
wlp:wlp730-chardonnay-white-wine-yeast rdf:type owl:NamedIndividual ,
                                                yeast:BrewersYeast ;
                                       yeast:hasAlcoholTolerance "High (10 - 15%)" ;
                                       yeast:hasFlocculation "Low" ;
                                       yeast:hasHighAttenuation 100.00 ;
                                       yeast:hasHighOptimumFermentationTemperature 90.00 ;
                                       yeast:hasLowAttenuation 80.00 ;
                                       yeast:hasLowOptimumFermentationTemperature 50.00 ;
                                       yeast:usedForBrewingStyle beertype:chardonnay ;
                                       dcterms:bibliographicCitation "http://www.whitelabs.com/yeast-bank/wlp730-chardonnay-white-wine-yeast" ;
                                       gr:hasMPN "wlp730" ;
                                       rdfs:label "WLP730 Chardonnay White Wine Yeast" ;
                                       skos:definition "Dry wine yeast with slight ester production and low sulfur dioxide production which enhances varietal character." ;
                                       skos:prefLabel "WLP730 Chardonnay White Wine Yeast" .


###  http://peterbrau.com/whitelabs/yeast-bank/wlp735-french-white-wine-yeast
wlp:wlp735-french-white-wine-yeast rdf:type owl:NamedIndividual ,
                                            yeast:BrewersYeast ;
                                   yeast:hasAlcoholTolerance "Very High (Over 15%)" ;
                                   yeast:hasFlocculation "Low" ;
                                   yeast:hasHighAttenuation 100.00 ;
                                   yeast:hasHighOptimumFermentationTemperature 90.00 ;
                                   yeast:hasLowAttenuation 80.00 ;
                                   yeast:hasLowOptimumFermentationTemperature 60.00 ;
                                   yeast:usedForBrewingStyle beertype:merlot ,
                                                             beertype:zinfandel ;
                                   dcterms:bibliographicCitation "http://www.whitelabs.com/yeast-bank/wlp735-french-white-wine-yeast" ;
                                   gr:hasMPN "wlp735" ;
                                   rdfs:label "WLP735 French White Wine Yeast" ;
                                   skos:definition "Classic yeast for white wine fermentation, giving an enhanced creamy texture. Low foam producer." ;
                                   skos:prefLabel "WLP735 French White Wine Yeast" .


###  http://peterbrau.com/whitelabs/yeast-bank/wlp740-merlot-red-wine-yeast
wlp:wlp740-merlot-red-wine-yeast rdf:type owl:NamedIndividual ,
                                          yeast:BrewersYeast ;
                                 yeast:hasAlcoholTolerance "Very High (Over 15%)" ;
                                 yeast:hasFlocculation "Low" ;
                                 yeast:hasHighAttenuation 100.00 ;
                                 yeast:hasHighOptimumFermentationTemperature 90.00 ;
                                 yeast:hasLowAttenuation 80.00 ;
                                 yeast:hasLowOptimumFermentationTemperature 60.00 ;
                                 yeast:usedForBrewingStyle beertype:chardonnay ,
                                                           beertype:cyser ,
                                                           beertype:merlot ,
                                                           beertype:pinot-noir ,
                                                           beertype:sauvignon-blanc ,
                                                           beertype:semillon ,
                                                           beertype:shiraz ;
                                 dcterms:bibliographicCitation "http://www.whitelabs.com/yeast-bank/wlp740-merlot-red-wine-yeast" ;
                                 gr:hasMPN "wlp740" ;
                                 rdfs:label "WLP740 Merlot Red Wine Yeast" ;
                                 skos:definition "Neutral character, with low fusel-alcohol production. Ferments dry." ;
                                 skos:prefLabel "WLP740 Merlot Red Wine Yeast" .


###  http://peterbrau.com/whitelabs/yeast-bank/wlp749-assmanshausen-wine-yeast
wlp:wlp749-assmanshausen-wine-yeast rdf:type owl:NamedIndividual ,
                                             yeast:BrewersYeast ;
                                    yeast:hasAlcoholTolerance "Very High (Over 15%)" ;
                                    yeast:hasFlocculation "Low" ;
                                    yeast:hasHighAttenuation 100.00 ;
                                    yeast:hasHighOptimumFermentationTemperature 90.00 ;
                                    yeast:hasLowAttenuation 80.00 ;
                                    yeast:hasLowOptimumFermentationTemperature 50.00 ;
                                    yeast:usedForBrewingStyle beertype:pinot-noir ,
                                                              beertype:riesling ,
                                                              beertype:zinfandel ;
                                    dcterms:bibliographicCitation "http://www.whitelabs.com/yeast-bank/wlp749-assmanshausen-wine-yeast" ;
                                    gr:hasMPN "wlp749" ;
                                    rdfs:label "WLP749 Assmanshausen Wine Yeast" ;
                                    skos:definition "This strain is a German red wine yeast that is cold tolerant. Produces spicy fruit aromas." ;
                                    skos:prefLabel "WLP749 Assmanshausen Wine Yeast" .


###  http://peterbrau.com/whitelabs/yeast-bank/wlp750-french-red-wine-yeast
wlp:wlp750-french-red-wine-yeast rdf:type owl:NamedIndividual ,
                                          yeast:BrewersYeast ;
                                 yeast:hasAlcoholTolerance "Very High (Over 15%)" ;
                                 yeast:hasFlocculation "Low" ;
                                 yeast:hasHighAttenuation 100.00 ;
                                 yeast:hasHighOptimumFermentationTemperature 90.00 ;
                                 yeast:hasLowAttenuation 80.00 ;
                                 yeast:hasLowOptimumFermentationTemperature 60.00 ;
                                 yeast:usedForBrewingStyle beertype:cabernet-franc ,
                                                           beertype:cabernet-sauvignon ,
                                                           beertype:cyser ,
                                                           beertype:gin ,
                                                           beertype:grappa ,
                                                           beertype:malbec ,
                                                           beertype:merlot ,
                                                           beertype:sauvignon-blanc ,
                                                           beertype:semillon ,
                                                           beertype:vodka ;
                                 dcterms:bibliographicCitation "http://www.whitelabs.com/yeast-bank/wlp750-french-red-wine-yeast" ;
                                 gr:hasMPN "wlp750" ;
                                 rdfs:label "WLP750 French Red Wine Yeast" ;
                                 skos:definition "Classic Bordeaux yeast with a rich, smooth flavor profile." ;
                                 skos:prefLabel "WLP750 French Red Wine Yeast" .


###  http://peterbrau.com/whitelabs/yeast-bank/wlp760-cabernet-red-wine-yeast
wlp:wlp760-cabernet-red-wine-yeast rdf:type owl:NamedIndividual ,
                                            yeast:BrewersYeast ;
                                   yeast:hasAlcoholTolerance "Very High (Over 15%)" ;
                                   yeast:hasFlocculation "Low" ;
                                   yeast:hasHighAttenuation 100.00 ;
                                   yeast:hasHighOptimumFermentationTemperature 90.00 ;
                                   yeast:hasLowAttenuation 80.00 ;
                                   yeast:hasLowOptimumFermentationTemperature 60.00 ;
                                   yeast:usedForBrewingStyle beertype:cabernet-franc ,
                                                             beertype:cabernet-sauvignon ,
                                                             beertype:chardonnay ,
                                                             beertype:grenache ,
                                                             beertype:nebbiolo ,
                                                             beertype:sangiovese ,
                                                             beertype:zinfandel ;
                                   dcterms:bibliographicCitation "http://www.whitelabs.com/yeast-bank/wlp760-cabernet-red-wine-yeast" ;
                                   gr:hasMPN "wlp760" ;
                                   rdfs:label "WLP760 Cabernet Red Wine Yeast" ;
                                   skos:definition "A versatile strain for full-bodied red wines with ester production that complements dry aromatic white wines." ;
                                   skos:prefLabel "WLP760 Cabernet Red Wine Yeast" .


###  http://peterbrau.com/whitelabs/yeast-bank/wlp770-suremain-burgundy-wine-yeast
wlp:wlp770-suremain-burgundy-wine-yeast rdf:type owl:NamedIndividual ,
                                                 yeast:BrewersYeast ;
                                        yeast:hasAlcoholTolerance "Very High (Over 15%)" ;
                                        yeast:hasFlocculation "Low" ;
                                        yeast:hasHighAttenuation 100.00 ;
                                        yeast:hasHighOptimumFermentationTemperature 90.00 ;
                                        yeast:hasLowAttenuation 80.00 ;
                                        yeast:hasLowOptimumFermentationTemperature 60.00 ;
                                        yeast:usedForBrewingStyle beertype:chardonnay ,
                                                                  beertype:pinot-noir ,
                                                                  beertype:sauvignon-blanc ;
                                        dcterms:bibliographicCitation "http://www.whitelabs.com/yeast-bank/wlp770-suremain-burgundy-wine-yeast" ;
                                        gr:hasMPN "wlp770" ;
                                        rdfs:label "WLP770 Suremain Burgundy Wine Yeast" ;
                                        skos:definition "Emphasizes fruit aromas in barrel fermentations. Posesses a high nutrient requirement to avoid volatile acidity production." ;
                                        skos:prefLabel "WLP770 Suremain Burgundy Wine Yeast" .


###  http://peterbrau.com/whitelabs/yeast-bank/wlp773-scottish-cider-yeast-blend
wlp:wlp773-scottish-cider-yeast-blend rdf:type owl:NamedIndividual ,
                                               yeast:BrewersYeast ;
                                      yeast:hasFlocculation "Medium to High" ;
                                      yeast:hasHighAttenuation 80.00 ;
                                      yeast:hasLowAttenuation 80.00 ;
                                      yeast:usedForBrewingStyle beertype:cider ,
                                                                beertype:cyser ,
                                                                beertype:english-cider ,
                                                                beertype:french-cider ,
                                                                beertype:new-england-cider ,
                                                                beertype:sweet-cider ;
                                      dcterms:bibliographicCitation "http://www.whitelabs.com/yeast-bank/wlp773-scottish-cider-yeast-blend" ;
                                      gr:hasMPN "wlp773" ;
                                      rdfs:label "WLP773 Scottish Cider Yeast Blend" ;
                                      skos:definition "This is an exciting blend of two ale strains and one wine strain. Unlike a lot of ale strains that typically dry out most ciders, this unique blend of Saccharomyces strains will leave some residual sweetness for a smooth mouthfeel. This strain is perfect for those looking for a still cider with some lingering apple characteristic or a dryer sparkling cider." ;
                                      skos:prefLabel "WLP773 Scottish Cider Yeast Blend" .


###  http://peterbrau.com/whitelabs/yeast-bank/wlp775-english-cider-yeast
wlp:wlp775-english-cider-yeast rdf:type owl:NamedIndividual ,
                                        yeast:BrewersYeast ;
                               yeast:hasAlcoholTolerance "Medium - High (8 - 12%)" ;
                               yeast:hasFlocculation "Medium" ;
                               yeast:hasHighAttenuation 100.00 ;
                               yeast:hasHighOptimumFermentationTemperature 75.00 ;
                               yeast:hasLowAttenuation 80.00 ;
                               yeast:hasLowOptimumFermentationTemperature 68.00 ;
                               yeast:usedForBrewingStyle beertype:apple-wine ,
                                                         beertype:cider ,
                                                         beertype:cyser ,
                                                         beertype:english-cider ,
                                                         beertype:semi-sweet-mead ;
                               dcterms:bibliographicCitation "http://www.whitelabs.com/yeast-bank/wlp775-english-cider-yeast" ;
                               gr:hasMPN "wlp775" ;
                               rdfs:label "WLP775 English Cider Yeast" ;
                               skos:definition "Classic cider yeast that ferments dry, but retains the flavor from apples." ;
                               skos:prefLabel "WLP775 English Cider Yeast" .


###  http://peterbrau.com/whitelabs/yeast-bank/wlp780-thai-rice-chong-yeast
wlp:wlp780-thai-rice-chong-yeast rdf:type owl:NamedIndividual ,
                                          yeast:BrewersYeast ;
                                 yeast:hasAlcoholTolerance "High (10 - 15%)" ;
                                 yeast:hasHighAttenuation 76.00 ;
                                 yeast:hasLowAttenuation 76.00 ;
                                 yeast:usedForBrewingStyle beertype:barleywine-ale ,
                                                           beertype:sake ;
                                 dcterms:bibliographicCitation "http://www.whitelabs.com/yeast-bank/wlp780-thai-rice-chong-yeast" ;
                                 gr:hasMPN "wlp780" ;
                                 rdfs:label "WLP780 Thai Rice Chong Yeast" ;
                                 skos:definition "None" ;
                                 skos:prefLabel "WLP780 Thai Rice Chong Yeast" .


###  http://peterbrau.com/whitelabs/yeast-bank/wlp800-pilsner-lager-yeast
wlp:wlp800-pilsner-lager-yeast rdf:type owl:NamedIndividual ,
                                        yeast:BrewersYeast ;
                               yeast:hasAlcoholTolerance "Medium (5 - 10%)" ;
                               yeast:hasFlocculation "Medium to High" ;
                               yeast:hasHighAttenuation 77.00 ;
                               yeast:hasHighOptimumFermentationTemperature 55.00 ;
                               yeast:hasLowAttenuation 72.00 ;
                               yeast:hasLowOptimumFermentationTemperature 50.00 ;
                               yeast:usedForBrewingStyle beertype:american-lager ,
                                                         beertype:american-light-lager ,
                                                         beertype:bock ,
                                                         beertype:bohemian-pilsner ,
                                                         beertype:doppelbock ,
                                                         beertype:lager ,
                                                         beertype:m-nchen-helles ,
                                                         beertype:m-nchner-dunkel ,
                                                         beertype:m-rzen ,
                                                         beertype:schwarzbier ,
                                                         beertype:vienna-lager ;
                               dcterms:bibliographicCitation "http://www.whitelabs.com/yeast-bank/wlp800-pilsner-lager-yeast" ;
                               gr:hasMPN "wlp800" ;
                               rdfs:label "WLP800 Pilsner Lager Yeast" ;
                               skos:definition "A classic pilsner strain from the Czech Republic, this strain produces a clean, crisp beer that’s somewhat dry with a malty finish. A to-style pilsner strain, this yeast is also well suited for thirst quenching lagers such as Munich helles, dunkels and American lagers." ;
                               skos:prefLabel "WLP800 Pilsner Lager Yeast" .


###  http://peterbrau.com/whitelabs/yeast-bank/wlp802-czech-budejovice-lager-yeast
wlp:wlp802-czech-budejovice-lager-yeast rdf:type owl:NamedIndividual ,
                                                 yeast:BrewersYeast ;
                                        yeast:hasAlcoholTolerance "Medium (5 - 10%)" ;
                                        yeast:hasFlocculation "Medium" ;
                                        yeast:hasHighAttenuation 80.00 ;
                                        yeast:hasHighOptimumFermentationTemperature 55.00 ;
                                        yeast:hasLowAttenuation 75.00 ;
                                        yeast:hasLowOptimumFermentationTemperature 50.00 ;
                                        yeast:usedForBrewingStyle beertype:american-lager ,
                                                                  beertype:american-light-lager ,
                                                                  beertype:bock ,
                                                                  beertype:bohemian-pilsner ,
                                                                  beertype:doppelbock ,
                                                                  beertype:lager ,
                                                                  beertype:m-nchen-helles ,
                                                                  beertype:m-nchner-dunkel ,
                                                                  beertype:m-rzen ,
                                                                  beertype:schwarzbier ,
                                                                  beertype:vienna-lager ;
                                        dcterms:bibliographicCitation "http://www.whitelabs.com/yeast-bank/wlp802-czech-budejovice-lager-yeast" ;
                                        gr:hasMPN "wlp802" ;
                                        rdfs:label "WLP802 Czech Budejovice Lager Yeast " ;
                                        skos:definition "A pilsner lager yeast from southern Czech Republic, this strain produces dry and crisp lagers with low diacetyl production. With up to 80% attenuation, this strain will make a dry beer and showcase rounded hop bitterness. Low diacetyl production makes conditioning of this beer an ease." ;
                                        skos:prefLabel "WLP802 Czech Budejovice Lager Yeast " .


###  http://peterbrau.com/whitelabs/yeast-bank/wlp810-san-francisco-lager-yeast
wlp:wlp810-san-francisco-lager-yeast rdf:type owl:NamedIndividual ,
                                              yeast:BrewersYeast ;
                                     yeast:hasAlcoholTolerance "Medium - High (8 - 12%)" ;
                                     yeast:hasFlocculation "High" ;
                                     yeast:hasHighAttenuation 70.00 ;
                                     yeast:hasHighOptimumFermentationTemperature 65.00 ;
                                     yeast:hasLowAttenuation 65.00 ;
                                     yeast:hasLowOptimumFermentationTemperature 58.00 ;
                                     yeast:usedForBrewingStyle beertype:american-lager ,
                                                               beertype:american-light-lager ,
                                                               beertype:bock ,
                                                               beertype:bohemian-pilsner ,
                                                               beertype:doppelbock ,
                                                               beertype:lager ,
                                                               beertype:m-nchen-helles ,
                                                               beertype:m-nchner-dunkel ,
                                                               beertype:m-rzen ,
                                                               beertype:schwarzbier ,
                                                               beertype:vienna-lager ;
                                     dcterms:bibliographicCitation "http://www.whitelabs.com/yeast-bank/wlp810-san-francisco-lager-yeast" ;
                                     gr:hasMPN "wlp810" ;
                                     rdfs:label "WLP810 San Francisco Lager Yeast " ;
                                     skos:definition "A unique lager strain because it can ferment at a wide range of temperatures — 50°F (10°C) to 65°F (18°C) — while retaining lager-like characteristics. This strain is traditionally used to brew the California common or steam beer styles. At lower temperatures can also produce märzens, pilsners and helles style lagers." ;
                                     skos:prefLabel "WLP810 San Francisco Lager Yeast " .


###  http://peterbrau.com/whitelabs/yeast-bank/wlp815-belgian-lager-yeast
wlp:wlp815-belgian-lager-yeast rdf:type owl:NamedIndividual ,
                                        yeast:BrewersYeast ;
                               yeast:hasAlcoholTolerance "Medium (5 - 10%)" ;
                               yeast:hasFlocculation "Medium" ;
                               yeast:hasHighAttenuation 78.00 ;
                               yeast:hasHighOptimumFermentationTemperature 55.00 ;
                               yeast:hasLowAttenuation 72.00 ;
                               yeast:hasLowOptimumFermentationTemperature 50.00 ;
                               yeast:usedForBrewingStyle beertype:american-lager ,
                                                         beertype:american-light-lager ,
                                                         beertype:baltic-style-porter ,
                                                         beertype:bohemian-pilsner ,
                                                         beertype:doppelbock ,
                                                         beertype:lager ,
                                                         beertype:schwarzbier ,
                                                         beertype:vault-seasonal-release ,
                                                         beertype:vienna-lager ;
                               dcterms:bibliographicCitation "http://www.whitelabs.com/yeast-bank/wlp815-belgian-lager-yeast" ;
                               gr:hasMPN "wlp815" ;
                               rdfs:label "WLP815 Belgian Lager Yeast" ;
                               skos:definition "A clean, crisp European lager yeast with low sulfur production. This strain originates from a very old brewery in west Belgium. Great for European-style pilsners, dark lagers, Vienna lagers, and American-style lagers." ;
                               skos:prefLabel "WLP815 Belgian Lager Yeast" .


###  http://peterbrau.com/whitelabs/yeast-bank/wlp820-oktoberfest-m-rzen-lager-yeast
wlp:wlp820-oktoberfest-m-rzen-lager-yeast rdf:type owl:NamedIndividual ,
                                                   yeast:BrewersYeast ;
                                          yeast:hasAlcoholTolerance "Medium - High (8 - 12%)" ;
                                          yeast:hasFlocculation "Medium" ;
                                          yeast:hasHighAttenuation 73.00 ;
                                          yeast:hasHighOptimumFermentationTemperature 58.00 ;
                                          yeast:hasLowAttenuation 65.00 ;
                                          yeast:hasLowOptimumFermentationTemperature 52.00 ;
                                          yeast:usedForBrewingStyle beertype:american-lager ,
                                                                    beertype:american-light-lager ,
                                                                    beertype:baltic-style-porter ,
                                                                    beertype:bock ,
                                                                    beertype:bohemian-pilsner ,
                                                                    beertype:doppelbock ,
                                                                    beertype:lager ,
                                                                    beertype:m-nchen-helles ,
                                                                    beertype:m-nchner-dunkel ,
                                                                    beertype:m-rzen ,
                                                                    beertype:schwarzbier ,
                                                                    beertype:vienna-lager ;
                                          dcterms:bibliographicCitation "http://www.whitelabs.com/yeast-bank/wlp820-oktoberfest-m-rzen-lager-yeast" ;
                                          gr:hasMPN "wlp820" ;
                                          rdfs:label "WLP820 Oktoberfest/Märzen Lager Yeast" ;
                                          skos:definition "This strain is ideal for producing malty lagers. Residual sweetness further helps promote malt nuances while contributing to a balanced finish. The first generation of this strain can be slow, so we encourage using a larger initial culture or scheduling longer fermentation and conditioning times. Great for lagers with a wide gravity range including bocks, doppelbocks, märzens, Oktoberfests and American amber lagers." ;
                                          skos:prefLabel "WLP820 Oktoberfest/Märzen Lager Yeast" .


###  http://peterbrau.com/whitelabs/yeast-bank/wlp830-german-lager-yeast
wlp:wlp830-german-lager-yeast rdf:type owl:NamedIndividual ,
                                       yeast:BrewersYeast ;
                              yeast:hasAlcoholTolerance "Medium (5 - 10%)" ;
                              yeast:hasFlocculation "Medium" ;
                              yeast:hasHighAttenuation 79.00 ;
                              yeast:hasHighOptimumFermentationTemperature 55.00 ;
                              yeast:hasLowAttenuation 74.00 ;
                              yeast:hasLowOptimumFermentationTemperature 50.00 ;
                              yeast:usedForBrewingStyle beertype:american-lager ,
                                                        beertype:american-light-lager ,
                                                        beertype:bock ,
                                                        beertype:bohemian-pilsner ,
                                                        beertype:doppelbock ,
                                                        beertype:lager ,
                                                        beertype:m-nchen-helles ,
                                                        beertype:m-nchner-dunkel ,
                                                        beertype:m-rzen ,
                                                        beertype:schwarzbier ,
                                                        beertype:vienna-lager ;
                              dcterms:bibliographicCitation "http://www.whitelabs.com/yeast-bank/wlp830-german-lager-yeast" ;
                              gr:hasMPN "wlp830" ;
                              rdfs:label "WLP830 German Lager Yeast" ;
                              skos:definition "Our most popular lager yeast, this strain is one of the most widely used lager strains in the world. It can be used in almost any lager style and tends to produce clean and crisp beers with some accentuation of hop characteristics." ;
                              skos:prefLabel "WLP830 German Lager Yeast" .


###  http://peterbrau.com/whitelabs/yeast-bank/wlp833-german-bock-lager-yeast
wlp:wlp833-german-bock-lager-yeast rdf:type owl:NamedIndividual ,
                                            yeast:BrewersYeast ;
                                   yeast:hasAlcoholTolerance "Medium - High (8 - 12%)" ;
                                   yeast:hasFlocculation "Medium" ;
                                   yeast:hasHighAttenuation 76.00 ;
                                   yeast:hasHighOptimumFermentationTemperature 55.00 ;
                                   yeast:hasLowAttenuation 70.00 ;
                                   yeast:hasLowOptimumFermentationTemperature 48.00 ;
                                   yeast:usedForBrewingStyle beertype:american-lager ,
                                                             beertype:bock ,
                                                             beertype:doppelbock ,
                                                             beertype:lager ,
                                                             beertype:m-nchen-helles ,
                                                             beertype:m-nchner-dunkel ,
                                                             beertype:m-rzen ,
                                                             beertype:schwarzbier ,
                                                             beertype:vienna-lager ;
                                   dcterms:bibliographicCitation "http://www.whitelabs.com/yeast-bank/wlp833-german-bock-lager-yeast" ;
                                   gr:hasMPN "wlp833" ;
                                   rdfs:label "WLP833 German Bock Lager Yeast" ;
                                   skos:definition "From the Alps of southern Bavaria, this yeast produces a beer that is well-balanced between malt and hop character. The excellent malt profile makes it well suited for bocks, dopplebocks, and Oktoberfest- style beers. A very versatile lager yeast, it has gained tremendous popularity for use in classic American-style lagers." ;
                                   skos:prefLabel "WLP833 German Bock Lager Yeast" .


###  http://peterbrau.com/whitelabs/yeast-bank/wlp835-german-x-lager-yeast
wlp:wlp835-german-x-lager-yeast rdf:type owl:NamedIndividual ,
                                         yeast:BrewersYeast ;
                                yeast:hasAlcoholTolerance "Medium - High (8 - 12%)" ;
                                yeast:hasFlocculation "Medium" ;
                                yeast:hasHighAttenuation 76.00 ;
                                yeast:hasHighOptimumFermentationTemperature 54.00 ;
                                yeast:hasLowAttenuation 70.00 ;
                                yeast:hasLowOptimumFermentationTemperature 50.00 ;
                                yeast:usedForBrewingStyle beertype:bock ,
                                                          beertype:doppelbock ,
                                                          beertype:lager ,
                                                          beertype:m-nchen-helles ,
                                                          beertype:m-nchner-dunkel ,
                                                          beertype:m-rzen ;
                                dcterms:bibliographicCitation "http://www.whitelabs.com/yeast-bank/wlp835-german-x-lager-yeast" ;
                                gr:hasMPN "wlp835" ;
                                rdfs:label "WLP835 German X Lager Yeast" ;
                                skos:definition "Classic yeast from a famous Bavarian monastery. This strain develops a creamy, malty beer profile with low sulfur production and low esters. It is a great choice for styles like traditional Helles, Oktoberfest, Bock, and Dunkel." ;
                                skos:prefLabel "WLP835 German X Lager Yeast" .


###  http://peterbrau.com/whitelabs/yeast-bank/wlp838-southern-german-lager-yeast
wlp:wlp838-southern-german-lager-yeast rdf:type owl:NamedIndividual ,
                                                yeast:BrewersYeast ;
                                       yeast:hasAlcoholTolerance "Medium (5 - 10%)" ;
                                       yeast:hasFlocculation "Medium to High" ;
                                       yeast:hasHighAttenuation 76.00 ;
                                       yeast:hasHighOptimumFermentationTemperature 55.00 ;
                                       yeast:hasLowAttenuation 68.00 ;
                                       yeast:hasLowOptimumFermentationTemperature 50.00 ;
                                       yeast:usedForBrewingStyle beertype:american-lager ,
                                                                 beertype:american-light-lager ,
                                                                 beertype:bock ,
                                                                 beertype:bohemian-pilsner ,
                                                                 beertype:doppelbock ,
                                                                 beertype:lager ,
                                                                 beertype:m-nchen-helles ,
                                                                 beertype:m-nchner-dunkel ,
                                                                 beertype:m-rzen ,
                                                                 beertype:schwarzbier ,
                                                                 beertype:vienna-lager ;
                                       dcterms:bibliographicCitation "http://www.whitelabs.com/yeast-bank/wlp838-southern-german-lager-yeast" ;
                                       gr:hasMPN "wlp838" ;
                                       rdfs:label "WLP838 Southern German Lager Yeast" ;
                                       skos:definition "This yeast is characterized by a malty finish, balanced aroma and great flocculation. It is a strong fermenter which produces slight sulfur and low diacetyl during fermentation. This strain benefits from a diacetyl rest and conditioning." ;
                                       skos:prefLabel "WLP838 Southern German Lager Yeast" .


###  http://peterbrau.com/whitelabs/yeast-bank/wlp840-american-lager-yeast
wlp:wlp840-american-lager-yeast rdf:type owl:NamedIndividual ,
                                         yeast:BrewersYeast ;
                                yeast:hasAlcoholTolerance "Medium (5 - 10%)" ;
                                yeast:hasFlocculation "Medium" ;
                                yeast:hasHighAttenuation 80.00 ;
                                yeast:hasHighOptimumFermentationTemperature 55.00 ;
                                yeast:hasLowAttenuation 75.00 ;
                                yeast:hasLowOptimumFermentationTemperature 50.00 ;
                                yeast:usedForBrewingStyle beertype:american-lager ,
                                                          beertype:american-light-lager ,
                                                          beertype:bohemian-pilsner ,
                                                          beertype:lager ,
                                                          beertype:m-nchen-helles ,
                                                          beertype:m-nchner-dunkel ,
                                                          beertype:m-rzen ,
                                                          beertype:schwarzbier ,
                                                          beertype:vienna-lager ;
                                dcterms:bibliographicCitation "http://www.whitelabs.com/yeast-bank/wlp840-american-lager-yeast" ;
                                gr:hasMPN "wlp840" ;
                                rdfs:label "WLP840 American Lager Yeast" ;
                                skos:definition "This strain makes dry and clean lagers with a light note of apple fruitiness. Sulfur and diacetyl production is minimal making this strain easy to work with and fitting for American-style lagers." ;
                                skos:prefLabel "WLP840 American Lager Yeast" .


###  http://peterbrau.com/whitelabs/yeast-bank/wlp845-fast-lager-yeast
wlp:wlp845-fast-lager-yeast rdf:type owl:NamedIndividual ,
                                     yeast:BrewersYeast ;
                            yeast:hasHighAttenuation 78.00 ;
                            yeast:hasLowAttenuation 75.00 ;
                            yeast:usedForBrewingStyle beertype:american-lager ,
                                                      beertype:american-light-lager ,
                                                      beertype:bock ,
                                                      beertype:bohemian-pilsner ,
                                                      beertype:doppelbock ,
                                                      beertype:lager ,
                                                      beertype:m-nchen-helles ,
                                                      beertype:m-nchner-dunkel ,
                                                      beertype:m-rzen ,
                                                      beertype:schwarzbier ,
                                                      beertype:vienna-lager ;
                            dcterms:bibliographicCitation "http://www.whitelabs.com/yeast-bank/wlp845-fast-lager-yeast" ;
                            gr:hasMPN "wlp845" ;
                            rdfs:label "WLP845 Fast Lager Yeast" ;
                            skos:definition "Use this strain when you need a lager sooner rather than later. Low sulfur production and medium flocculation characteristics." ;
                            skos:prefLabel "WLP845 Fast Lager Yeast" .


###  http://peterbrau.com/whitelabs/yeast-bank/wlp850-copenhagen-lager-yeast
wlp:wlp850-copenhagen-lager-yeast rdf:type owl:NamedIndividual ,
                                           yeast:BrewersYeast ;
                                  yeast:hasAlcoholTolerance "Medium (5 - 10%)" ;
                                  yeast:hasFlocculation "Medium" ;
                                  yeast:hasHighAttenuation 78.00 ;
                                  yeast:hasHighOptimumFermentationTemperature 58.00 ;
                                  yeast:hasLowAttenuation 72.00 ;
                                  yeast:hasLowOptimumFermentationTemperature 50.00 ;
                                  yeast:usedForBrewingStyle beertype:american-lager ,
                                                            beertype:american-light-lager ,
                                                            beertype:bock ,
                                                            beertype:bohemian-pilsner ,
                                                            beertype:doppelbock ,
                                                            beertype:lager ,
                                                            beertype:m-nchen-helles ,
                                                            beertype:m-nchner-dunkel ,
                                                            beertype:m-rzen ,
                                                            beertype:schwarzbier ,
                                                            beertype:vienna-lager ;
                                  dcterms:bibliographicCitation "http://www.whitelabs.com/yeast-bank/wlp850-copenhagen-lager-yeast" ;
                                  gr:hasMPN "wlp850" ;
                                  rdfs:label "WLP850 Copenhagen Lager Yeast" ;
                                  skos:definition "This northern European lager strain emphasizes clean and crisp characteristics. Malt flavors tend to be secondary, promoting clean drinkability. It is ideal for Vienna, schwarzbier or American-style lagers." ;
                                  skos:prefLabel "WLP850 Copenhagen Lager Yeast" .


###  http://peterbrau.com/whitelabs/yeast-bank/wlp860-munich-helles-lager-yeast
wlp:wlp860-munich-helles-lager-yeast rdf:type owl:NamedIndividual ,
                                              yeast:BrewersYeast ;
                                     yeast:hasAlcoholTolerance "Medium (5 - 10%)" ;
                                     yeast:hasFlocculation "Medium" ;
                                     yeast:hasHighAttenuation 72.00 ;
                                     yeast:hasHighOptimumFermentationTemperature 52.00 ;
                                     yeast:hasLowAttenuation 68.00 ;
                                     yeast:hasLowOptimumFermentationTemperature 48.00 ;
                                     yeast:usedForBrewingStyle beertype:bohemian-pilsner ,
                                                               beertype:lager ,
                                                               beertype:m-nchen-helles ,
                                                               beertype:m-rzen ,
                                                               beertype:schwarzbier ;
                                     dcterms:bibliographicCitation "http://www.whitelabs.com/yeast-bank/wlp860-munich-helles-lager-yeast" ;
                                     gr:hasMPN "wlp860" ;
                                     rdfs:label "WLP860 Munich Helles Lager Yeast" ;
                                     skos:definition "This yeast helps to produce a malty, yet balanced traditional Munich-style lager. Clean and a strong fermentor, it’s great for a variety of lager styles ranging from helles to rauchbier." ;
                                     skos:prefLabel "WLP860 Munich Helles Lager Yeast" .


###  http://peterbrau.com/whitelabs/yeast-bank/wlp885-zurich-lager-yeast
wlp:wlp885-zurich-lager-yeast rdf:type owl:NamedIndividual ,
                                       yeast:BrewersYeast ;
                              yeast:hasAlcoholTolerance "Very High (Over 15%)" ;
                              yeast:hasFlocculation "Medium" ;
                              yeast:hasHighAttenuation 80.00 ;
                              yeast:hasHighOptimumFermentationTemperature 55.00 ;
                              yeast:hasLowAttenuation 70.00 ;
                              yeast:hasLowOptimumFermentationTemperature 50.00 ;
                              yeast:usedForBrewingStyle beertype:american-lager ,
                                                        beertype:american-light-lager ,
                                                        beertype:bock ,
                                                        beertype:bohemian-pilsner ,
                                                        beertype:doppelbock ,
                                                        beertype:lager ,
                                                        beertype:m-nchen-helles ,
                                                        beertype:m-nchner-dunkel ,
                                                        beertype:m-rzen ,
                                                        beertype:schwarzbier ,
                                                        beertype:vienna-lager ;
                              dcterms:bibliographicCitation "http://www.whitelabs.com/yeast-bank/wlp885-zurich-lager-yeast" ;
                              gr:hasMPN "wlp885" ;
                              rdfs:label "WLP885 Zurich Lager Yeast" ;
                              skos:definition "A Swiss-style lager yeast that with proper care can be used to produce lagers over 11% ABV. Sulfur and diacetyl production is minimal." ;
                              skos:prefLabel "WLP885 Zurich Lager Yeast" .


###  http://peterbrau.com/whitelabs/yeast-bank/wlp920-old-bavarian-lager-yeast
wlp:wlp920-old-bavarian-lager-yeast rdf:type owl:NamedIndividual ,
                                             yeast:BrewersYeast ;
                                    yeast:hasAlcoholTolerance "Medium - High (8 - 12%)" ;
                                    yeast:hasFlocculation "Medium" ;
                                    yeast:hasHighAttenuation 73.00 ;
                                    yeast:hasHighOptimumFermentationTemperature 55.00 ;
                                    yeast:hasLowAttenuation 66.00 ;
                                    yeast:hasLowOptimumFermentationTemperature 50.00 ;
                                    yeast:usedForBrewingStyle beertype:baltic-style-porter ,
                                                              beertype:bock ,
                                                              beertype:doppelbock ,
                                                              beertype:lager ,
                                                              beertype:m-nchner-dunkel ,
                                                              beertype:m-rzen ,
                                                              beertype:schwarzbier ,
                                                              beertype:vienna-lager ;
                                    dcterms:bibliographicCitation "http://www.whitelabs.com/yeast-bank/wlp920-old-bavarian-lager-yeast" ;
                                    gr:hasMPN "wlp920" ;
                                    rdfs:label "WLP920 Old Bavarian Lager Yeast" ;
                                    skos:definition "From Southern Germany, this yeast finishes malty with a slight ester profile. Use in beers such as Oktoberfests, bocks, and dark lagers." ;
                                    skos:prefLabel "WLP920 Old Bavarian Lager Yeast" .


###  http://peterbrau.com/whitelabs/yeast-bank/wlp925-high-pressure-lager-yeast
wlp:wlp925-high-pressure-lager-yeast rdf:type owl:NamedIndividual ,
                                              yeast:BrewersYeast ;
                                     yeast:hasAlcoholTolerance "Medium (5 - 10%)" ;
                                     yeast:hasFlocculation "Medium" ;
                                     yeast:hasHighAttenuation 82.00 ;
                                     yeast:hasHighOptimumFermentationTemperature 68.00 ;
                                     yeast:hasLowAttenuation 73.00 ;
                                     yeast:hasLowOptimumFermentationTemperature 62.00 ;
                                     yeast:usedForBrewingStyle beertype:american-lager ,
                                                               beertype:american-light-lager ,
                                                               beertype:bohemian-pilsner ,
                                                               beertype:lager ,
                                                               beertype:vienna-lager ;
                                     dcterms:bibliographicCitation "http://www.whitelabs.com/yeast-bank/wlp925-high-pressure-lager-yeast" ;
                                     gr:hasMPN "wlp925" ;
                                     rdfs:label "WLP925 High Pressure Lager Yeast" ;
                                     skos:definition "Used to ferment lager beer in one week. Ferment at room temperature; 62-68°F (17-20°C) under 1.0 bar (14.7 PSI) until final gravity is obtained, generally in one week. Lager the beer at 35°F (2°C), 15 PSI, for 3-5 days to condition. Sulfur production is strong the first 2 days, then disappears by day 5." ;
                                     skos:prefLabel "WLP925 High Pressure Lager Yeast" .


###  http://peterbrau.com/whitelabs/yeast-bank/wlp940-mexican-lager-yeast
wlp:wlp940-mexican-lager-yeast rdf:type owl:NamedIndividual ,
                                        yeast:BrewersYeast ;
                               yeast:hasAlcoholTolerance "Medium (5 - 10%)" ;
                               yeast:hasFlocculation "Medium" ;
                               yeast:hasHighAttenuation 78.00 ;
                               yeast:hasHighOptimumFermentationTemperature 55.00 ;
                               yeast:hasLowAttenuation 70.00 ;
                               yeast:hasLowOptimumFermentationTemperature 50.00 ;
                               yeast:usedForBrewingStyle beertype:american-lager ,
                                                         beertype:american-light-lager ,
                                                         beertype:bock ,
                                                         beertype:bohemian-pilsner ,
                                                         beertype:doppelbock ,
                                                         beertype:lager ,
                                                         beertype:m-nchen-helles ,
                                                         beertype:m-nchner-dunkel ,
                                                         beertype:m-rzen ,
                                                         beertype:schwarzbier ,
                                                         beertype:vienna-lager ;
                               dcterms:bibliographicCitation "http://www.whitelabs.com/yeast-bank/wlp940-mexican-lager-yeast" ;
                               gr:hasMPN "wlp940" ;
                               rdfs:label "WLP940 Mexican Lager Yeast" ;
                               skos:definition "From Mexico City, this strain produces clean lager beers with a crisp finish. It keeps drinkability on the forefront while allowing malt and hop flavors and aromas to be background notes. A great strain choice for light-style lagers like Vienna-style." ;
                               skos:prefLabel "WLP940 Mexican Lager Yeast" .


###  Generated by the OWL API (version 4.5.9.2019-02-01T07:24:44Z) https://github.com/owlcs/owlapi
